<?xml version="1.0" encoding="UTF-8"?>
<rdf:RDF xmlns:rdf="http://www.w3.org/1999/02/22-rdf-syntax-ns#" xmlns:skos="http://www.w3.org/2004/02/skos/core#" xmlns:owl="http://www.w3.org/2002/07/owl#" xmlns:xsd="http://www.w3.org/2001/XMLSchema#" xmlns:swrl="http://www.w3.org/2003/11/swrl#" xmlns:swrlb="http://www.w3.org/2003/11/swrlb#" xmlns:rdfs="http://www.w3.org/2000/01/rdf-schema#" xml:base="https://ontology.swissartresearch.net/aaao/">
  <!--
						This document represents the formal specification for an unofficial formal extension of the CIDOC CRM designed for application in the area of art and architectural historical research. The scope of this extension is to support art and architectural research in the sense of the study of primary and secondary documents for the derivation, manually and programmatically, of historically contextual facts that can be used to support reflection and structured argumentation. The core expressivity that this extension adds is the ability to accurately express historically bound, contextual social facts relative to the agents holding those beliefs and the temporal period for which those beliefs were valid. The extension enables this expressivity by introducing the notions of institutional fact and speech act as core modelling concepts. Institutional facts are collective beliefs about the world held by groups for a period of time. Such collective beliefs, while subjectively grounded, are epistemically objective for the community over which they hold sway. Introducing the notion of institutional fact allows for a specialization of the core CRM to be able to express these social realities (expressed in simple, aoristic binary properties in the core CRM) in their full social complexity as temporally and socially bound beliefs. The concomitant core notion introduced in this extension is the idea of Speech Act in the Austinian and Serlean sense. A speech act is a kind of intentional event (E7 Activity of CRM base) in which agents purposefully apply a rule and perform a set practice in order to bring about a new social state or institutional fact. Introducing the notion of speech act provides both a high-level ontological category and set of relations for describing the kinds of events which are the cause of institutional facts as well as providing a starting point for the analysis of the non-truth propositional use of information objects. In speech acts, information objects (e.g. phrases and formulae) are deployed not to convey states of the world but to generate states of the world. The subject of historical investigation is not simply the bare facts available to an empirical analysis of the physical world but involves an investigation of the social activities which generated contexts of understanding and belief that may differ significantly across times and peoples. Materializing the social facts implicit in CRM base as explicit institutional facts gives them a richer ontological representation and offers a consistent epistemological approach to their study by recognizing social, negotiated facts as objective realities in themselves and treating them as first order entities of study. This involves a departure from the aims of CRM base which is guided by an information integration functionality which favours the representation of the latest state of knowledge in a presentist perspective. In the study of the history of art and architecture it is in no small part the different non-coinciding facts held or supported by different actors over different times which are of interest. The materialization of institutional facts supports the information management functionality which guides this informal extension of the CIDOC CRM and which aims to support historians in representing the positive knowledge they can gather from primary and secondary sources of evidence of both past simple and institutional facts for the purposes of proposing hypotheses and analyses of texts, authors, periods, works and so on. In this regard, AAAo also provides an initial limited set of classes for describing traditional and digital methods of deriving facts from texts, in order to support the linking of contemporary research processes as provenance nodes for the different data points of simple and institutional facts which they generate in the course of their research.  Examples Used  With this in mind, examples have been chosen which potentially support a variety of social facts. Some of these facts, i.e., those held by one group of people at some time or other, may directly contradict another, i.e., that held by a different group of people at some potentially different time. Most of the examples have been reused across different types of social fact, in order to tell more completely the history of the objects in question and the beliefs that have been held about them by specific groups of people over a given period of time. These histories can in themselves be quite complex. References are thus provided for further contextualization. These appear in brackets following the examples, like so:    The Ownership Status (ZE8) of the Gʼpsgolox totem pole (E22) as 'has current owner' the Haisla people (E74) from 1872 - 2012 holds for the Haisla people (E74) and as 'has current owner' the Swedish National Museum of Ethnography (E74) from 1929 - 2006 holds for the Swedish Polity. (https://en.wikipedia.org/wiki/G%CA%BCpsgolox_totem_pole)    Compatibility and Nomenclature  This unofficial extension of the CIDOC CRM is formulated in relation to the following official extensions:    CIDOC CRM v.7.1.3  CIDOC CRM Dig v.4.0  CRMtex v.1.0  LRM v.1.0     The specification consists of a set of declarations for formalized classes and properties that extend the CIDOC CRM and the above official extensions.   Adopting the conventions of the CIDOC CRM each class and property have been given an identifier in addition to their names. The naming convention adopted for this extension is:  ZE = class  ZP = property  The choice of these names was arbitrary, making a conceptual connection with the official CRM representation while clearly distinguishing the new classes and properties from those of either CRM base or its official extensions.  Namespace  https://ontology.swissartresearch.net/aaao     Maintenance and Archiving  AAAo is an actively maintained ontology. It is our aim to develop publicly and participatively, learning from and engaging with the scholarly community that adopts it. Towards this end we maintain the ontology with the following processes and relative tools.  Ontology Development  We adopt the OntoMe tool developed by LARHRA to manage the ontology and produce editions. This ensures a consistent management of the ontology and provides a public space to engage in revisions.  The maintenance space for the ontology can be found here: https://ontome.net/project/69   Please note, at time of publishing, OntoME is not capable of producing complete, provenanced RDF serializations, so please only use the official RDF for this standard stored on our github. See below.   Issue Management and Revision Storage  We adopt github as a platform for inviting and managing issues related to the ontology as well as providing an active place to be able to access the latest edition of the ontology, its specification and relevant documentation.  The address for the github repository is: https://github.com/swiss-art-research-net/aaao   Acknowledgements  The initiative for creating, developing and maintaining this ontology is made possible by important on-going funding and institutional commitment, which is gratefully acknowledged here.  Funding Support    The development of the initial version (v0.9) of AAAo was initiated and generously funded by ETH Zurich, Chair of the History and Theory of Architecture, Prof. Maarten Delbeke.  The  continuted development and enrichment of the latest version (v1.5) has been generously funded as part of the Open Research Data (ORD) initiative by swissuniversities.    Collaborations  Collaborations with the following projects provided important feedback and input for the testing and further elaboration of the standard:  The initial modelling around this extension have been supported by collaboration with:    the Releven: Re-evaluating the Eleventh Century project  the Globalise project     Institutional Support  The continuous maintenance and promotion of AAAo is made possible by the initial commitment of its partners to maintain the ontology and promote its understanding and adoption.    Swiss Art Research Infrastructure - University of Zurich  Takin.solutions     
						Exported from OntoME: Art and Architectural Argumentation Ontology Version 2.0
						Official URI : https://ontology.swissartresearch.net/aaao/
						-->
  <rdfs:Class rdf:about="http://www.ics.forth.gr/isl/CRMdig/D7_Digital_Machine_Event">
    <skos:notation rdf:datatype="http://www.w3.org/2001/XMLSchema#string">D7</skos:notation>
    <rdfs:comment xml:lang="en" rdf:datatype="http://www.w3.org/2001/XMLSchema#string">This class comprises events that happen on physical digital devices following a human activity that intentionally caused its immediate or delayed initiation and results in the creation of a new instance of D1 Digital Object on behalf of the human actor.
The input of a D7 Digital Machine Event may be parameter settings and/or data to be processed. Some D7 Digital Machine Events may form part of a wider E65 Creation event. In this case, all machine output of the partial events is regarded as creation of the overall activity.</rdfs:comment>
    <rdfs:label xml:lang="en">Digital Machine Event</rdfs:label>
  </rdfs:Class>
  <rdfs:Class rdf:about="http://www.cidoc-crm.org/cidoc-crm/E1_CRM_Entity">
    <skos:notation rdf:datatype="http://www.w3.org/2001/XMLSchema#string">E1</skos:notation>
    <rdfs:comment xml:lang="en" rdf:datatype="http://www.w3.org/2001/XMLSchema#string">This class comprises all things in the universe of discourse of the CIDOC Conceptual Reference Model. It is an abstract concept providing for three general properties:Identification by name or appellation, and in particular by a preferred identifierClassification by type, allowing further refinement of the specific subclass an instance belongs to Attachment of free text and other unstructured data for the expression of anything not captured by formal propertiesAll other classes within the CIDOC CRM are directly or indirectly specialisations of E1 CRM Entity. </rdfs:comment>
    <rdfs:label xml:lang="en">CRM Entity</rdfs:label>
  </rdfs:Class>
  <rdfs:Class rdf:about="http://www.cidoc-crm.org/cidoc-crm/E2_Temporal_Entity">
    <skos:notation rdf:datatype="http://www.w3.org/2001/XMLSchema#string">E2</skos:notation>
    <rdfs:comment xml:lang="en" rdf:datatype="http://www.w3.org/2001/XMLSchema#string">This class comprises all phenomena, such as the instances of E4 Periods and E5 Events, which happen over a limited extent in time. This extent in time must be contiguous, i.e., without gaps. In case the defining kinds of phenomena for an instance of E2 Temporal Entity cease to happen, and occur later again at another time, we regard that the former instance of E2 Temporal Entity has ended and a new instance has come into existence. In more intuitive terms, the same event cannot happen twice.In some contexts, such phenomena are also called perdurants. This class is disjoint from E77 Persistent Item and is an abstract class that typically has no direct instances. E2 Temporal Entity is specialized into E4 Period, which applies to a particular geographic area (defined with a greater or lesser degree of precision), and E3 Condition State, which applies to instances of E18 Physical Thing.</rdfs:comment>
    <rdfs:label xml:lang="en">Temporal Entity</rdfs:label>
  </rdfs:Class>
  <rdfs:Class rdf:about="http://www.cidoc-crm.org/cidoc-crm/E4_Period">
    <skos:notation rdf:datatype="http://www.w3.org/2001/XMLSchema#string">E4</skos:notation>
    <rdfs:comment xml:lang="en" rdf:datatype="http://www.w3.org/2001/XMLSchema#string">This class comprises sets of coherent phenomena or cultural manifestations occurring in time and space.It is the social or physical coherence of these phenomena that identify an instance of E4 Period and not the associated spatiotemporal extent. This extent is only the “ground” or space in an abstract physical sense that the actual process of growth, spread and retreat has covered. Consequently, different periods can overlap and coexist in time and space, such as when a nomadic culture exists in the same area and time as a sedentary culture. This also means that overlapping land use rights, common among first nations, amounts to overlapping periods.Often, this class is used to describe prehistoric or historic periods such as the “Neolithic Period”, the “Ming Dynasty” or the “McCarthy Era”, but also geopolitical units and activities of settlements are regarded as special cases of E4 Period. However, there are no assumptions about the scale of the associated phenomena. In particular all events are seen as synthetic processes consisting of coherent phenomena. Therefore, E4 Period is a superclass of E5 Event. For example, a modern clinical birth, an instance of E67 Birth, can be seen as both a single event, i.e., an instance of E5 Event, and as an extended period, i.e., an instance of E4 Period, that consists of multiple physical processes and complementary activities performed by multiple instances of E39 Actor.As the actual extent of an instance of E4 Period in spacetime we regard the trajectories of the participating physical things during their participation in an instance of E4 Period. This includes the open spaces via which these things have interacted and the spaces by which they had the potential to interact during that period or event in the way defined by the type of the respective period or event. Examples include the air in a meeting room transferring the voices of the participants. Since these phenomena are fuzzy, we assume the spatiotemporal extent to be contiguous, except for cases of phenomena spreading out over islands or other separated areas, including geopolitical units distributed over disconnected areas such as islands or colonies.Whether the trajectories necessary for participants to travel between these areas are regarded as part of the spatiotemporal extent or not has to be decided in each case based on a concrete analysis, taking use of the sea for other purposes than travel, such as fishing, into consideration. One may also argue that the activities to govern disconnected areas imply travelling through spaces connecting them and that these areas hence are spatially connected in a way, but it appears counterintuitive to consider for instance travel routes in international waters as extensions of geopolitical units.Consequently, an instance of E4 Period may occupy a number of disjoint spacetime volumes, however there must not be a discontinuity in the time-span covered by these spacetime volumes. This means that an instance of E4 Period must be contiguous in time. If it has ended in all areas, it has ended as a whole. However, it may end in one area before another, such as in the Polynesian migration, and it continues as long as it is ongoing in at least one area.We model E4 Period as a subclass of E2 Temporal Entity and of E92 Spacetime Volume. The latter is intended as a phenomenal spacetime volume as defined in CIDOC CRMgeo (Doerr   Hiebel, 2013). By virtue of this multiple inheritance, we can discuss the physical extent of an instance of E4 Period without representing each instance of it together with an instance of its associated spacetime volume. This model combines two quite different kinds of substance: an instance of E4 Period is a phenomenon while an instance of E92 Spacetime Volume is an aggregation of points in spacetime. However, the real spatiotemporal extent of an instance of E4 Period is regarded to be unique to it due to all its details and fuzziness; its identity and existence depends uniquely on the identity of the instance of E4 Period. Therefore, this multiple inheritance is unambiguous and effective and furthermore corresponds to the intuitions of natural language.Typical use of this class in cultural heritage documentation is for documenting cultural and artistic periods. There are two different conceptualisations of ‘artistic style’, defined either by physical features or by historical context. For example, “Impressionism” can be viewed as a period in the European sphere of influence lasting from approximately 1870 to 1905 during which paintings with particular characteristics were produced by a group of artists that included (among others) Monet, Renoir, Pissarro, Sisley and Degas. Alternatively, it can be regarded as a style applicable to all paintings sharing the characteristics of the works produced by the Impressionist painters, regardless of historical context. The first interpretation is an instance of E4 Period, and the second defines morphological object types that fall under E55 Type.A geopolitical unit as a specific case of an instance of E4 Period is the set of activities and phenomena related to the claim of power, the consequences of belonging to a jurisdictional area and an administrative system that establishes a geopolitical unit. Examples from the modern period are countries or administrative areas of countries such as districts whose actions and structures define activities and phenomena in the area that they intend to govern. The borders of geopolitical units are often defined in contracts or treaties although they may deviate from the actual practice. The spatiotemporal properties of Geopolitical units can be modelled through the properties inherited from E92 Spacetime Volume.Another specific case of an instance of E4 Period is the actual extent of the set of activities and phenomena as evidenced by their physical traces that define a settlement, such as the populated period of Nineveh. </rdfs:comment>
    <rdfs:label xml:lang="en">Period</rdfs:label>
  </rdfs:Class>
  <rdfs:Class rdf:about="http://www.cidoc-crm.org/cidoc-crm/E5_Event">
    <skos:notation rdf:datatype="http://www.w3.org/2001/XMLSchema#string">E5</skos:notation>
    <rdfs:comment xml:lang="en" rdf:datatype="http://www.w3.org/2001/XMLSchema#string">This class comprises distinct, delimited and coherent processes and interactions of a material nature, in cultural, social or physical systems, involving and affecting instances of E77 Persistent Item in a way characteristic of the kind of process. Typical examples are meetings, births, deaths, actions of decision taking, making or inventing things, but also more complex and extended ones such as conferences, elections, building of a castle, or battles.While the continuous growth of a tree lacks the limits characteristic of an event, its germination from a seed does qualify as an event. Similarly, the blowing of the wind lacks the distinctness and limits of an event, but a hurricane, flood or earthquake would qualify as an event. Mental processes are considered as events, in cases where they are connected with the material externalization of their results; for example, the creation of a poem, a performance or a change of intention that becomes obvious from subsequent actions or declarations.The effects of an instance of E5 Event may not lead to relevant permanent changes of properties or relations of the items involved in it, for example an unrecorded performance. Of course, in order to be documented, some kind of evidence for an event must exist, be it witnesses, traces or products of the event.While instances of E4 Period always require some form of coherence between its constituent phenomena, in addition, the essential constituents of instances of E5 Event should contribute to an overall effect; for example, the statements made during a meeting and the listening of the audience.Viewed at a coarse level of detail, an instance of E5 Event may appear as if it had an ‘instantaneous’ overall effect, but any process or interaction of material nature in reality have an extent in time and space. At a fine level, instances of E5 Event may be analysed into component phenomena and phases within a space and timeframe, and as such can be seen as a period, regardless of the size of the phenomena. The reverse is not necessarily the case: not all instances of E4 Period give rise to a noteworthy overall effect and are thus not instances of E5 Event.</rdfs:comment>
    <rdfs:label xml:lang="en">Event</rdfs:label>
  </rdfs:Class>
  <rdfs:Class rdf:about="http://www.cidoc-crm.org/cidoc-crm/E7_Activity">
    <skos:notation rdf:datatype="http://www.w3.org/2001/XMLSchema#string">E7</skos:notation>
    <rdfs:comment xml:lang="en" rdf:datatype="http://www.w3.org/2001/XMLSchema#string">This class comprises actions intentionally carried out by instances of E39 Actor that result in changes of state in the cultural, social, or physical systems documented. This notion includes complex, composite and long-lasting actions such as the building of a settlement or a war, as well as simple, short-lived actions such as the opening of a door.</rdfs:comment>
    <rdfs:label xml:lang="en">Activity</rdfs:label>
  </rdfs:Class>
  <rdfs:Class rdf:about="http://www.cidoc-crm.org/cidoc-crm/E8_Acquisition">
    <skos:notation rdf:datatype="http://www.w3.org/2001/XMLSchema#string">E8</skos:notation>
    <rdfs:comment xml:lang="en" rdf:datatype="http://www.w3.org/2001/XMLSchema#string">This class comprises transfers of legal ownership from one or more instances of E39 Actor to one or more other instances of E39 Actor. The class also applies to the establishment or loss of ownership of instances of E18 Physical Thing. It does not, however, imply changes of any other kinds of right. The recording of the donor and/or recipient is optional. It is possible that in an instance of E8 Acquisition there is either no donor or no recipient. Depending on the circumstances, it may describe:the beginning of ownershipthe end of ownershipthe transfer of ownershipthe acquisition from an unknown sourcethe loss of title due to destruction of the itemIt may also describe events where a collector appropriates legal title, for example by annexation or field collection. The interpretation of the museum notion of "accession" differs between institutions. The CIDOC CRM therefore models legal ownership (E8 Acquisition) and physical custody (E10 Transfer of Custody) separately. Institutions will then model their specific notions of accession and deaccession as combinations of these.</rdfs:comment>
    <rdfs:label xml:lang="en">Acquisition</rdfs:label>
  </rdfs:Class>
  <rdfs:Class rdf:about="http://www.cidoc-crm.org/cidoc-crm/E10_Transfer_of_Custody">
    <skos:notation rdf:datatype="http://www.w3.org/2001/XMLSchema#string">E10</skos:notation>
    <rdfs:comment xml:lang="en" rdf:datatype="http://www.w3.org/2001/XMLSchema#string">This class comprises transfers of the physical custody or the legal responsibility for the physical custody of objects. The recording of the donor or recipient is optional. It is possible that in an instance of E10 Transfer of Custody there is either no donor or no recipient. Depending on the circumstances, it may describe: the beginning of custody (there is no previous custodian)the end of custody (there is no subsequent custodian)the transfer of custody (transfer from one custodian to the next)the receipt of custody from an unknown source (the previous custodian is unknown)the declared loss of an object (the current or subsequent custodian is unknown)In the event that only a single kind of transfer of custody occurs, either the legal responsibility for the custody or the actual physical possession of the object but not both, this difference should be expressed using the property P2 has type (is type of). The sense of physical possession requires that the object of custody be in the hands of the keeper at least with a part representative for the whole. The way, in which a representative part is defined, should ensure that it is unambiguous who keeps a part and who the whole and should be consistent with the identity criteria of the kept instance of E18 Physical Thing. The interpretation of the museum notion of "accession" differs between institutions. The CIDOC CRM therefore models legal ownership and physical custody separately. Institutions will then model their specific notions of accession and deaccession as combinations of these. Theft is a specific case of illegal transfer of custody.</rdfs:comment>
    <rdfs:label xml:lang="en">Transfer of Custody</rdfs:label>
  </rdfs:Class>
  <rdfs:Class rdf:about="http://www.cidoc-crm.org/cidoc-crm/E13_Attribute_Assignment">
    <skos:notation rdf:datatype="http://www.w3.org/2001/XMLSchema#string">E13</skos:notation>
    <rdfs:comment xml:lang="en" rdf:datatype="http://www.w3.org/2001/XMLSchema#string">This class comprises the actions of making assertions about one property of an object or any single relation between two items or concepts. The type of the property asserted to hold between two items or concepts can be described by the property P177 assigned property of type (is type of property assigned): E55 Type. For example, the class describes the actions of people making propositions and statements during certain scientific/scholarly procedures, e.g., the person and date when a condition statement was made, an identifier was assigned, the museum object was measured, etc. Which kinds of such assignments and statements need to be documented explicitly in structures of a schema rather than free text, depends on whether this information should be accessible by structured queries.This class allows for the documentation of how the respective assignment came about, and whose opinion it was. Note that all instances of properties described in a knowledge base are the opinion of someone. Per default, they are the opinion of the team maintaining the knowledge base. This fact must not individually be registered for all instances of properties provided by the maintaining team, because it would result in an endless recursion of whose opinion was the description of an opinion. Therefore, the use of instances of E13 Attribute Assignment marks the fact, that the maintaining team is in general neutral to the validity of the respective assertion, but registers someone else’s opinion and how it came about.All properties assigned in such an action can also be seen as directly relating the respective pair of items or concepts. Multiple use of instances of E13 Attribute Assignment may possibly lead to a collection of contradictory values. All cases of properties in this model that are also described indirectly through a subclass of E13 Attribute Assignment are characterised as "short cuts" of a path via this subclass. This redundant modelling of two alternative views is preferred because many implementations may have good reasons to model either the action of assertion or the short cut, and the relation between both alternatives can be captured by simple rules.</rdfs:comment>
    <rdfs:label xml:lang="en">Attribute Assignment</rdfs:label>
  </rdfs:Class>
  <rdfs:Class rdf:about="http://www.cidoc-crm.org/cidoc-crm/E18_Physical_Thing">
    <skos:notation rdf:datatype="http://www.w3.org/2001/XMLSchema#string">E18</skos:notation>
    <rdfs:comment xml:lang="en" rdf:datatype="http://www.w3.org/2001/XMLSchema#string">This class comprises all persistent physical items with a relatively stable form, human-made or natural.Depending on the existence of natural boundaries of such things, the CIDOC CRM distinguishes the instances of E19 Physical Object from instances of E26 Physical Feature, such as holes, rivers, pieces of land etc. Most instances of E19 Physical Object can be moved (if not too heavy), whereas features are integral to the surrounding matter.An instance of E18 Physical Thing occupies not only a particular geometric space at any instant of its existence, but in the course of its existence it also forms a trajectory through spacetime, which occupies a real, that is phenomenal, volume in spacetime. We include in the occupied space the space filled by the matter of the physical thing and all its inner spaces, such as the interior of a box. For the purpose of more detailed descriptions of the presence of an instance of E18 Physical Thing in space and time it can be associated with its specific instance of E92 Spacetime Volume by the property P196 defines (is defined by). The CIDOC CRM is generally not concerned with amounts of matter in fluid or gaseous states, as long as they are not confined in an identifiable way for an identifiable minimal time-span.</rdfs:comment>
    <rdfs:label xml:lang="en">Physical Thing</rdfs:label>
  </rdfs:Class>
  <rdfs:Class rdf:about="http://www.cidoc-crm.org/cidoc-crm/E21_Person">
    <skos:notation rdf:datatype="http://www.w3.org/2001/XMLSchema#string">E21</skos:notation>
    <rdfs:comment xml:lang="en" rdf:datatype="http://www.w3.org/2001/XMLSchema#string">This class comprises real persons who live or are assumed to have lived. Legendary figures that may have existed, such as Ulysses and King Arthur, fall into this class if the documentation refers to them as historical figures. In cases where doubt exists as to whether several persons are in fact identical, multiple instances can be created and linked to indicate their relationship. The CIDOC CRM does not propose a specific form to support reasoning about possible identity.In a bibliographic context, a name presented following the conventions usually employed for personal names will be assumed to correspond to an actual real person (an instance of E21 Person), unless evidence is available to indicate that this is not the case. The fact that a persona may erroneously be classified as an instance of E21 Person does not imply that the concept comprises personae. </rdfs:comment>
    <rdfs:label xml:lang="en">Person</rdfs:label>
  </rdfs:Class>
  <rdfs:Class rdf:about="http://www.cidoc-crm.org/cidoc-crm/E28_Conceptual_Object">
    <skos:notation rdf:datatype="http://www.w3.org/2001/XMLSchema#string">E28</skos:notation>
    <rdfs:comment xml:lang="en" rdf:datatype="http://www.w3.org/2001/XMLSchema#string">This class comprises non-material products of our minds and other human produced data that have become objects of a discourse about their identity, circumstances of creation or historical implication. The production of such information may have been supported by the use of technical devices such as cameras or computers.Characteristically, instances of this class are created, invented or thought by someone, and then may be documented or communicated between persons. Instances of E28 Conceptual Object have the ability to exist on more than one particular carrier at the same time, such as paper, electronic signals, marks, audio media, paintings, photos, human memories, etc.They cannot be destroyed. They exist as long as they can be found on at least one carrier or in at least one human memory. Their existence ends when the last carrier and the last memory are lost. </rdfs:comment>
    <rdfs:label xml:lang="en">Conceptual Object</rdfs:label>
  </rdfs:Class>
  <rdfs:Class rdf:about="http://www.cidoc-crm.org/cidoc-crm/E29_Design_or_Procedure">
    <skos:notation rdf:datatype="http://www.w3.org/2001/XMLSchema#string">E29</skos:notation>
    <rdfs:comment xml:lang="en" rdf:datatype="http://www.w3.org/2001/XMLSchema#string">This class comprises documented plans for the execution of actions in order to achieve a result of a specific quality, form or contents. In particular, it comprises plans for deliberate human activities that may result in new instances of E71 Human-Made Thing or for shaping or guiding the execution of an instance of E7 Activity.Instances of E29 Design or Procedure can be structured in parts and sequences or depend on others.This is modelled using P69 has association with (is associated with): E29 Design or Procedure.Designs or procedures can be seen as one of the followingA schema for the activities it describesA schema of the products that result from their application.An independent intellectual product that may have never been applied, such as Leonardo da Vinci’s famous plans for flying machines.Because designs or procedures may never be applied or only partially executed, the CIDOC CRM models a loose relationship between the plan and the respective product.</rdfs:comment>
    <rdfs:label xml:lang="en">Design or Procedure</rdfs:label>
  </rdfs:Class>
  <rdfs:Class rdf:about="http://www.cidoc-crm.org/cidoc-crm/E39_Actor">
    <skos:notation rdf:datatype="http://www.w3.org/2001/XMLSchema#string">E39</skos:notation>
    <rdfs:comment xml:lang="en" rdf:datatype="http://www.w3.org/2001/XMLSchema#string">This class comprises people, either individually or in groups, who have the potential to perform intentional actions of kinds for which someone may be held responsible. </rdfs:comment>
    <rdfs:label xml:lang="en">Actor</rdfs:label>
  </rdfs:Class>
  <rdfs:Class rdf:about="http://www.cidoc-crm.org/cidoc-crm/E41_Appellation">
    <skos:notation rdf:datatype="http://www.w3.org/2001/XMLSchema#string">E41</skos:notation>
    <rdfs:comment xml:lang="en" rdf:datatype="http://www.w3.org/2001/XMLSchema#string">This class comprises signs, either meaningful or not, or arrangements of signs following a specific syntax, that are used or can be used to refer to and identify a specific instance of some class or category within a certain context.Instances of E41 Appellation do not identify things by their meaning, even if they happen to have one, but instead by convention, tradition, or agreement. Instances of E41 Appellation are cultural constructs; as such, they have a context, a history, and a use in time and space by some group of users. A given instance of E41 Appellation can have alternative forms, i.e., other instances of E41 Appellation that are always regarded as equivalent independent from the thing it denotes.Different languages may use different appellations for the same thing, such as the names of major cities. Some appellations may be formulated using a valid noun phrase of a particular language. In these cases, the respective instances of E41 Appellation should also be declared as instances of E33 Linguistic Object. Then the language using the appellation can be declared with the property P72 has language: E56 Language.Instances of E41 Appellation may be used to identify any instance of E1 CRM Entity and sometimes are characteristic for instances of more specific subclasses E1 CRM Entity, such as for instances of E52 Time-Span (for instance “dates”), E39 Actor, E53 Place or E28 Conceptual Object. Postal addresses and E-mail addresses are characteristic examples of identifiers used by services transporting things between clients.Even numerically expressed identifiers for extents in space or time are also regarded as instances of E41 Appellation, such as Gregorian dates or spatial coordinates, even though they allow for determining some time or location by a known procedure starting from a reference point and by virtue of that fact play a double role as instances of E59 Primitive Value.E41 Appellation should not be confused with the act of naming something. Cf. E15 Identifier Assignment</rdfs:comment>
    <rdfs:label xml:lang="en">Appellation</rdfs:label>
  </rdfs:Class>
  <rdfs:Class rdf:about="http://www.cidoc-crm.org/cidoc-crm/E42_Identifier">
    <skos:notation rdf:datatype="http://www.w3.org/2001/XMLSchema#string">E42</skos:notation>
    <rdfs:comment xml:lang="en" rdf:datatype="http://www.w3.org/2001/XMLSchema#string">This class comprises strings or codes assigned to instances of E1 CRM Entity in order to identify them uniquely and permanently within the context of one or more organisations. Such codes are often known as inventory numbers, registration codes, etc. and are typically composed of alphanumeric sequences. Postal addresses, telephone numbers, URLs and e-mail addresses are characteristic examples of identifiers used by services transporting things between clients.The class E42 Identifier is not normally used for machine-generated identifiers used for automated processing unless these are also used by human agents. </rdfs:comment>
    <rdfs:label xml:lang="en">Identifier</rdfs:label>
  </rdfs:Class>
  <rdfs:Class rdf:about="http://www.cidoc-crm.org/cidoc-crm/E53_Place">
    <skos:notation rdf:datatype="http://www.w3.org/2001/XMLSchema#string">E53</skos:notation>
    <rdfs:comment xml:lang="en" rdf:datatype="http://www.w3.org/2001/XMLSchema#string">This class comprises extents in the natural space we live in, in particular on the surface of the Earth, in the pure sense of physics: independent from temporal phenomena and matter. They may serve describing the physical location of things or phenomena or other areas of interest. Geometrically, instances of E53 Place constitute single contiguous areas or a finite aggregation of disjoint areas in space which are each individually contiguous. They may have fuzzy boundaries. The instances of E53 Place are usually determined by reference to the position of “immobile” objects such as buildings, cities, mountains, rivers, or dedicated geodetic marks, but may also be determined by reference to mobile objects. A Place can be determined by combining a frame of reference and a location with respect to this frame. It is sometimes argued that instances of E53 Place are best identified by global coordinates or absolute reference systems. However, relative references are often more relevant in the context of cultural documentation and tend to be more precise. In particular, we are often interested in position in relation to large, mobile objects, such as ships. For example, the Place at which Nelson died is known with reference to a large mobile object – H.M.S Victory. A resolution of this Place in terms of absolute coordinates would require knowledge of the movements of the vessel and the precise time of death, either of which may be revised, and the result would lack historical and cultural relevance.Any instance of E18 Physical Thing can serve as a frame of reference for an instance of E53 Place. This may be documented using the property P157 is at rest relative to (provides reference space for). </rdfs:comment>
    <rdfs:label xml:lang="en">Place</rdfs:label>
  </rdfs:Class>
  <rdfs:Class rdf:about="http://www.cidoc-crm.org/cidoc-crm/E54_Dimension">
    <skos:notation rdf:datatype="http://www.w3.org/2001/XMLSchema#string">E54</skos:notation>
    <rdfs:comment xml:lang="en" rdf:datatype="http://www.w3.org/2001/XMLSchema#string">This class comprises quantifiable properties that can be measured by some calibrated means and can be approximated by values, i.e., by points or regions in a mathematical or conceptual space, such as natural or real numbers, RGB values etc.An instance of E54 Dimension represents the empirical or theoretically derived quantity, including the precision tolerances resulting from the particular method or calculation. The identity of an instance of E54 Dimension depends on the method of its determination because each method may produce different values even when determining comparable qualities. For instance, the wingspan of a bird alive or dead is a different dimension. Thermoluninescence dating and Rehydroxylation [RHX] dating are different dimensions of temporal distance from now, even if they aim at dating the same object. The method of determination should be expressed using the property P2 has type (is type of). Note that simple terms such as “diameter” or “length” are normally insufficient to unambiguously describe a respective dimension. In contrast, “maximum linear extent” may be sufficient.The properties of the class E54 Dimension allow for expressing the numerical approximation of the values of instances of E54 Dimension adequate to the precision of the applied method of determination. If the respective quantity belongs to a non-discrete space according to the laws of physics, such as spatial distances, it is recommended to record them as approximations by intervals or regions of indeterminacy enclosing the assumed true values. For instance, a length of 5 cm may be recorded as 4.5-5.5 cm, according to the precision of the respective observation. Note, that comparability of values described in different units depends critically on the representation as value regions.Numerical approximations in archaic instances of E58 Measurement Unit used in historical records should be preserved. Equivalents corresponding to current knowledge should be recorded as additional instances of E54 Dimension, as appropriate.</rdfs:comment>
    <rdfs:label xml:lang="en">Dimension</rdfs:label>
  </rdfs:Class>
  <rdfs:Class rdf:about="http://www.cidoc-crm.org/cidoc-crm/E55_Type">
    <skos:notation rdf:datatype="http://www.w3.org/2001/XMLSchema#string">E55</skos:notation>
    <rdfs:comment xml:lang="en" rdf:datatype="http://www.w3.org/2001/XMLSchema#string">This class comprises concepts denoted by terms from thesauri and controlled vocabularies used to characterize and classify instances of CIDOC CRM classes. Instances of E55 Type represent concepts in contrast to instances of E41 Appellation which are used to name instances of CIDOC CRM classes. E55 Type is the CIDOC CRM’s interface to domain specific ontologies and thesauri. These can be represented in the CIDOC CRM as subclasses of E55 Type, forming hierarchies of terms, i.e., instances of E55 Type linked via P127 has broader term (has narrower term): E55 Type. Such hierarchies may be extended with additional properties. </rdfs:comment>
    <rdfs:label xml:lang="en">Type</rdfs:label>
  </rdfs:Class>
  <rdfs:Class rdf:about="http://www.cidoc-crm.org/cidoc-crm/E66_Formation">
    <skos:notation rdf:datatype="http://www.w3.org/2001/XMLSchema#string">E66</skos:notation>
    <rdfs:comment xml:lang="en" rdf:datatype="http://www.w3.org/2001/XMLSchema#string">This class comprises events that result in the formation of a formal or informal E74 Group of people, such as a club, society, association, corporation or nation. E66 Formation does not include the arbitrary aggregation of people who do not act as a collective.The formation of an instance of E74 Group does not require that the group is populated with members at the time of formation. In order to express the joining of members at the time of formation, the respective activity should be simultaneously an instance of both E66 Formation and E85 Joining. </rdfs:comment>
    <rdfs:label xml:lang="en">Formation</rdfs:label>
  </rdfs:Class>
  <rdfs:Class rdf:about="http://www.cidoc-crm.org/cidoc-crm/E68_Dissolution">
    <skos:notation rdf:datatype="http://www.w3.org/2001/XMLSchema#string">E68</skos:notation>
    <rdfs:comment xml:lang="en" rdf:datatype="http://www.w3.org/2001/XMLSchema#string">This class comprises the events that result in the formal or informal termination of an instance of E74 Group. If the dissolution was deliberate, the Dissolution event should also be instantiated as an instance of E7 Activity.</rdfs:comment>
    <rdfs:label xml:lang="en">Dissolution</rdfs:label>
  </rdfs:Class>
  <rdfs:Class rdf:about="http://www.cidoc-crm.org/cidoc-crm/E70_Thing">
    <skos:notation rdf:datatype="http://www.w3.org/2001/XMLSchema#string">E70</skos:notation>
    <rdfs:comment xml:lang="en" rdf:datatype="http://www.w3.org/2001/XMLSchema#string">This general class comprises discrete, identifiable, instances of E77 Persistent Item that are documented as single units, that either consist of matter or depend on being carried by matter and are characterized by relative stability. They may be intellectual products or physical things. They may for instance have a solid physical form, an electronic encoding, or they may be a logical concept or structure.</rdfs:comment>
    <rdfs:label xml:lang="en">Thing</rdfs:label>
  </rdfs:Class>
  <rdfs:Class rdf:about="http://www.cidoc-crm.org/cidoc-crm/E72_Legal_Object">
    <skos:notation rdf:datatype="http://www.w3.org/2001/XMLSchema#string">E72</skos:notation>
    <rdfs:comment xml:lang="en" rdf:datatype="http://www.w3.org/2001/XMLSchema#string">This class comprises those material or immaterial items to which instances of E30 Right, such as the right of ownership or use, can be applied. This is true for all instances of E18 Physical Thing. In the case of instances of E28 Conceptual Object, however, the identity of an instance of E28 Conceptual Object or the method of its use may be too ambiguous to reliably establish instances of E30 Right, as in the case of taxa and inspirations. Ownership of corporations is currently regarded as out of scope of the CIDOC CRM. </rdfs:comment>
    <rdfs:label xml:lang="en">Legal Object</rdfs:label>
  </rdfs:Class>
  <rdfs:Class rdf:about="http://www.cidoc-crm.org/cidoc-crm/E73_Information_Object">
    <skos:notation rdf:datatype="http://www.w3.org/2001/XMLSchema#string">E73</skos:notation>
    <rdfs:comment xml:lang="en" rdf:datatype="http://www.w3.org/2001/XMLSchema#string">This class comprises identifiable immaterial items, such as poems, jokes, data sets, images, texts, multimedia objects, procedural prescriptions, computer program code, algorithm or mathematical formulae, that have an objectively recognizable structure and are documented as single units. The encoding structure known as a "named graph" also falls under this class, so that each "named graph" is an instance of E73 Information Object.An instance of E73 Information Object does not depend on a specific physical carrier, which can include human memory, and it can exist on one or more carriers simultaneously.Instances of E73 Information Object of a linguistic nature should be declared as instances of the E33 Linguistic Object subclass. Instances of E73 Information Object of a documentary nature should be declared as instances of the E31 Document subclass. Conceptual items such as types and classes are not instances of E73 Information Object, nor are ideas without a reproducible expression.</rdfs:comment>
    <rdfs:label xml:lang="en">Information Object</rdfs:label>
  </rdfs:Class>
  <rdfs:Class rdf:about="http://www.cidoc-crm.org/cidoc-crm/E74_Group">
    <skos:notation rdf:datatype="http://www.w3.org/2001/XMLSchema#string">E74</skos:notation>
    <rdfs:comment xml:lang="en" rdf:datatype="http://www.w3.org/2001/XMLSchema#string">This class comprises any gatherings or organizations of human individuals or groups that act collectively or in a similar way due to any form of unifying relationship. In the wider sense this class also comprises official positions which used to be regarded in certain contexts as one actor, independent of the current holder of the office, such as the president of a country. In such cases, it may happen that the group never had more than one member. A joint pseudonym (i.e., a name that seems indicative of an individual but that is actually used as a persona by two or more people) is a particular case of E74 Group.A gathering of people becomes an instance of E74 Group when it exhibits organizational characteristics usually typified by a set of ideas or beliefs held in common, or actions performed together. These might be communication, creating some common artifact, a common purpose such as study, worship, business, sports, etc. Nationality can be modelled as membership in an instance of E74 Group. Married couples and other concepts of family are regarded as particular examples of E74 Group.</rdfs:comment>
    <rdfs:label xml:lang="en">Group</rdfs:label>
  </rdfs:Class>
  <rdfs:Class rdf:about="http://www.cidoc-crm.org/cidoc-crm/E77_Persistent_Item">
    <skos:notation rdf:datatype="http://www.w3.org/2001/XMLSchema#string">E77</skos:notation>
    <rdfs:comment xml:lang="en" rdf:datatype="http://www.w3.org/2001/XMLSchema#string">This class comprises items that have persistent characteristics of structural nature substantially related to their identity and their integrity, sometimes known as “endurants” in philosophy. Persistent Items may be physical entities, such as people, animals or things, conceptual entities such as ideas, concepts, products of the imagination or even names. Instances of E77 Persistent Item may be present or be part of interactions in different periods or events. They can repeatedly be recognized at disparate occasions during their existence by characteristics of structural nature. The respective characteristics need not be exactly the same during all the existence of an instance of E77 Persistent Item. Often, they undergo gradual change, still bearing some similarities with that of previous times, or disappear completely and new emerge. For instance, a person, from the time of being born on, will gradually change all its features and acquire new ones, such as a scar. Even the DNA in different body cells will develop defects and mutations. Nevertheless, relevant characteristics used should be sufficiently similar to recognize the instance for some substantial period of time. The more specific criteria that determine the identity of instances of subclasses of E77 Persistent Item may vary considerably and are described or referred to in the respective scope notes. The decision about which exact criteria to use depends on whether the observable behaviour of the respective part of reality such confined conforms to the reasoning the user is interested in. For example, a building can be regarded as no longer existing if it is dismantled and the materials reused in a different configuration. On the other hand, human beings go through radical and profound changes during their life-span, affecting both material composition and form, yet preserve their identity by other criteria, such as being bodily separated from other persons. Similarly, inanimate objects may be subject to exchange of parts and matter. On the opposite, the identity of a (version of a) text of a scientific publication is given by the exact arrangement of its relevant symbols. The main classes of objects that fall outside the scope of the E77 Persistent Item class are temporal objects such as periods, events and acts, and descriptive properties. An instance of E77 Persistent Item does not require actual knowledge of the identifying features of the instance being currently known. There may be cases, where the actual identifying features of an instance of E77 Persistent Item are not decidable at a particular state of knowledge. </rdfs:comment>
    <rdfs:label xml:lang="en">Persistent Item</rdfs:label>
  </rdfs:Class>
  <rdfs:Class rdf:about="http://www.cidoc-crm.org/cidoc-crm/E85_Joining">
    <skos:notation rdf:datatype="http://www.w3.org/2001/XMLSchema#string">E85</skos:notation>
    <rdfs:comment xml:lang="en" rdf:datatype="http://www.w3.org/2001/XMLSchema#string">This class comprises the activities that result in an instance of E39 Actor becoming a member of an instance of E74 Group. This class does not imply initiative by either party. It may be the initiative of a third party.Typical scenarios include becoming a member of a social organisation, becoming employee of a company, marriage, the adoption of a child by a family and the inauguration of somebody into an official position. </rdfs:comment>
    <rdfs:label xml:lang="en">Joining</rdfs:label>
  </rdfs:Class>
  <rdfs:Class rdf:about="http://www.cidoc-crm.org/cidoc-crm/E86_Leaving">
    <skos:notation rdf:datatype="http://www.w3.org/2001/XMLSchema#string">E86</skos:notation>
    <rdfs:comment xml:lang="en" rdf:datatype="http://www.w3.org/2001/XMLSchema#string">This class comprises the activities that result in an instance of E39 Actor to be disassociated from an instance of E74 Group. This class does not imply initiative by either party. It may be the initiative of a third party.Typical scenarios include the termination of membership in a social organisation, ending the employment at a company, divorce, and the end of tenure of somebody in an official position.</rdfs:comment>
    <rdfs:label xml:lang="en">Leaving</rdfs:label>
  </rdfs:Class>
  <rdfs:Class rdf:about="http://www.cidoc-crm.org/cidoc-crm/E89_Propositional_Object">
    <skos:notation rdf:datatype="http://www.w3.org/2001/XMLSchema#string">E89</skos:notation>
    <rdfs:comment xml:lang="en" rdf:datatype="http://www.w3.org/2001/XMLSchema#string">This class comprises immaterial items, including but not limited to stories, plots, procedural prescriptions, algorithms, laws of physics or images that are, or represent in some sense, sets of propositions about real or imaginary things and that are documented as single units or serve as topic of discourse. This class also comprises items that are “about” something in the sense of a subject. In the wider sense, this class includes expressions of psychological value such as non-figural art and musical themes. However, conceptual items such as types and classes are not instances of E89 Propositional Object. This should not be confused with the definition of a type, which is indeed an instance of E89 Propositional Object.</rdfs:comment>
    <rdfs:label xml:lang="en">Propositional Object</rdfs:label>
  </rdfs:Class>
  <rdfs:Class rdf:about="http://iflastandards.info/ns/lrm/lrmoo/F2">
    <skos:notation rdf:datatype="http://www.w3.org/2001/XMLSchema#string">F2</skos:notation>
    <rdfs:comment xml:lang="en" rdf:datatype="http://www.w3.org/2001/XMLSchema#string">This class comprises the intellectual or artistic realisations of Works in the form of identifiable immaterial objects, such as texts, poems, jokes, musical or choreographic notations, movement pattern, sound pattern, images, multimedia objects, or any combination of such forms. The substance of F2 Expression is signs.An Expression is the outcome of the intellectual or creative process of realizing a Work. Subsequent expressions conveying the same work may be created over time.Expressions do not depend on a specific physical carrier and can exist on one or more carriers simultaneously. As far as bibliographic practice is concerned, only instances of F2 Expression that are externalised on physical carriers other than both the creator’s brain and an auditor’s brain are taken into account.The form of F2 Expression is an inherent characteristic of the F2 Expression. Differences in form imply different Expressions (e.g., from text to spoken word, a transcript of a recording). Similarly, differences in language or means of performance imply different Expressions (e.g., translations or arrangements for different instruments). Thus, if a text is revised or modified, the result is considered to be a new F2 Expression. While theoretically any change in signs will result in a new Expression, conventionally the context and use will determine the rules for distinguishing among expressions.An instance of F2 Expression which includes spoken or written text may be multiply instantiated as an instance of E33 Linguistic Object. This allows for the association of the E56 Language of the text with the instance of F2 Expression by using the property P72 has language (is language of).</rdfs:comment>
    <rdfs:label xml:lang="en">Expression</rdfs:label>
  </rdfs:Class>
  <rdfs:Class rdf:about="http://iflastandards.info/ns/lrm/lrmoo/F28">
    <skos:notation rdf:datatype="http://www.w3.org/2001/XMLSchema#string">F28</skos:notation>
    <rdfs:comment xml:lang="en" rdf:datatype="http://www.w3.org/2001/XMLSchema#string">This class comprises activities that result in instances of F2 Expression coming into existence. An instance of F2 Expression is considered to be created when it is captured on a carrier other than the creator’s brain.Although F2 Expression is an abstract entity, a conceptual object, the creation of an expression inevitably also affects the physical world: when you scribble the first draft of a poem on a sheet of paper, you produce an instance of F3 Manifestation and an instance of F5 Item. F28 Expression Creation is a subclass of E12 Production because the recording of the expression causes a physical modification of the E18 Physical Thing that serves as the carrier. The creation of an instance of F2 Expression coincides with the creation of the first instance of F3 Manifestation that R4 embodies (is embodied in) this instance of F2 Expression.The P2 has type (is type of) property can be used to specify the type of the instance of F28 Expression Creation (i.e., activities such as translating, revising, or arranging music are types of creation process). The type of the process is distinct from the type of result even though the typology frequently used for instances of the resulting F2 Expressions may imply the category of the instance of the F28 Expression Creation.An instance of F28 Expression Creation may use as source material one or more specific instances of F2 Expression. When the source expression is documented this is also expressed by the property R76 is derivative of (has derivative).</rdfs:comment>
    <rdfs:label xml:lang="en">Expression Creation</rdfs:label>
  </rdfs:Class>
  <rdfs:Class rdf:about="http://www.cidoc-crm.org/extensions/crminf/I1_Argumentation">
    <skos:notation rdf:datatype="http://www.w3.org/2001/XMLSchema#string">I1</skos:notation>
    <rdfs:comment xml:lang="en" rdf:datatype="http://www.w3.org/2001/XMLSchema#string">This class comprises the activity of making honest inferences or observations. An honest inference or observation is one in which the E39 Actor carrying out the I1 Argumentation justifies and believes that the I6 Belief Value associated with the resulting I2 Belief about the I4 Proposition Set is the correct value at the time that the activity was undertaken and that any I3 Inference Logic or methodology was correctly applied.
One instance of E39 Actor may carry out an instance of I1 Argumentation, though the E39 Actor may, of course, be an instance of E74 Group.</rdfs:comment>
    <rdfs:label xml:lang="en">Argumentation</rdfs:label>
  </rdfs:Class>
  <rdfs:Class rdf:about="http://www.cidoc-crm.org/extensions/crmtex/TX4_Writing_Field">
    <skos:notation rdf:datatype="http://www.w3.org/2001/XMLSchema#string">TX4</skos:notation>
    <rdfs:comment xml:lang="en" rdf:datatype="http://www.w3.org/2001/XMLSchema#string">This class describes the portion of the physical carrier
          arranged and usually reserved and delimited for the purpose of accommodating a written
          text, highlighting and isolating it from the other parts of the object to which it
          belongs, enhancing and guaranteeing its readability. This entity is paramount specially in
          epigraphy, in which a specific element called “epigraphic field” has been defined by the
          discipline itself. Its importance is also evident in papyrology and codicology, where a
          clear distinction between area(s) containing the written text and empty parts of the
          support (margins, intercolumnia, etc.) is significant for the
          definition of styles and periods of the document.</rdfs:comment>
    <rdfs:label xml:lang="en">Writing Field</rdfs:label>
  </rdfs:Class>
  <rdfs:Class rdf:about="http://www.cidoc-crm.org/extensions/crmtex/TX5_Text_Recognition">
    <skos:notation rdf:datatype="http://www.w3.org/2001/XMLSchema#string">TX5</skos:notation>
    <rdfs:comment xml:lang="en" rdf:datatype="http://www.w3.org/2001/XMLSchema#string">This class comprises activities of recognizing physical
          features on some surface, often an instance of TX4 Writing Field, as an arrangement of a
          series of identifiable glyphs of some known script, deciphered or not, in an order
          characteristic for a text.For study purposes, the text recognition
          procedure requires a scientific autoptic examination of the text. An autoptic examination
          consists of an accurate analysis of the surface and the signs, and prescribes the use of
          specific tools and procedures for establishing the exact value of each sign on the
          physical feature. Deterioration of the original medium or “sloppy” writing may render
          parts of the original text as undecipherable or ambiguous, which may be annotated in the
          transcript following epigraphic standards; a text recognition typically results in a
          record of an equivalent sequence of graphemes on another persistent medium in a scholarly
          established form of representation of the respective graphemes, often called a
          “transcript”.An instance of TX5 Text Recognition may in particular
          apply even to a single glyph, typically forming part of an instance of TX5 Text
          Recognition applying to a larger sequence of glyphs containing the former
          glyph.The recognition process may be assisted by mechanical means,
          imaging technology, or a traditional squeeze for incised glyphs. In case the recognition
          process is solely based on the latter, the observation concerns only the representations
          on the latter as present to the researcher in some physical form or projection and should
          unambiguously be documented as such.In case the
          recognized text has not been documented in a transcript, text recognition may constitute
          an implicit part of an overarching reading process, instance of TX14 Reading, which has
          resulted in other noteworthy propositions related to the content of the recognized text.
          On the other side, recognition of single glyphs or contracted parts of texts, as they are
          characteristic for the use of ligatured scripts, may quite well be implicitly supported by
          the reader’s comprehension of the text and the creator of the transcript may have chosen
          not to annotate parts that the reader regarded as unambiguous. Since these cases can often
          hardly be separated from the shape recognition of the glyphs in isolation, documenting
          such implicit comprehension as a separate process may not be relevant. It is however
          regarded as good practice to document explicitly the reading process and associated
          interpretative reasoning for any non-trivial resolution of ambiguity or gaps in the
          recognized text that has a bearing on the transcript or further completion of the
          transcript.</rdfs:comment>
    <rdfs:label xml:lang="en">Text Recognition</rdfs:label>
  </rdfs:Class>
  <rdfs:Class rdf:about="https://ontology.swissartresearch.net/aaao/ZE1_Institutional_Fact">
    <skos:notation rdf:datatype="http://www.w3.org/2001/XMLSchema#string">ZE1</skos:notation>
    <rdfs:comment xml:lang="en" rdf:datatype="http://www.w3.org/2001/XMLSchema#string">An instance of institutional fact is an ascription of a status function to an object by a community. The institutional fact is a concretization of a collective intentionality of the community in question towards a certain object over a certain period of time.
An instance of institutional fact is recognizable to a competent speaker/member of a symbolic community (native or learner with sufficient competence). It may not be perceived through a single sense impression but through multiple experiences and implicit reasonings (e.g.: embedded participation, behavioural observation, linguistic evidence and interview), yet typically such intermediate observations and inferences are not necessarily recorded or accessible. The historical statement is typically the assertion of the institutional fact, that such and such a fact was the case, and was in force for a given community, at some time. The epistemic veridicality of the stated /reference instance of institutional fact is always open to contestation. The means of contestation involve analyzing the sources which support it.
Instances of institutional fact come into existence based on conventions establishing the conditions under which they come into effect. Typically, an instance of institutional fact will come into existence either because of the performance of its stipulated, initiating speech act (e.g.: state of being married via marriage) or as a result of events fulfilling existing norm prescriptions in the community (e.g.: state of being uncle as result of birth of child of sister).  An institutional fact comes to be through the agreed fiat of a community. It typically ceases to exist either because of a stipulated, nullifying speech act (e.g. divorce proceeding), because a community ceases to support the effective rule supporting its declaration (e.g.: ownership of people) or force majeure (e.g.: object ascribed function/status or community perceiving status is eliminated).</rdfs:comment>
    <rdfs:label xml:lang="en">Institutional Fact</rdfs:label>
    <rdfs:subClassOf rdf:resource="http://www.cidoc-crm.org/cidoc-crm/E2_Temporal_Entity"/>
  </rdfs:Class>
  <rdfs:Class rdf:about="https://ontology.swissartresearch.net/aaao/ZE2_Appellative_Status">
    <skos:notation rdf:datatype="http://www.w3.org/2001/XMLSchema#string">ZE2</skos:notation>
    <rdfs:comment xml:lang="en" rdf:datatype="http://www.w3.org/2001/XMLSchema#string">An instance of appellative status is the collective ascription of an appellation to an object by a community. The substance of the appellative status is the communal commitment to the naming of the object in question with a designated appellation, under a designated modality.
Instances of appellative status are recognizable through evidence of community members adopting the intentional stance of so-naming towards the object in question, as observable from direct witnesses, through the reports of competent observers or through evidence of a declarative act [e.g.: ZE19 Naming] initiating this status. Examples of such evidence include, several individuals so naming a thing, a witness declaring that a thing is ‘so named, by us’ or through documents reporting this fact.
Instances of appellative status may come to be through a formal process such as a declarative act of naming, or may have arisen through habit, fiat or be of unknown origin. Instances of appellative status may end either through a formal process, such as a new declarative act of naming, the formal stripping of a name, or may simply fade out of use, be eliminated by fiat or be of unknown reason. </rdfs:comment>
    <rdfs:label xml:lang="en">Appellative Status</rdfs:label>
    <rdfs:subClassOf rdf:resource="https://ontology.swissartresearch.net/aaao/ZE1_Institutional_Fact"/>
  </rdfs:Class>
  <rdfs:Class rdf:about="https://ontology.swissartresearch.net/aaao/ZE3_Contact_Point_Status">
    <skos:notation rdf:datatype="http://www.w3.org/2001/XMLSchema#string">ZE3</skos:notation>
    <rdfs:comment xml:lang="en" rdf:datatype="http://www.w3.org/2001/XMLSchema#string">An instance of contact status is the collective ascription of a contact point to an actor by a community. The substance of the contact status is the communal commitment to the addressing of messages to the actor in question according to a designated contact point appellation, using the implied message exchanging method.
Instances of contact status are recognizable through evidence of community members adopting the intentional stance of so-addressing messages to the actor in question, as observable from direct witnesses, through the reports of competent observers or through evidence of a declarative act [e.g.: E15 Identifier Assignment] initiating this status. Examples of such evidence include, several individuals so addressing messages to an actor via this contact point appellation, a witness declaring that an actor can so be reached, or through documents reporting this fact.
Instances of contact status may come to be through a formal process such as a declarative act of identifier assignment, or may have arisen through habit, fiat or be of unknown origin. Instances of contact status may end either though a formal process, such as a new declarative act of identifier assignment, through formal assignment, or may simply fade out of use, be eliminated by fiat or for unknown reasons. </rdfs:comment>
    <rdfs:label xml:lang="en">Contact Point Status</rdfs:label>
    <rdfs:subClassOf rdf:resource="https://ontology.swissartresearch.net/aaao/ZE2_Appellative_Status"/>
  </rdfs:Class>
  <rdfs:Class rdf:about="https://ontology.swissartresearch.net/aaao/ZE4_Classificatory_Status">
    <skos:notation rdf:datatype="http://www.w3.org/2001/XMLSchema#string">ZE4</skos:notation>
    <rdfs:comment xml:lang="en" rdf:datatype="http://www.w3.org/2001/XMLSchema#string">An instance of classificatory status is the collective ascription of a type to an object by a community. The substance of the classificatory status is the communal commitment to the classification of the object in question according to the designated type.
Instances of classificatory status are recognizable through evidence of community members adopting the intentional stance of so-classifying the object in question, as observable from direct witnesses, through the reports of competent observers or through evidence of a declarative act [e.g.: E17 Type Assignment] initiating this status.
Instances of classificatory status may come to be through a formal process such as a declarative act of classification [E17 Type Assignment], or may have arisen through habit, fiat or be of unknown origin. Instances of classificatory status may end either though a formal process, such as a new declarative act of classification, be officially declassified, or may simply fade out of use, be eliminated by fiat or be of unknown reason. </rdfs:comment>
    <rdfs:label xml:lang="en">Classificatory Status</rdfs:label>
    <rdfs:subClassOf rdf:resource="https://ontology.swissartresearch.net/aaao/ZE1_Institutional_Fact"/>
  </rdfs:Class>
  <rdfs:Class rdf:about="https://ontology.swissartresearch.net/aaao/ZE5_Function_Status">
    <skos:notation rdf:datatype="http://www.w3.org/2001/XMLSchema#string">ZE5</skos:notation>
    <rdfs:comment xml:lang="en" rdf:datatype="http://www.w3.org/2001/XMLSchema#string">An instance of function status is the collective ascription of an operative functionality to an object by a community. The substance of the function status is the communal commitment to relating to and / or using the object in question according to a designated function.
Instances of function status are recognizable through evidence of community members adopting the intentional stance of so using or relating to the object in question, as observable from direct witnesses, through the reports of competent observers or through evidence of a declarative act [e.g.: E17 Type Assignment] initiating this status.
Instances of function status may come to be through a formal process such as a declarative act of classification [E17 type Assignment], or may have arisen through habit, fiat or be of unknown origin. Instances of function status may end either though a formal process, such as a new declarative act of classification, or may simply fade out of use, be eliminated by fiat or by unknown reason.</rdfs:comment>
    <rdfs:label xml:lang="en">Function Status</rdfs:label>
    <rdfs:subClassOf rdf:resource="https://ontology.swissartresearch.net/aaao/ZE4_Classificatory_Status"/>
  </rdfs:Class>
  <rdfs:Class rdf:about="https://ontology.swissartresearch.net/aaao/ZE6_Social_Status">
    <skos:notation rdf:datatype="http://www.w3.org/2001/XMLSchema#string">ZE6</skos:notation>
    <rdfs:comment xml:lang="en" rdf:datatype="http://www.w3.org/2001/XMLSchema#string">An instance of social status is the collective ascription of a social function to an actor by a community. The substance of the social status is the communal commitment to relating to and acting toward the actor in question according to the designated status.
It is important to underline that an instance of social status relates to a classification of an individual as holding a particular role or function in the community in general. This is to be distinguished from a social relation status, a binary construct that binds two different actors in a certain relation. For example, an instance of social status could be the social status of "Coach". This social status, if ascribed to an individual, holds for that person within a general social context and for a particular group and/or population. This is distinct from a social relation status that is recognized particularly between the two individuals concerned, such as "coach of", that would particularly hold between the individual who is coach and the individual who is a team member.
Instances of social status are recognizable through evidence of community members adopting the intentional stance of so relating or acting toward the actor in question, as observable from direct witnesses, through the reports of competent observers or through evidence of a declarative act [e.g.: E17 Type Assignment] initiating this status.
Instances of social status may be attributed to individuals or to groups of individuals. Instances of social status may also be held in relation to a third party, to whom the subject of the social status bears certain rights and/or responsibilities.
Instances of social status may come to be through a formal process such as a declarative act of assignment [E17 Type Assignment], or may have arisen through habit, fiat or be of unknown origin. Instances of social status may end either though a formal process, such as a new declarative act of classification, or may simply fade out of use, be eliminated by fiat or by unknown reason.</rdfs:comment>
    <rdfs:label xml:lang="en">Social Status</rdfs:label>
    <rdfs:subClassOf rdf:resource="https://ontology.swissartresearch.net/aaao/ZE4_Classificatory_Status"/>
  </rdfs:Class>
  <rdfs:Class rdf:about="https://ontology.swissartresearch.net/aaao/ZE7_Custodial_Status">
    <skos:notation rdf:datatype="http://www.w3.org/2001/XMLSchema#string">ZE7</skos:notation>
    <rdfs:comment xml:lang="en" rdf:datatype="http://www.w3.org/2001/XMLSchema#string">An instance of custodial status is the collective ascription of a relationship of custodianship of some actor over an object by a community. The substance of the custodial status is the communal commitment to the recognition of the relationship of custodianship over the designated object by the actor in question.
Instances of custodial status are recognizable through evidence of community members adopting the intentional stance of so recognizing this status, as observable from direct witnesses, through the reports of competent observers or through evidence of a declarative act [e.g.: ZE21 Declarative Transfer of Custody] initiating this status.
Instances of classificatory status may come to be through a formal process such as a declarative transfer of custody, or may have arisen through habit, fiat or be of unknown origin. Instances of custodial status may end either though a formal process, such as a new declarative act of legal transfer of custody, or may simply fade out of use, be eliminated by fiat or be of unknown reason. </rdfs:comment>
    <rdfs:label xml:lang="en">Custodial Status</rdfs:label>
    <rdfs:subClassOf rdf:resource="https://ontology.swissartresearch.net/aaao/ZE30_Property_Right_Status"/>
  </rdfs:Class>
  <rdfs:Class rdf:about="https://ontology.swissartresearch.net/aaao/ZE8_Ownership_Status">
    <skos:notation rdf:datatype="http://www.w3.org/2001/XMLSchema#string">ZE8</skos:notation>
    <rdfs:comment xml:lang="en" rdf:datatype="http://www.w3.org/2001/XMLSchema#string">An instance of ownership status is the collective ascription of a relationship of legal possession of some actor over a legal object by a community. The substance of the ownership status is the communal commitment to the recognition of the relationship of possession over the designated legal object by the actor in question.
Instances of ownership status are recognizable through evidence of community members adopting the intentional stance of so recognizing this status, as observable from direct witnesses, through the reports of competent observers or through evidence of a declarative act [e.g.: ZE20 Declarative Acquisition] initiating this status.
Instances of ownership status may come to be through a formal process such as a declarative act of taking ownership, or may have arisen through habit, fiat or be of unknown origin. Instances of ownership status may end either though a formal process, such as a new declarative act of acquisition, or may simply fade out of use, be eliminated by fiat or be of unknown reason.</rdfs:comment>
    <rdfs:label xml:lang="en">Ownership Status</rdfs:label>
    <rdfs:subClassOf rdf:resource="https://ontology.swissartresearch.net/aaao/ZE30_Property_Right_Status"/>
  </rdfs:Class>
  <rdfs:Class rdf:about="https://ontology.swissartresearch.net/aaao/ZE9_Residential_Status">
    <skos:notation rdf:datatype="http://www.w3.org/2001/XMLSchema#string">ZE9</skos:notation>
    <rdfs:comment xml:lang="en" rdf:datatype="http://www.w3.org/2001/XMLSchema#string">An instance of residential status is the collective ascription to an actor of a formal place of residence by a community. The substance of the residential status is the communal commitment to the recognition and use of the designated place with regards to the residence of the designated actor.
Instances of residential status are recognizable through evidence of community members adopting the intentional stance of so-recognizing this status, as observable from direct witnesses, through the reports of competent observers or through evidence of a declarative act initiating this status.
Instances of residence status may come to be through a formal process such as a declarative act of taking up residence, or may have arisen through habit, fiat or be of unknown origin. Instances of residence status may end either though a formal process, such as a new declarative act, or may simply fade out of use, be eliminated by fiat or be of unknown reason.  </rdfs:comment>
    <rdfs:label xml:lang="en">Residential Status</rdfs:label>
    <rdfs:subClassOf rdf:resource="https://ontology.swissartresearch.net/aaao/ZE35_Locative_Status"/>
  </rdfs:Class>
  <rdfs:Class rdf:about="https://ontology.swissartresearch.net/aaao/ZE10_Family_Status">
    <skos:notation rdf:datatype="http://www.w3.org/2001/XMLSchema#string">ZE10</skos:notation>
    <rdfs:comment xml:lang="en" rdf:datatype="http://www.w3.org/2001/XMLSchema#string">An instance of family status is the collective ascription of a familial relationship between one person and another by a community. The substance of the family status is the communal recognition of the familial connection between the two actors in question.
Instances of family status are recognizable through evidence of community members adopting the intentional stance  and behaviour indicated as proper to this relation, as observable from direct witnesses, through the reports of competent observers or through evidence of a declarative act (e.g.: adoption) initiating this status.
Instances of family status may come to be simply through birth in a certain community or may require that a formal process such as a right of passage has been undertaken. Instances of family status may end either though a formal process such as a renunciation or through death.  </rdfs:comment>
    <rdfs:label xml:lang="en">Family Status</rdfs:label>
    <rdfs:subClassOf rdf:resource="https://ontology.swissartresearch.net/aaao/ZE55_Social_Relation_Status"/>
  </rdfs:Class>
  <rdfs:Class rdf:about="https://ontology.swissartresearch.net/aaao/ZE11_Membership_Status">
    <skos:notation rdf:datatype="http://www.w3.org/2001/XMLSchema#string">ZE11</skos:notation>
    <rdfs:comment xml:lang="en" rdf:datatype="http://www.w3.org/2001/XMLSchema#string">An instance of membership status is the collective ascription of a membership relationship between an actor and some group by a community. The substance of the membership status is the communal recognition of the ascribed membership relation between the actor and the group in question.
Instances of membership status are recognizable through evidence of community members adopting the intentional stance  and behaviour indicated as proper to this relation, as observable from direct witnesses, through the reports of competent observers or through evidence of a declarative act [e.g.: ZE22 Declarative Joining] initiating this status.
Instances of membership status may come to be through a formal process such as a declarative act of declarative joining or may have arisen through habit, fiat or be of unknown origin. Instances of membership status may end either though a formal process [e.g.: ZE23 Declarative Leaving], or may simply fade out, be eliminated by fiat or for unknown reasons. </rdfs:comment>
    <rdfs:label xml:lang="en">Membership Status</rdfs:label>
    <rdfs:subClassOf rdf:resource="https://ontology.swissartresearch.net/aaao/ZE1_Institutional_Fact"/>
  </rdfs:Class>
  <rdfs:Class rdf:about="https://ontology.swissartresearch.net/aaao/ZE12_Referential_Status">
    <skos:notation rdf:datatype="http://www.w3.org/2001/XMLSchema#string">ZE12</skos:notation>
    <rdfs:comment xml:lang="en" rdf:datatype="http://www.w3.org/2001/XMLSchema#string">An instance of referential status is the collective ascription of a referential relationship between a propositional object and some entity by a community. The substance of the referential status is the communal recognition of the ascribed referential relation holding between the propositional object and the entity in question.
Instances of referential status are recognizable through evidence of community members adopting the intentional stance  and behaviour indicated as properly holding between the propositional object and the object it is taken to refer to in the manner it is meant to refer, as observable from direct witnesses, through the reports of competent observers or through evidence of a declarative act initiating this status.
Instances of referential status may come to be through a formal process such as a declarative act or may have arisen through habit, fiat or be of unknown origin. Instances of referential status may end either though a formal process, or may simply fade out, be eliminated by fiat or for unknown reasons. </rdfs:comment>
    <rdfs:label xml:lang="en">Referential Status</rdfs:label>
    <rdfs:subClassOf rdf:resource="https://ontology.swissartresearch.net/aaao/ZE1_Institutional_Fact"/>
  </rdfs:Class>
  <rdfs:Class rdf:about="https://ontology.swissartresearch.net/aaao/ZE13_Speech_Act">
    <skos:notation rdf:datatype="http://www.w3.org/2001/XMLSchema#string">ZE13</skos:notation>
    <rdfs:comment xml:lang="en" rdf:datatype="http://www.w3.org/2001/XMLSchema#string">An instance of speech act comprises an intentional activity engaged in by a set of actors to create a new institutional fact - or to nullify an existing one - that holds for a given community. In this sense, a speech act is transformative symbolic act. Speech acts are carried out by intentional actors through invoking a social rule and performing a prescribed set of actions often including the locution of set formulae of phrases by certain actors, fulfilling certain roles. Correct execution of the speech act as specified by the rule results in the existence of new institutional facts or their negation. The substance of speech act is ritual action performed by a group.
An instance of speech act begins when the intended ritual proceeding as specified by the rule invoked is initiated. The instance of speech act ends when the required set of actions specified for the act in question are executed or it is abandoned.</rdfs:comment>
    <rdfs:label xml:lang="en">Speech Act</rdfs:label>
    <rdfs:subClassOf rdf:resource="https://ontology.swissartresearch.net/aaao/ZE52_Transformative_Symbolic_Act"/>
  </rdfs:Class>
  <rdfs:Class rdf:about="https://ontology.swissartresearch.net/aaao/ZE14_Similarity_Status">
    <skos:notation rdf:datatype="http://www.w3.org/2001/XMLSchema#string">ZE14</skos:notation>
    <rdfs:comment xml:lang="en" rdf:datatype="http://www.w3.org/2001/XMLSchema#string">An instance of similarity status is the collective ascription of a similarity relationship between any two objects by a community. The substance of the similarity status is the communal recognition of the ascribed similarity relation between the two entities in question.
Instances of similarity status are recognizable through evidence of community members adopting the intentional stance and behaviour indicated by the kind of similarity believed to hold between the two referenced entities, as observable from direct witnesses, through the reports of competent observers or through evidence of a declarative act initiating this status.
Instances of similarity status may come to be through a formal process such as a declarative act (e.g., scholarship) or may have arisen through habit, fiat or be of unknown origin. Instances of similarity status may end either though a formal process (e.g., disproof or refutation), or may simply fade out, be eliminated by fiat or for unknown reasons.  </rdfs:comment>
    <rdfs:label xml:lang="en">Similarity Status</rdfs:label>
    <rdfs:subClassOf rdf:resource="https://ontology.swissartresearch.net/aaao/ZE1_Institutional_Fact"/>
  </rdfs:Class>
  <rdfs:Class rdf:about="https://ontology.swissartresearch.net/aaao/ZE15_Set_Status">
    <skos:notation rdf:datatype="http://www.w3.org/2001/XMLSchema#string">ZE15</skos:notation>
    <rdfs:comment xml:lang="en" rdf:datatype="http://www.w3.org/2001/XMLSchema#string">An instance of set status is the collective ascription of some relationship of belonging between some entity and a notional set by a community. The substance of the set status is the communal recognition of the ascribed belonging between the subject entity and the set in question.
Instances of set status are recognizable through evidence of community members adopting the intentional stance and behaviour indicated as proper to this set-belonging relation, as observable from direct witnesses, through the reports of competent observers or through evidence of a declarative act initiating this status.
Instances of set status may come to be through a formal process or may have arisen through habit, fiat or be of unknown origin. Instances of membership status may end either though a formal process, or may simply fade out, be eliminated by fiat or for unknown reasons.  </rdfs:comment>
    <rdfs:label xml:lang="en">Set Status</rdfs:label>
    <rdfs:subClassOf rdf:resource="https://ontology.swissartresearch.net/aaao/ZE1_Institutional_Fact"/>
  </rdfs:Class>
  <rdfs:Class rdf:about="https://ontology.swissartresearch.net/aaao/ZE17_Digital_Reading">
    <skos:notation rdf:datatype="http://www.w3.org/2001/XMLSchema#string">ZE17</skos:notation>
    <rdfs:comment xml:lang="en" rdf:datatype="http://www.w3.org/2001/XMLSchema#string">An instance of digital reading is a digital processing event guided by a set of instructions or parameters which in turn returns a digital output. The digital output will consist in a set of propositions related to the 'read' input which might include things like classifications, identifications, transformations, comparisons and so on. In the context of semantic data processes, such output might consist in semantically encoded knowledge graph statements, the collection of which may be referred to as an I4 Propositional Set, which can be regarded as the 'conclusion' of the digital reading. As such, Digital reading may be regarded as a computational process guided by a parametrized hypothesis resulting in a new propositional dataset for scientific consideration. The propositional information generated by the digital reading process should be considered as provisional knowledge posited under a hypothesis. Typically propositions generated by the digital reading may become the subject of further scholarly research.
Instances of this class come to be when a process is initiated to generate new information and finish upon completion of that process or if the process is interrupted and fails to complete.</rdfs:comment>
    <rdfs:label xml:lang="en">Digital Reading</rdfs:label>
    <rdfs:subClassOf rdf:resource="http://www.ics.forth.gr/isl/CRMdig/D7_Digital_Machine_Event"/>
    <rdfs:subClassOf rdf:resource="http://www.cidoc-crm.org/extensions/crmtex/TX5_Text_Recognition"/>
    <rdfs:subClassOf rdf:resource="https://ontology.swissartresearch.net/aaao/ZE13_Speech_Act"/>
  </rdfs:Class>
  <rdfs:Class rdf:about="https://ontology.swissartresearch.net/aaao/ZE18_Critical_Reading">
    <skos:notation rdf:datatype="http://www.w3.org/2001/XMLSchema#string">ZE18</skos:notation>
    <rdfs:comment xml:lang="en" rdf:datatype="http://www.w3.org/2001/XMLSchema#string">An instance of critical reading is a process of analysis undertaken by a scholar to derive analytical facts from a specific information resource. Critical reading engages the background knowledge of the scholar and their interpretive horizon in order to support them in actively reading the research object to derive factual, historically contextualized/contextualizing information regarding the propositional content in question and the world(s) it pertains too. This process can take as input previous scholarly documentation or outputs of digital reading events. Critical reading may result in a series of constructed arguments, serving as a foundation for the documentation and analysis of an argument regarding the text and its referents. Critical reading might also result in the observation, documentation or assertion of a social fact, such as the assertion of an appellative or classificatory status. In the latter case, the instance of ZE18 Critical Reading serves as provenance for the existence of the fact in the network.</rdfs:comment>
    <rdfs:label xml:lang="en">Critical Reading</rdfs:label>
    <rdfs:subClassOf rdf:resource="https://ontology.swissartresearch.net/aaao/ZE13_Speech_Act"/>
  </rdfs:Class>
  <rdfs:Class rdf:about="https://ontology.swissartresearch.net/aaao/ZE19_Naming">
    <skos:notation rdf:datatype="http://www.w3.org/2001/XMLSchema#string">ZE19</skos:notation>
    <rdfs:comment xml:lang="en" rdf:datatype="http://www.w3.org/2001/XMLSchema#string">Instances of naming are comprised of an act which officially confers a name to some object under a specific procedure. The substance of naming is an intentional, social act.
Instances of ZE19 Naming come about when the specific social procedure required is intentionally and successfully enacted according to the prevalent rules. They end with the successful termination of the act or because of its premature termination.
The result of the instance of naming is the coming to be of a collective acceptance of a name for some object in some mode for some time. The details of this institutional fact are documented in the resultant instance of ZE2 Appellative Status.</rdfs:comment>
    <rdfs:label xml:lang="en">Naming</rdfs:label>
    <rdfs:subClassOf rdf:resource="https://ontology.swissartresearch.net/aaao/ZE13_Speech_Act"/>
    <rdfs:subClassOf rdf:resource="http://www.cidoc-crm.org/cidoc-crm/E13_Attribute_Assignment"/>
  </rdfs:Class>
  <rdfs:Class rdf:about="https://ontology.swissartresearch.net/aaao/ZE20_Declarative_Acquisition">
    <skos:notation rdf:datatype="http://www.w3.org/2001/XMLSchema#string">ZE20</skos:notation>
    <rdfs:comment xml:lang="en" rdf:datatype="http://www.w3.org/2001/XMLSchema#string">Instances of this class comprise official acquisition events undertaken following formal procedures within a social grouping leading to formal ownership status over an object by some actor according to the participating parties. The substance of declarative acquisition is an intentional, social act. 
Instances of ZE20 Declarative Acquisition come about when the specific social procedure required is intentionally and successfully enacted according to the prevalent rules. They end with the successful termination of the act or because of its premature termination.
A successful act of ZE20 Declarative Acquisition leads to the generation of an instance of ZE8 Ownership Status, the institutional fact that thereafter mediates the social relation to this object until it has been abrogated.</rdfs:comment>
    <rdfs:label xml:lang="en">Declarative Acquisition</rdfs:label>
    <rdfs:subClassOf rdf:resource="https://ontology.swissartresearch.net/aaao/ZE29_Transfer_of_Property_Right"/>
    <rdfs:subClassOf rdf:resource="http://www.cidoc-crm.org/cidoc-crm/E8_Acquisition"/>
  </rdfs:Class>
  <rdfs:Class rdf:about="https://ontology.swissartresearch.net/aaao/ZE21_Declarative_Transfer_of_Custody">
    <skos:notation rdf:datatype="http://www.w3.org/2001/XMLSchema#string">ZE21</skos:notation>
    <rdfs:comment xml:lang="en" rdf:datatype="http://www.w3.org/2001/XMLSchema#string">Instances of this class comprise official transfer of custody events undertaken following formal procedures within a social grouping leading to formal change in the custody status over an object, ascribing it to some actor's custody, according to the participating parties. The substance of declarative transfer of custody is an intentional, social act. 
Instances of ZE21 Declarative Transfer of Custody come about when the specific social procedure required is intentionally and successfully enacted according to the prevalent rules. They end with the successful termination of the act or because of its premature termination.
A successful act of declarative transfer of custody leads to the generation of an instance of ZE7 Custodial Status, the institutional fact that thereafter mediates the social relation to this object until it has been abrogated.</rdfs:comment>
    <rdfs:label xml:lang="en">Declarative Transfer of Custody</rdfs:label>
    <rdfs:subClassOf rdf:resource="http://www.cidoc-crm.org/cidoc-crm/E10_Transfer_of_Custody"/>
    <rdfs:subClassOf rdf:resource="https://ontology.swissartresearch.net/aaao/ZE29_Transfer_of_Property_Right"/>
  </rdfs:Class>
  <rdfs:Class rdf:about="https://ontology.swissartresearch.net/aaao/ZE22_Declarative_Joining">
    <skos:notation rdf:datatype="http://www.w3.org/2001/XMLSchema#string">ZE22</skos:notation>
    <rdfs:comment xml:lang="en" rdf:datatype="http://www.w3.org/2001/XMLSchema#string">Instances of this class comprise official joining events undertaken following formal procedures within a social grouping leading to formal change in the membership status of an actor relative to a group for the participating parties. The substance of declarative joining is an intentional, social act. 
Instances of ZE22 Declarative Joining come about when the specific social procedure required is intentionally and successfully enacted according to the prevalent rules. They end with the successful termination of the act or because of its premature termination.
A successful act of ZE22 Declarative Joining leads to the generation of an instance of ZE11 Membership Status, the institutional fact that thereafter mediates the social relation between the group and actor in question until it has been abrogated.</rdfs:comment>
    <rdfs:label xml:lang="en">Declarative Joining</rdfs:label>
    <rdfs:subClassOf rdf:resource="http://www.cidoc-crm.org/cidoc-crm/E85_Joining"/>
    <rdfs:subClassOf rdf:resource="https://ontology.swissartresearch.net/aaao/ZE13_Speech_Act"/>
  </rdfs:Class>
  <rdfs:Class rdf:about="https://ontology.swissartresearch.net/aaao/ZE23_Declarative_Leaving">
    <skos:notation rdf:datatype="http://www.w3.org/2001/XMLSchema#string">ZE23</skos:notation>
    <rdfs:comment xml:lang="en" rdf:datatype="http://www.w3.org/2001/XMLSchema#string">Instances of this class comprise official leaving events undertaken following formal procedures within a social grouping leading to formal change in the membership status of an actor relative to a group for the participating parties. The substance of declarative leaving is an intentional, social act. 
Instances of ZE23 Declarative Leaving come about when the specific social procedure required is intentionally and successfully enacted according to the prevalent rules. They end with the successful termination of the act or because of its premature termination.
A successful act of ZE23 Declarative Leaving leads to the termination of an instance of ZE11 Membership Status, the institutional fact that thereafter no longer mediates the social relation between the group and actor in question.</rdfs:comment>
    <rdfs:label xml:lang="en">Declarative Leaving</rdfs:label>
    <rdfs:subClassOf rdf:resource="http://www.cidoc-crm.org/cidoc-crm/E86_Leaving"/>
    <rdfs:subClassOf rdf:resource="https://ontology.swissartresearch.net/aaao/ZE13_Speech_Act"/>
  </rdfs:Class>
  <rdfs:Class rdf:about="https://ontology.swissartresearch.net/aaao/ZE24_Notional_Set">
    <skos:notation rdf:datatype="http://www.w3.org/2001/XMLSchema#string">ZE24</skos:notation>
    <rdfs:comment xml:lang="en" rdf:datatype="http://www.w3.org/2001/XMLSchema#string">Instances of this class comprise notional sets of objects which have been grouped together for one reason or another. The substance of notional set is ideational.
A notional set comes to be when it is asserted or otherwise declared. It gains or loses members according to the particular rules guiding its maintenance. Typically instances of ZE24 Notional Set serve a functional purpose such as the grouping of some objects according to an ad hoc, context particular, or a context categorical criterion. 
See also Linked.Art:Set</rdfs:comment>
    <rdfs:label xml:lang="en">Notional Set</rdfs:label>
    <rdfs:subClassOf rdf:resource="http://www.cidoc-crm.org/cidoc-crm/E28_Conceptual_Object"/>
  </rdfs:Class>
  <rdfs:Class rdf:about="https://ontology.swissartresearch.net/aaao/ZE25_Dating_Status">
    <skos:notation rdf:datatype="http://www.w3.org/2001/XMLSchema#string">ZE25</skos:notation>
    <rdfs:comment xml:lang="en" rdf:datatype="http://www.w3.org/2001/XMLSchema#string">An instance of dating status is the collective ascription of a relative dating to an event (such as the production or the use of an object or the despotional moment of an archaeological context) by its association to an established and named historical or archaeological period or event. The substance of the dating status is the communal recognition of the ascribed chronology as holding true for the dated event and potential, relative object(s) it involves.
Instances of dating status are typically recorded in the archaeological / archival record.
Instances of dating status are most typically initiated by a formal process such as a scholarly dating attribution (ZE26 Dating Declaration). Instances of dating status may be terminated either through a formal process (official disproof) or be replaced by another dating declaration holding an updated belief and supported by further evidence.</rdfs:comment>
    <rdfs:label xml:lang="en">Dating Status</rdfs:label>
    <rdfs:subClassOf rdf:resource="https://ontology.swissartresearch.net/aaao/ZE1_Institutional_Fact"/>
  </rdfs:Class>
  <rdfs:Class rdf:about="https://ontology.swissartresearch.net/aaao/ZE26_Dating_Declaration">
    <skos:notation rdf:datatype="http://www.w3.org/2001/XMLSchema#string">ZE26</skos:notation>
    <rdfs:comment xml:lang="en" rdf:datatype="http://www.w3.org/2001/XMLSchema#string">Instances of dating declaration are scholarly acts which officially assign a historical or archaeological period to an event of interest (paradigmatic cases being the production or the time of use or termination of existence of some object or physical thing) of which, typically, a material artefact is the material remain. 
The result of the instance of dating declaration is the coming to be of a collective acceptance of the dating status for some object or some physical thing at some time by some group of people. This status may come to be contested or replaced by some new status, either through reasoned argumentation, assertion or even forgetting.
The details of this institutional fact are documented in the resultant instance of ZE25 Dating Status.</rdfs:comment>
    <rdfs:label xml:lang="en">Dating Declaration</rdfs:label>
    <rdfs:subClassOf rdf:resource="http://www.cidoc-crm.org/extensions/crminf/I1_Argumentation"/>
    <rdfs:subClassOf rdf:resource="https://ontology.swissartresearch.net/aaao/ZE13_Speech_Act"/>
  </rdfs:Class>
  <rdfs:Class rdf:about="https://ontology.swissartresearch.net/aaao/ZE27_Declaration_of_Obligation">
    <skos:notation rdf:datatype="http://www.w3.org/2001/XMLSchema#string">ZE27</skos:notation>
    <rdfs:comment xml:lang="en" rdf:datatype="http://www.w3.org/2001/XMLSchema#string">Instances of declaration of obligation are characterized by formal acts of recognition of a state of obligation between one party and another party for a certain measurable amount of goods.
Instances of this class comprise official acts undertaken following formal procedures within a social grouping leading to formal recognition of an obligation status between two actors. The substance of declaration of obligation is an intentional, social act.
Instances of ZE27 Declaration of Obligation come about when the specific social procedure required is intentionally and successfully enacted according to the prevalent rules. They end with the successful termination of the act or because of its premature termination.
A successful act of ZE27 Declaration of Obligation leads to the generation of an instance of ZE28 Obligation Status, the institutional fact that thereafter holds between two actors until it has been abrogated.</rdfs:comment>
    <rdfs:label xml:lang="en">Declaration of Obligation</rdfs:label>
    <rdfs:subClassOf rdf:resource="https://ontology.swissartresearch.net/aaao/ZE46_Promisory_Agreement"/>
  </rdfs:Class>
  <rdfs:Class rdf:about="https://ontology.swissartresearch.net/aaao/ZE28_Obligation_Status">
    <skos:notation rdf:datatype="http://www.w3.org/2001/XMLSchema#string">ZE28</skos:notation>
    <rdfs:comment xml:lang="en" rdf:datatype="http://www.w3.org/2001/XMLSchema#string">An instance of obligation status demarks a socially recognized state of obligation holding between two parties, wherein the first party is recognized to have the requirement to fulfil a debt to the second party for a certain measurable amount. The substance of the obligation status is the commitment from one party to another for compensation in a socially recognized form.
Instances of obligation status are recognizable through evidence of community members adopting the intentional stance of so recognizing this status, as observable from direct witnesses, through the reports of competent observers or through evidence of a declarative act [e.g.: ZE27 Declaration of Obligation) initiating this status.
Instances of obligation status may come to be through a formal process such as an act of declaring obligation [ZE27 Declaration of Obligation), or may have arisen through habit, fiat or be of unknown origin. Instances of obligation may end either though a formal process, such as an act of renunciation, or may simply fade out of use, be eliminated by fiat or be of unknown reason.</rdfs:comment>
    <rdfs:label xml:lang="en">Obligation Status</rdfs:label>
    <rdfs:subClassOf rdf:resource="https://ontology.swissartresearch.net/aaao/ZE45_Promisory_Status"/>
  </rdfs:Class>
  <rdfs:Class rdf:about="https://ontology.swissartresearch.net/aaao/ZE29_Transfer_of_Property_Right">
    <skos:notation rdf:datatype="http://www.w3.org/2001/XMLSchema#string">ZE29</skos:notation>
    <rdfs:comment xml:lang="en" rdf:datatype="http://www.w3.org/2001/XMLSchema#string">Instances of declaration of transfer of property right consist of events in which an official transfer of a property right is undertaken between two individuals with the result that a new right is assigned to the receiver and the right of the giver may be forfeited.
Instances of this class consist of events in which an official transfer of a property right is undertaken between two individuals with the result that a new right is assigned to the receiver and the right of the giver may be forfeited. The substance of transfer of property right is an intentional, social act. 
Instances of ZE29 Transfer of Property Right come about when the specific social procedure required is intentionally and successfully enacted according to the prevalent rules. They end with the successful termination of the act or because of its premature termination.
A successful act of ZE29 Transfer of Property Right leads to the generation of an instance of ZE30 Property Right Status, the institutional fact that thereafter mediates the social relation to this object until it has been abrogated.</rdfs:comment>
    <rdfs:label xml:lang="en">Transfer of Property Right</rdfs:label>
    <rdfs:subClassOf rdf:resource="https://ontology.swissartresearch.net/aaao/ZE13_Speech_Act"/>
  </rdfs:Class>
  <rdfs:Class rdf:about="https://ontology.swissartresearch.net/aaao/ZE30_Property_Right_Status">
    <skos:notation rdf:datatype="http://www.w3.org/2001/XMLSchema#string">ZE30</skos:notation>
    <rdfs:comment xml:lang="en" rdf:datatype="http://www.w3.org/2001/XMLSchema#string">Instances of property right status indicate the holding of a right over a legal object by some actor for some time.
An instance of property right status is the collective ascription of a relationship of legal right of some actor over a legal object by a community. The substance of the property right status is the communal commitment to the recognition of the right of use, right to earn income from, and right of disposal (of some sort) over the designated legal object by the actor in question.
Instances of property right status are recognizable through evidence of community members adopting the intentional stance of so recognizing this status, as observable from direct witnesses, through the reports of competent observers or through evidence of a declarative act [e.g.: ZE29 Transfer of Property Right) initiating this status.
Instances of property right status may come to be through a formal process such as a declarative act of taking possession of right [ZE29 Transfer of Property Right), or may have arisen through habit, fiat or be of unknown origin. Instances of property right status may end either though a formal process, such as a new transfer or right, or may simply fade out of use, be eliminated by fiat or be of unknown reason.</rdfs:comment>
    <rdfs:label xml:lang="en">Property Right Status</rdfs:label>
    <rdfs:subClassOf rdf:resource="https://ontology.swissartresearch.net/aaao/ZE1_Institutional_Fact"/>
  </rdfs:Class>
  <rdfs:Class rdf:about="https://ontology.swissartresearch.net/aaao/ZE33_Declarative_Formation">
    <skos:notation rdf:datatype="http://www.w3.org/2001/XMLSchema#string">ZE33</skos:notation>
    <rdfs:comment xml:lang="en" rdf:datatype="http://www.w3.org/2001/XMLSchema#string">Instances of this class comprise official group formation events undertaken following formal procedures within a social grouping leading to the formal existence of the group relative to the participating parties, whether subgroups or individual persons. The substance of declarative group formation is an intentional, social act. 
Instances of ZE33 Declarative Formation come about when the specific social procedure required is intentionally and successfully enacted according to the prevalent rules. They end with the successful termination of the act or because of its premature termination.
A successful act of ZE33 Declarative Formation leads to the generation of an instance of ZE11 Membership Status, the institutional fact that thereafter mediates the social relation between the group and actor in question until it has been abrogated.</rdfs:comment>
    <rdfs:label xml:lang="en">Declarative Formation</rdfs:label>
    <rdfs:subClassOf rdf:resource="http://www.cidoc-crm.org/cidoc-crm/E66_Formation"/>
    <rdfs:subClassOf rdf:resource="https://ontology.swissartresearch.net/aaao/ZE13_Speech_Act"/>
  </rdfs:Class>
  <rdfs:Class rdf:about="https://ontology.swissartresearch.net/aaao/ZE34_Declarative_Dissolution">
    <skos:notation rdf:datatype="http://www.w3.org/2001/XMLSchema#string">ZE34</skos:notation>
    <rdfs:comment xml:lang="en" rdf:datatype="http://www.w3.org/2001/XMLSchema#string">Instances of this class comprise official group dissolution events undertaken following formal procedures within a social grouping leading to the formal termination of the existence of the group relative to the participating parties, whether subgroups or individual persons. The substance of declarative group dissolution is an intentional, social act. 
Instances of ZE34 Declarative Dissolution come about when the specific social procedure required is intentionally and successfully enacted according to the prevalent rules. They end with the successful completion of the act or because of its premature termination.
A successful act of ZE34 Declarative Dissolution leads to the termination of an instance of ZE11 Membership Status for each of the groups members, whether individuals or subgroups, until such a time as the group is reformed.</rdfs:comment>
    <rdfs:label xml:lang="en">Declarative Dissolution</rdfs:label>
    <rdfs:subClassOf rdf:resource="https://ontology.swissartresearch.net/aaao/ZE13_Speech_Act"/>
    <rdfs:subClassOf rdf:resource="http://www.cidoc-crm.org/cidoc-crm/E68_Dissolution"/>
  </rdfs:Class>
  <rdfs:Class rdf:about="https://ontology.swissartresearch.net/aaao/ZE35_Locative_Status">
    <skos:notation rdf:datatype="http://www.w3.org/2001/XMLSchema#string">ZE35</skos:notation>
    <rdfs:comment xml:lang="en" rdf:datatype="http://www.w3.org/2001/XMLSchema#string">An instance of locative status is the collective ascription to an entity of a formal association to a geographic place. The substance of the locative status is the communal attribution of a defined association type between the designated entity and place. As opposed to connections created between entities and places through their passage through space and time, e.g.: the place of birth being a property of the birth event of an individual, locative statuses are created de jure rather than de facto and create a socially recognized connection between an entity and a location regardless the real or known spatiotemporal history of that object. For example, documentation may point to ambiguous evidence linking an object and a place such as the 'origin' of a person or the 'provenance' location of a physical object. In these cases, when we do not know the actual physical history of the object in question, but we do have a de jure attribution from which some knowledge may be derived, we can document and follow an instance of Locative Status for an object in relation to a geographic location.
Instances of locative status are recognizable through evidence of community members adopting the intentional stance of so recognizing this status, as observable from direct witnesses, through the reports of competent observers or through evidence of a declarative act initiating this status.
Instances of locative status may come to be through a formal process such as a declarative act of such definition, or may have arisen through habit, fiat or be of unknown origin. Instances of locative status may end either though a formal process, such as a new declarative act, or may simply fade out of use, be eliminated by fiat or be of unknown reason.</rdfs:comment>
    <rdfs:label xml:lang="en">Locative Status</rdfs:label>
    <rdfs:subClassOf rdf:resource="https://ontology.swissartresearch.net/aaao/ZE1_Institutional_Fact"/>
  </rdfs:Class>
  <rdfs:Class rdf:about="https://ontology.swissartresearch.net/aaao/ZE36_Persons">
    <skos:notation rdf:datatype="http://www.w3.org/2001/XMLSchema#string">ZE36</skos:notation>
    <rdfs:comment xml:lang="en" rdf:datatype="http://www.w3.org/2001/XMLSchema#string">Instances of this class comprise sentient beings endowed, to more or less extent, with intentionality, either as individuals or collectives. Instances of Persons are first causes and ends in themselves in a philosophical sense. The substance of Persons is personhood in this sense of being endowed with intentionality and the requisite respect qua sentient being. </rdfs:comment>
    <rdfs:label xml:lang="en">Persons</rdfs:label>
    <rdfs:subClassOf rdf:resource="http://www.cidoc-crm.org/cidoc-crm/E77_Persistent_Item"/>
  </rdfs:Class>
  <rdfs:Class rdf:about="https://ontology.swissartresearch.net/aaao/ZE37_Population">
    <skos:notation rdf:datatype="http://www.w3.org/2001/XMLSchema#string">ZE37</skos:notation>
    <rdfs:comment xml:lang="en" rdf:datatype="http://www.w3.org/2001/XMLSchema#string">This class comprises a defined set of persons who are considered to together form a coherent, identifiable unit according to certain characteristics such as citizenry, religious affiliation or other uniting characteristics or properties. Instances of population may be emically or etically defined. The substance of population is a collectivity of people[.]
Instances of population existence natural population come into and go out of existence through natural and social processes the particular details of which are often difficult to know or the subject of research and investigation. If a population is declaratively defined such as 'male voters between the age of 20 and 30 in Alabama in 2024 election cycle', then the existence condition is relative to the de jure declaration of their composition. An instance of population can be identified to be in existence when a suitable collective of individuals matching to its description can be identified to live and conform to those characteristics</rdfs:comment>
    <rdfs:label xml:lang="en">Population</rdfs:label>
    <rdfs:subClassOf rdf:resource="https://ontology.swissartresearch.net/aaao/ZE36_Persons"/>
    <rdfs:subClassOf rdf:resource="http://www.cidoc-crm.org/cidoc-crm/E18_Physical_Thing"/>
  </rdfs:Class>
  <rdfs:Class rdf:about="https://ontology.swissartresearch.net/aaao/ZE38_Population_Existence">
    <skos:notation rdf:datatype="http://www.w3.org/2001/XMLSchema#string">ZE38</skos:notation>
    <rdfs:comment xml:lang="en" rdf:datatype="http://www.w3.org/2001/XMLSchema#string">This class comprises the proper existence event of a population. Population existence consists in the temporal continuance of a specified population over a time and space.
Instances of population existence come into existence with the appearance or expression of the population and cease to exist with its dissolution. In the case of a de jure population, the duration of the population existence is a matter of declaration.</rdfs:comment>
    <rdfs:label xml:lang="en">Population Existence</rdfs:label>
    <rdfs:subClassOf rdf:resource="http://www.cidoc-crm.org/cidoc-crm/E5_Event"/>
  </rdfs:Class>
  <rdfs:Class rdf:about="https://ontology.swissartresearch.net/aaao/ZE39_Polity">
    <skos:notation rdf:datatype="http://www.w3.org/2001/XMLSchema#string">ZE39</skos:notation>
    <rdfs:comment xml:lang="en" rdf:datatype="http://www.w3.org/2001/XMLSchema#string">This class comprises a defined set of persons who are joined together by virtue of belonging to a shared civil society, collectively subject to the rights and responsibilities that that civil society confers. As an otherwise unorganized group, polities lack the agency required to undertake collective actions. They may however be subject to the actions of others, with the authority to organize the civil society to which the individuals belong. The substance of polity is a collectivity of people defined by their belonging to a shared civil society.
Instances of polity come into and go out of existence through natural and social processes, these may be formal (in the case, e.g., of a constitutional formation) or informal, where the particular details of the polity's formation are difficult to know or the subject of research and investigation. An instance of polity can be identified when a suitable collective of individuals matching to its description can be identified to live within the bounds of a recognized civil society.</rdfs:comment>
    <rdfs:label xml:lang="en">Polity</rdfs:label>
    <rdfs:subClassOf rdf:resource="https://ontology.swissartresearch.net/aaao/ZE37_Population"/>
  </rdfs:Class>
  <rdfs:Class rdf:about="https://ontology.swissartresearch.net/aaao/ZE43_Physical_Locative_Status">
    <skos:notation rdf:datatype="http://www.w3.org/2001/XMLSchema#string">ZE43</skos:notation>
    <rdfs:comment xml:lang="en" rdf:datatype="http://www.w3.org/2001/XMLSchema#string">An instance of physical locative status is the collective ascription to a physical object of a formal association to a geographic place. The substance of the locative status is the communal attribution of a defined association type between the designated object and place.
As opposed to connections created between physical objects and places through their passage through space and time, e.g.: the place of production being a property of the production event of an individual, physical locative statuses are created de jure rather than de facto and create a socially recognized connection between an object and a location regardless the real or known spatiotemporal history of that object. For example, documentation may point to ambiguous evidence linking an object and a place such as the 'provenance' location of a physical object. In these cases, when we do not know the actual physical history of the object in question, but we do have a de jure attribution from which some knowledge may be derived, we can document and follow an instance of Physical Locative Status for an object in relation to a geographic location.
Instances of physical locative status are recognizable through evidence of community members adopting the intentional stance of so recognizing this status, as observable from direct witnesses, through the reports of competent observers or through evidence of a declarative act initiating this status.
Instances of locative status may come to be through a formal process such as a declarative act of such definition, or may have arisen through habit, fiat or be of unknown origin. Instances of locative status may end either though a formal process, such as a new declarative act, or may simply fade out of use, be eliminated by fiat or be of unknown reason.</rdfs:comment>
    <rdfs:label xml:lang="en">Physical Locative Status</rdfs:label>
    <rdfs:subClassOf rdf:resource="https://ontology.swissartresearch.net/aaao/ZE35_Locative_Status"/>
  </rdfs:Class>
  <rdfs:Class rdf:about="https://ontology.swissartresearch.net/aaao/ZE44_Topographical_Status">
    <skos:notation rdf:datatype="http://www.w3.org/2001/XMLSchema#string">ZE44</skos:notation>
    <rdfs:comment xml:lang="en" rdf:datatype="http://www.w3.org/2001/XMLSchema#string">An instance of topographical status is the collective ascription to a geographical place of a formal spatial association to another geographic place. The substance of the topographical status is the communal attribution of a defined spatial association between two geographic places.
As opposed to connections created between geographic places as determine through a pure mathematic relation, e.g.: the falling within of a larger geometry by a smaller geometry, topographical statuses depend also on a de jure, socially recognized connection between two topographies. For example, when there are distinct political positions on the boundaries of a country, whether a geographic area 'falls within' another geographic area depends not only on the geometric calculation, but on the definition of extents of the geographic spaces in the first place. 
IInstances of topographical status are recognizable through evidence of community members adopting the intentional stance of so recognizing this status, as observable from direct witnesses, through the reports of competent observers or through evidence of a declarative act initiating this status.
Instances of topographical status may come to be through a formal process such as a declarative act of such definition, or may have arisen through habit, fiat or be of unknown origin. Instances of locative status may end either though a formal process, such as a new declarative act, or may simply fade out of use, be eliminated by fiat or be of unknown reason.</rdfs:comment>
    <rdfs:label xml:lang="en">Topographical Status</rdfs:label>
    <rdfs:subClassOf rdf:resource="https://ontology.swissartresearch.net/aaao/ZE35_Locative_Status"/>
  </rdfs:Class>
  <rdfs:Class rdf:about="https://ontology.swissartresearch.net/aaao/ZE45_Promisory_Status">
    <skos:notation rdf:datatype="http://www.w3.org/2001/XMLSchema#string">ZE45</skos:notation>
    <rdfs:comment xml:lang="en" rdf:datatype="http://www.w3.org/2001/XMLSchema#string">An instance of promissory status is the collective ascription of a promissory obligation between two parties. The substance of the promissory status is the communal recognition of the promise in question, which may nonetheless only bind two individuals directly. The substance of promissory status includes the ascription of an outcome which may detail guidelines and constraints that downstream activities on the part of promissory parties should comply with. Put otherwise, the promise promises a futural event on the part of the promisor to the promisee. The specified promissory constraints of this event can be instantiated on the level of kinds of processes, items or qualities and quantities involved in the action.
Instances of promissory status are recognizable through evidence of community members adopting an intentional stance towards the promise that exists between the two parties, as observable from direct witnesses, through the reports of competent observers or through documentary evidence of a declarative act (e.g.: ZE46 Promissory Agreement Event) initiating this status.
Instances of promissory status may come to be through a formal process such as a declarative promisory agreement, or may have arisen through habit, fiat or be of unknown origin. Instances of promissory status may end either through a formal process, such as a new declarative promissory agreement, the formal stripping of an existing promissory status, or may simply fade out of use, be eliminated by fiat or be of unknown reason.</rdfs:comment>
    <rdfs:label xml:lang="en">Promissory Status</rdfs:label>
    <rdfs:subClassOf rdf:resource="https://ontology.swissartresearch.net/aaao/ZE1_Institutional_Fact"/>
  </rdfs:Class>
  <rdfs:Class rdf:about="https://ontology.swissartresearch.net/aaao/ZE46_Promisory_Agreement">
    <skos:notation rdf:datatype="http://www.w3.org/2001/XMLSchema#string">ZE46</skos:notation>
    <rdfs:comment xml:lang="en" rdf:datatype="http://www.w3.org/2001/XMLSchema#string">Instances of promissory agreement event are characterized by formal acts of recognition of a promise between one party and another party for a certain outcome.
Instances of this class comprise explicit acts undertaken following given procedures within a social grouping leading to explicit recognition of a promissory status between two actors. The substance of promissory agreement is an intentional, social act.
Instances of ZE46 Promissory Agreement come about when the specific social procedure required is intentionally and successfully enacted according to the prevalent rules. They end with the successful termination of the act or because of its premature termination.
A successful act of ZE46 Promissory Agreement leads to the generation of an instance of ZE45 Promissory Status, the institutional fact that thereafter holds between two actors until it has been abrogated.</rdfs:comment>
    <rdfs:label xml:lang="en">Promissory Agreement Event</rdfs:label>
    <rdfs:subClassOf rdf:resource="http://iflastandards.info/ns/lrm/lrmoo/F28"/>
    <rdfs:subClassOf rdf:resource="https://ontology.swissartresearch.net/aaao/ZE13_Speech_Act"/>
  </rdfs:Class>
  <rdfs:Class rdf:about="https://ontology.swissartresearch.net/aaao/ZE49_Text_Sequence_Status">
    <skos:notation rdf:datatype="http://www.w3.org/2001/XMLSchema#string">ZE49</skos:notation>
    <rdfs:comment xml:lang="en" rdf:datatype="http://www.w3.org/2001/XMLSchema#string">An instance of text sequence status is a collective ascription to a written text sequence of a formal association to another written text sequence, in relation to which it is conceived as occupying a determinate place (i.e., the order in which they are to be read, wherein one text sequence follows another). The substance of the text sequence status is the communal attribution of a recognizable sequencing order between the designated text fields
As opposed to the connections created between a text field and the physical substrate upon which it is written, text sequence statuses are created de jure rather than de facto and create socially recognized connections between them. For example, an editorial annotation may indicate that a paragraph from a 'lower' position on the writing surface (such as a page) is to be inserted between two paragraphs at a 'higher' position (or on another page altogether). In such cases, the sequence in which the paragraphs are to be read does not coincide with the physical position of the text field in question, or the exact ordering of the paragraphs may be the subject of research or scholarly debate, but we do have de jure attribution from which some knowledge may be derived and documented with an instance of Text Sequence Status.
Instances of text sequence status are recognizable through evidence of community members adopting the intentional stance of so recognizing this status, as observable from direct witnesses, through the reports of competent observers or through evidence of a declarative act initiating this status.
Instances of text sequence status may come to be through a formal process such as a declarative act of such definition, or may have arisen through habit, fiat or be of unknown origin. Instances of text sequence status may end either though a formal process, such as a new declarative act, or may simply fade out of use, be eliminated by fiat or be of unknown reason.</rdfs:comment>
    <rdfs:label xml:lang="en">Text Sequence Status</rdfs:label>
    <rdfs:subClassOf rdf:resource="https://ontology.swissartresearch.net/aaao/ZE35_Locative_Status"/>
  </rdfs:Class>
  <rdfs:Class rdf:about="https://ontology.swissartresearch.net/aaao/ZE50_Authority_Status">
    <skos:notation rdf:datatype="http://www.w3.org/2001/XMLSchema#string">ZE50</skos:notation>
    <rdfs:comment xml:lang="en" rdf:datatype="http://www.w3.org/2001/XMLSchema#string">An instance of authority status is the collective ascription of an authority function to an actor by a community, although not necessary by their will. The substance of the authority status is the communal commitment to relating to and acting toward the actor in question according to the designated authority. Instances of authority status may be attributed to individuals or to groups of individuals.
Instances of authority status are recognizable through evidence of community members adopting the intentional stance of so relating or acting toward the actor in question, as observable from direct witnesses, through the reports of competent observers or through evidence of a declarative act [e.g.: E17 Type Assignment] initiating this status.
Instances of social status may come to be through a formal process such as a declarative act of assignment [E17 Type Assignment], or may have arisen through habit, fiat or be of unknown origin. Instances of social status may end either though a formal process, such as a new declarative act of classification, or simply fade out of existence.</rdfs:comment>
    <rdfs:label xml:lang="en">Authority Status</rdfs:label>
    <rdfs:subClassOf rdf:resource="https://ontology.swissartresearch.net/aaao/ZE6_Social_Status"/>
  </rdfs:Class>
  <rdfs:Class rdf:about="https://ontology.swissartresearch.net/aaao/ZE52_Transformative_Symbolic_Act">
    <skos:notation rdf:datatype="http://www.w3.org/2001/XMLSchema#string">ZE52</skos:notation>
    <rdfs:comment xml:lang="en" rdf:datatype="http://www.w3.org/2001/XMLSchema#string">This class comprises actions of a symbolic nature that are intentionally carried out by instances of E39 Actor and are transformative in consequence on a cultural and/or social level, initiating new instances of institutional fact or terminating the existence of previous institutional facts within that society / culture. An instance of transformative symbolic act is carried out within a social-cultural framework and makes use of the codes and symbols of that framework to communicate a message symbolically. As with any symbolic act, it may affirm or challenge one or more institutional facts recognized within such a system, but the specific difference of a transformative symbolic act is to be the cause of both new institutional facts and of the demise of existing institutional facts.
Instances of transformative symbolic act begin when an E39 Actor intentionally engages in an action invoking an existing code or symbol with the intent to affirm or challenge an institutional fact and end when the invoking act / practice has been completed (or was interrupted). The end of a transformative symbolic act is necessarily accompanied by the change in composition of the overall set of institutional facts of the social cultural framework in which it was undertaken, with one or more instances thereof either coming into or going out of existence.</rdfs:comment>
    <rdfs:label xml:lang="en">Transformative Symbolic Act</rdfs:label>
    <rdfs:subClassOf rdf:resource="https://ontology.swissartresearch.net/aaao/ZE53_Symbolic_Act"/>
  </rdfs:Class>
  <rdfs:Class rdf:about="https://ontology.swissartresearch.net/aaao/ZE53_Symbolic_Act">
    <skos:notation rdf:datatype="http://www.w3.org/2001/XMLSchema#string">ZE53</skos:notation>
    <rdfs:comment xml:lang="en" rdf:datatype="http://www.w3.org/2001/XMLSchema#string">This class comprises actions of a symbolic nature that are intentionally carried out by instances of E39 Actor. In engaging in a symbolic act, an E39 Actor communicates to other actors. The specific content of a symbolic act's communicative outcome currently lies beyond the scope of this class. Instances of this class can be used to document events of affirmative or negatory relation towards an extant social fact as communicated by an actor. An instance of symbolic act is carried out within a social-cultural framework and makes use of the codes and symbols of that framework to communicate a message symbolically and typically affirms or challenges one or more institutional facts recognized therein.
Instances of symbolic act begin when an E39 Actor intentionally engages in an action invoking an existing code or symbol with the intent to affirm or challenge an institutional fact and end when the invoking act / practice has been completed (or was interrupted).</rdfs:comment>
    <rdfs:label xml:lang="en">Symbolic Act</rdfs:label>
    <rdfs:subClassOf rdf:resource="http://www.cidoc-crm.org/cidoc-crm/E7_Activity"/>
  </rdfs:Class>
  <rdfs:Class rdf:about="https://ontology.swissartresearch.net/aaao/ZE55_Social_Relation_Status">
    <skos:notation rdf:datatype="http://www.w3.org/2001/XMLSchema#string">ZE55</skos:notation>
    <rdfs:comment xml:lang="en" rdf:datatype="http://www.w3.org/2001/XMLSchema#string">An instance of social relation status is the collective ascription of a social relationship between one person and another by a community. The substance of the social relation status is the communal recognition of the binary social connection between the two actors in question.
It is important to underline that an instance of social relation consists of is a binary construct that binds two different actors in a certain relation and is to be distinguished from social status. For example, an instance of social relation status could be the social relation status of "professor of" between a teacher and their student. This is a social relation status that is recognized particularly between the two individuals concerned, to be distinguished from a social status, recognized, for example, by the title 'Dr', which may or may not be held at the time in question and has no particular bearing on a relationship with any one individual.
Instances of social relation status are recognizable through evidence of community members adopting the intentional stance and behaviour indicated as proper to this relation, as observable from direct witnesses, through the reports of competent observers or through evidence of a declarative act initiating this status.
Instances of social relation status may come to be simply through birth in a certain community or may require that a formal process such as a right of passage has been undertaken. Instances of social relation status may end either though a formal process such as a renunciation, or may simply fade out of use, be eliminated by fiat or be of unknown reason. or through death.</rdfs:comment>
    <rdfs:label xml:lang="en">Social Relation Status</rdfs:label>
    <rdfs:subClassOf rdf:resource="https://ontology.swissartresearch.net/aaao/ZE1_Institutional_Fact"/>
  </rdfs:Class>
  <rdfs:Class rdf:about="https://ontology.swissartresearch.net/aaao/ZE59_Plan">
    <skos:notation rdf:datatype="http://www.w3.org/2001/XMLSchema#string">ZE59</skos:notation>
    <rdfs:comment xml:lang="en" rdf:datatype="http://www.w3.org/2001/XMLSchema#string">Instances of this class comprise symbolically expressed (whether in writing, orally or in some other recognized symbolic system within a socio-cultural group) projections of futural events and objectivities. An instance of this class is an intellectual object which describes a not yet extant futural world and describes how it is projected to be. A plan foresees what is foreseen to be brought about or to take place given certain eventualities. 
The content of a plan expressed as a machine-readable string can be documented in relation to an instance of this object via the property P190 has symbolic content.
The content of a plan can further be expressed in more analytic format by connecting it to a projected instance of Event Trigger Template which describes the particular set of parameters which are envisioned to take place when the plan would be executed.
An instance of plan comes into existence when it is symbolically formulated in some real instantiation and ceases to exist when no further carriers or memory of it remain.</rdfs:comment>
    <rdfs:label xml:lang="en">Plan</rdfs:label>
    <rdfs:subClassOf rdf:resource="http://www.cidoc-crm.org/cidoc-crm/E29_Design_or_Procedure"/>
    <rdfs:subClassOf rdf:resource="http://iflastandards.info/ns/lrm/lrmoo/F2"/>
  </rdfs:Class>
  <rdfs:Class rdf:about="https://ontology.swissartresearch.net/aaao/ZE60_Evental_Locative_Status">
    <skos:notation rdf:datatype="http://www.w3.org/2001/XMLSchema#string">ZE60</skos:notation>
    <rdfs:comment xml:lang="en" rdf:datatype="http://www.w3.org/2001/XMLSchema#string">An instance of evental locative status is the collective ascription to an event of a formal association to a geographic place. The substance of the locative status is the communal attribution of a defined association type between the designated event and place. As opposed to connections created between events and places through their passage through space and time, e.g.: the place of production being a property of the production event, evental locative statuses are created de jure rather than de facto and create a socially recognized connection between an event and a location regardless the real spatiotemporal history of that event, known or unknown.
Instances of evental locative status are recognizable through evidence of community members adopting the intentional stance of so recognizing this status, as observable from direct witnesses, through the reports of competent observers or through evidence of a declarative act initiating this status.
Instances of evental locative status may come to be through a formal process such as a declarative act of such definition, or may have arisen through habit, fiat or be of unknown origin. Instances of evental locative status may end either though a formal process, such as a new declarative act, or may simply fade out of use, be eliminated by fiat or be of unknown reason.</rdfs:comment>
    <rdfs:label xml:lang="en">Evental Locative Status</rdfs:label>
    <rdfs:subClassOf rdf:resource="https://ontology.swissartresearch.net/aaao/ZE35_Locative_Status"/>
  </rdfs:Class>
  <rdf:Property rdf:about="http://www.cidoc-crm.org/cidoc-crm/P11_had_participant">
    <rdfs:range rdf:resource="http://www.cidoc-crm.org/cidoc-crm/E39_Actor"/>
    <rdfs:comment xml:lang="en">This property describes the active or passive participation of instances of E39 Actors in an instance of E5 Event. It documents known events in which an instance of E39 Actor has participated during the course of that actor’s life or history. The instances of E53 Place and E52 Time-Span where and when these events happened provide us with constraints about the presence of the related instances of E39 Actor in the past. Collective actors, i.e., instances of E74 Group, may physically participate in events via their representing instances of E21 Persons only. The participation of multiple actors in an event is most likely an indication of their acquaintance and interaction.The property implies that the actor was involved in the event but does not imply any causal relationship. For instance, someone having been portrayed can be said to have participated in the creation of the portrait.</rdfs:comment>
    <rdfs:label xml:lang="en">had participant</rdfs:label>
    <skos:notation rdf:datatype="http://www.w3.org/2001/XMLSchema#string">P11</skos:notation>
    <rdfs:domain rdf:resource="http://www.cidoc-crm.org/cidoc-crm/E5_Event"/>
  </rdf:Property>
  <rdf:Property rdf:about="http://www.cidoc-crm.org/cidoc-crm/P12_occurred_in_the_presence_of">
    <rdfs:range rdf:resource="http://www.cidoc-crm.org/cidoc-crm/E77_Persistent_Item"/>
    <rdfs:comment xml:lang="en">This property describes the active or passive presence of an E77 Persistent Item in an instance of E5 Event without implying any specific role. It documents known events in which an instance of E77 Persistent Item was present during the course of its life or history. For example, an object may be the desk, now in a museum, on which a treaty was signed. The instance of E53 Place and the instance of E52 Time-Span where and when these events happened provide us with constraints about the presence of the related instance E77 Persistent Item in the past. Instances of E90 Symbolic Object, in particular information objects, are physically present in events via at least one of the instances of E18 Physical Thing carrying them. Note, that the human mind can be such a carrier. A precondition for a transfer of information to a person or another new physical carrier is the presence of the respective information object and this person or physical thing in one event.</rdfs:comment>
    <rdfs:label xml:lang="en">occurred in the presence of</rdfs:label>
    <skos:notation rdf:datatype="http://www.w3.org/2001/XMLSchema#string">P12</skos:notation>
    <rdfs:domain rdf:resource="http://www.cidoc-crm.org/cidoc-crm/E5_Event"/>
  </rdf:Property>
  <rdf:Property rdf:about="http://www.cidoc-crm.org/cidoc-crm/P14_carried_out_by">
    <rdfs:range rdf:resource="http://www.cidoc-crm.org/cidoc-crm/E39_Actor"/>
    <rdfs:comment xml:lang="en">This property describes the active participation of an instance of E39 Actor in an instance of E7 Activity. It implies causal or legal responsibility. The P14.1 in the role of property of the property specifies the nature of an Actor’s participation.</rdfs:comment>
    <rdfs:label xml:lang="en">carried out by</rdfs:label>
    <skos:notation rdf:datatype="http://www.w3.org/2001/XMLSchema#string">P14</skos:notation>
    <rdfs:domain rdf:resource="http://www.cidoc-crm.org/cidoc-crm/E7_Activity"/>
  </rdf:Property>
  <rdf:Property rdf:about="http://www.cidoc-crm.org/cidoc-crm/P16_used_specific_object">
    <rdfs:range rdf:resource="http://www.cidoc-crm.org/cidoc-crm/E70_Thing"/>
    <rdfs:comment xml:lang="en">This property describes the use of material or immaterial things in a way essential to the performance or the outcome of an instance of E7 Activity. This property typically applies to tools, instruments, moulds, raw materials and items embedded in a product. It implies that the presence of the object in question was a necessary condition for the action. For example, the activity of writing this text required the use of a computer. An immaterial thing can be used if at least one of its carriers is present. For example, the software tools on a computer.Another example is the use of a particular name by a particular group of people over some span to identify a thing, such as a settlement. In this case, the physical carriers of this name are at least the people understanding its use.</rdfs:comment>
    <rdfs:label xml:lang="en">used specific object</rdfs:label>
    <skos:notation rdf:datatype="http://www.w3.org/2001/XMLSchema#string">P16</skos:notation>
    <rdfs:domain rdf:resource="http://www.cidoc-crm.org/cidoc-crm/E7_Activity"/>
  </rdf:Property>
  <rdf:Property rdf:about="http://www.cidoc-crm.org/cidoc-crm/P33_used_specific_technique">
    <rdfs:range rdf:resource="http://www.cidoc-crm.org/cidoc-crm/E29_Design_or_Procedure"/>
    <rdfs:comment xml:lang="en">This property identifies a specific instance of E29 Design or Procedure in order to carry out an instance of E7 Activity or parts of it. The property differs from P32 used general technique (was technique of) in that P33 refers to an instance of E29 Design or Procedure, which is a concrete information object in its own right rather than simply being a term or a method known by tradition. Typical examples would include intervention plans for conservation or the construction plans of a building.</rdfs:comment>
    <rdfs:label xml:lang="en">used specific technique</rdfs:label>
    <skos:notation rdf:datatype="http://www.w3.org/2001/XMLSchema#string">P33</skos:notation>
    <rdfs:domain rdf:resource="http://www.cidoc-crm.org/cidoc-crm/E7_Activity"/>
  </rdf:Property>
  <rdf:Property rdf:about="http://iflastandards.info/ns/lrm/lrmoo/R17">
    <rdfs:range rdf:resource="http://iflastandards.info/ns/lrm/lrmoo/F2"/>
    <rdfs:comment xml:lang="en">This property associates an instance of F2 Expression that was externalised during a particular instance of F28 Expression Creation event with that particular creation event. An instance of expression creation creates an instance of expression and also creates any expressions that are parts of that expression.</rdfs:comment>
    <rdfs:label xml:lang="en">created</rdfs:label>
    <skos:notation rdf:datatype="http://www.w3.org/2001/XMLSchema#string">R17</skos:notation>
    <rdfs:domain rdf:resource="http://iflastandards.info/ns/lrm/lrmoo/F28"/>
  </rdf:Property>
  <rdf:Property rdf:about="https://ontology.swissartresearch.net/aaao/ZP1_has_intentional_subject">
    <rdfs:range rdf:resource="http://www.cidoc-crm.org/cidoc-crm/E1_CRM_Entity"/>
    <rdfs:comment xml:lang="en">This property is used to connect an instance of institutional fact to an entity with which it is concerned. The intentional subject indicated by this property is the object about which the institutional fact holds for the group committed to this institutional reality.</rdfs:comment>
    <rdfs:label xml:lang="en">has intentional subject</rdfs:label>
    <skos:notation rdf:datatype="http://www.w3.org/2001/XMLSchema#string">ZP1</skos:notation>
    <rdfs:domain rdf:resource="https://ontology.swissartresearch.net/aaao/ZE1_Institutional_Fact"/>
  </rdf:Property>
  <rdf:Property rdf:about="https://ontology.swissartresearch.net/aaao/ZP2_ascribes_intentional_target">
    <rdfs:range rdf:resource="http://www.cidoc-crm.org/cidoc-crm/E1_CRM_Entity"/>
    <rdfs:comment xml:lang="en">This property is used to indicate the entity which an instance of institutional fact ascribes to its subject. The intentional target indicated by this property is the object which the institutional fact establishes as holding of its subject for the group committed to this institutional reality. The manner of its holding is indicated by the intentional relation.</rdfs:comment>
    <rdfs:label xml:lang="en">ascribes intentional target</rdfs:label>
    <skos:notation rdf:datatype="http://www.w3.org/2001/XMLSchema#string">ZP2</skos:notation>
    <rdfs:domain rdf:resource="https://ontology.swissartresearch.net/aaao/ZE1_Institutional_Fact"/>
  </rdf:Property>
  <rdf:Property rdf:about="https://ontology.swissartresearch.net/aaao/ZP3_ascribes_intentional_relation">
    <rdfs:range rdf:resource="http://www.cidoc-crm.org/cidoc-crm/E55_Type"/>
    <rdfs:comment xml:lang="en">This property is used to indicate the relationship which an instance of institutional fact takes to hold between its subject and its object. The intentional relation indicated by this property is the kind of relationship which the institutional fact establishes as holding between them  for the group committed to this institutional reality.</rdfs:comment>
    <rdfs:label xml:lang="en">ascribes intentional relation</rdfs:label>
    <skos:notation rdf:datatype="http://www.w3.org/2001/XMLSchema#string">ZP3</skos:notation>
    <rdfs:domain rdf:resource="https://ontology.swissartresearch.net/aaao/ZE1_Institutional_Fact"/>
  </rdf:Property>
  <rdf:Property rdf:about="https://ontology.swissartresearch.net/aaao/ZP4_holds_for">
    <rdfs:range rdf:resource="http://www.cidoc-crm.org/cidoc-crm/E74_Group"/>
    <rdfs:comment xml:lang="en">This property is used to indicate the community or group for whom an instance of institutional fact holds. Institutional facts have identity only relative to some group for whom they have a significance as formulated through a chosen symbolic system. </rdfs:comment>
    <rdfs:label xml:lang="en">holds for</rdfs:label>
    <skos:notation rdf:datatype="http://www.w3.org/2001/XMLSchema#string">ZP4</skos:notation>
    <rdfs:domain rdf:resource="https://ontology.swissartresearch.net/aaao/ZE1_Institutional_Fact"/>
  </rdf:Property>
  <rdf:Property rdf:about="https://ontology.swissartresearch.net/aaao/ZP5_has_appellative_subject">
    <rdfs:range rdf:resource="http://www.cidoc-crm.org/cidoc-crm/E1_CRM_Entity"/>
    <rdfs:comment xml:lang="en">This property is used to indicate the entity for which an appellation holds as institutional fact.</rdfs:comment>
    <rdfs:label xml:lang="en">has appellative subject</rdfs:label>
    <skos:notation rdf:datatype="http://www.w3.org/2001/XMLSchema#string">ZP5</skos:notation>
    <rdfs:domain rdf:resource="https://ontology.swissartresearch.net/aaao/ZE2_Appellative_Status"/>
    <rdfs:subPropertyOf rdf:resource="https://ontology.swissartresearch.net/aaao/ZP1_has_intentional_subject"/>
  </rdf:Property>
  <rdf:Property rdf:about="https://ontology.swissartresearch.net/aaao/ZP6_ascribes_appellation">
    <rdfs:range rdf:resource="http://www.cidoc-crm.org/cidoc-crm/E41_Appellation"/>
    <rdfs:comment xml:lang="en">This property is used to indicate the appellation which is indicated as holding for the named subject of the appellative status.

 
</rdfs:comment>
    <rdfs:label xml:lang="en">ascribes appellation</rdfs:label>
    <skos:notation rdf:datatype="http://www.w3.org/2001/XMLSchema#string">ZP6</skos:notation>
    <rdfs:domain rdf:resource="https://ontology.swissartresearch.net/aaao/ZE2_Appellative_Status"/>
    <rdfs:subPropertyOf rdf:resource="https://ontology.swissartresearch.net/aaao/ZP2_ascribes_intentional_target"/>
  </rdf:Property>
  <rdf:Property rdf:about="https://ontology.swissartresearch.net/aaao/ZP7_ascribes_appellative_relation">
    <rdfs:range rdf:resource="http://www.cidoc-crm.org/cidoc-crm/E55_Type"/>
    <rdfs:comment xml:lang="en">This property is used to indicate the specific manner in which the appellation which is indicated as holding for the named subject of the appellative status pertains to this subject.

 
</rdfs:comment>
    <rdfs:label xml:lang="en">ascribes appellative relation</rdfs:label>
    <skos:notation rdf:datatype="http://www.w3.org/2001/XMLSchema#string">ZP7</skos:notation>
    <rdfs:domain rdf:resource="https://ontology.swissartresearch.net/aaao/ZE2_Appellative_Status"/>
    <rdfs:subPropertyOf rdf:resource="https://ontology.swissartresearch.net/aaao/ZP3_ascribes_intentional_relation"/>
  </rdf:Property>
  <rdf:Property rdf:about="https://ontology.swissartresearch.net/aaao/ZP8_has_contact_point_subject">
    <rdfs:range rdf:resource="http://www.cidoc-crm.org/cidoc-crm/E39_Actor"/>
    <rdfs:comment xml:lang="en">This property is used to indicate the entity for which a contact point has been specified as means of contact.

 
</rdfs:comment>
    <rdfs:label xml:lang="en">has contact point subject</rdfs:label>
    <skos:notation rdf:datatype="http://www.w3.org/2001/XMLSchema#string">ZP8</skos:notation>
    <rdfs:domain rdf:resource="https://ontology.swissartresearch.net/aaao/ZE3_Contact_Point_Status"/>
    <rdfs:subPropertyOf rdf:resource="https://ontology.swissartresearch.net/aaao/ZP5_has_appellative_subject"/>
  </rdf:Property>
  <rdf:Property rdf:about="https://ontology.swissartresearch.net/aaao/ZP9_ascribes_contact_point">
    <rdfs:range rdf:resource="http://www.cidoc-crm.org/cidoc-crm/E42_Identifier"/>
    <rdfs:comment xml:lang="en">This property is used to indicate the contact point which is indicated as holding for the named subject of the contact status.

 
</rdfs:comment>
    <rdfs:label xml:lang="en">ascribes contact point</rdfs:label>
    <skos:notation rdf:datatype="http://www.w3.org/2001/XMLSchema#string">ZP9</skos:notation>
    <rdfs:domain rdf:resource="https://ontology.swissartresearch.net/aaao/ZE3_Contact_Point_Status"/>
    <rdfs:subPropertyOf rdf:resource="https://ontology.swissartresearch.net/aaao/ZP6_ascribes_appellation"/>
  </rdf:Property>
  <rdf:Property rdf:about="https://ontology.swissartresearch.net/aaao/ZP10_ascribes_contact_point_relation">
    <rdfs:range rdf:resource="http://www.cidoc-crm.org/cidoc-crm/E55_Type"/>
    <rdfs:comment xml:lang="en">This property is used to indicate the specific manner in which the contact point which is indicated as holding for the named subject of the contact status pertains to this subject.

 
</rdfs:comment>
    <rdfs:label xml:lang="en">ascribes contact point relation</rdfs:label>
    <skos:notation rdf:datatype="http://www.w3.org/2001/XMLSchema#string">ZP10</skos:notation>
    <rdfs:domain rdf:resource="https://ontology.swissartresearch.net/aaao/ZE3_Contact_Point_Status"/>
    <rdfs:subPropertyOf rdf:resource="https://ontology.swissartresearch.net/aaao/ZP7_ascribes_appellative_relation"/>
  </rdf:Property>
  <rdf:Property rdf:about="https://ontology.swissartresearch.net/aaao/ZP11_has_classificatory_subject">
    <rdfs:range rdf:resource="http://www.cidoc-crm.org/cidoc-crm/E1_CRM_Entity"/>
    <rdfs:comment xml:lang="en">This property is used to indicate the entity for which a certain classification is taken to hold by the instance of classificatory status.

 
</rdfs:comment>
    <rdfs:label xml:lang="en">has classificatory subject</rdfs:label>
    <skos:notation rdf:datatype="http://www.w3.org/2001/XMLSchema#string">ZP11</skos:notation>
    <rdfs:domain rdf:resource="https://ontology.swissartresearch.net/aaao/ZE4_Classificatory_Status"/>
    <rdfs:subPropertyOf rdf:resource="https://ontology.swissartresearch.net/aaao/ZP1_has_intentional_subject"/>
  </rdf:Property>
  <rdf:Property rdf:about="https://ontology.swissartresearch.net/aaao/ZP12_ascribes_classification">
    <rdfs:range rdf:resource="http://www.cidoc-crm.org/cidoc-crm/E55_Type"/>
    <rdfs:comment xml:lang="en">This property is used to indicate the type which is indicated as holding for the subject of the classification status.

 
</rdfs:comment>
    <rdfs:label xml:lang="en">ascribes classification</rdfs:label>
    <skos:notation rdf:datatype="http://www.w3.org/2001/XMLSchema#string">ZP12</skos:notation>
    <rdfs:domain rdf:resource="https://ontology.swissartresearch.net/aaao/ZE4_Classificatory_Status"/>
    <rdfs:subPropertyOf rdf:resource="https://ontology.swissartresearch.net/aaao/ZP2_ascribes_intentional_target"/>
  </rdf:Property>
  <rdf:Property rdf:about="https://ontology.swissartresearch.net/aaao/ZP13_ascribes_classification_relation">
    <rdfs:range rdf:resource="http://www.cidoc-crm.org/cidoc-crm/E55_Type"/>
    <rdfs:comment xml:lang="en">This property is used to indicate the specific manner in which the type which is indicated as holding for the subject of the classification status pertains to this subject.

 
</rdfs:comment>
    <rdfs:label xml:lang="en">ascribes classification relation</rdfs:label>
    <skos:notation rdf:datatype="http://www.w3.org/2001/XMLSchema#string">ZP13</skos:notation>
    <rdfs:domain rdf:resource="https://ontology.swissartresearch.net/aaao/ZE4_Classificatory_Status"/>
    <rdfs:subPropertyOf rdf:resource="https://ontology.swissartresearch.net/aaao/ZP3_ascribes_intentional_relation"/>
  </rdf:Property>
  <rdf:Property rdf:about="https://ontology.swissartresearch.net/aaao/ZP14_has_functional_subject">
    <rdfs:range rdf:resource="http://www.cidoc-crm.org/cidoc-crm/E1_CRM_Entity"/>
    <rdfs:comment xml:lang="en">This property is used to indicate the entity for which a certain functional classification is taken to hold by the instance of functional status.

 
</rdfs:comment>
    <rdfs:label xml:lang="en">has functional subject</rdfs:label>
    <skos:notation rdf:datatype="http://www.w3.org/2001/XMLSchema#string">ZP14</skos:notation>
    <rdfs:domain rdf:resource="https://ontology.swissartresearch.net/aaao/ZE5_Function_Status"/>
    <rdfs:subPropertyOf rdf:resource="https://ontology.swissartresearch.net/aaao/ZP11_has_classificatory_subject"/>
  </rdf:Property>
  <rdf:Property rdf:about="https://ontology.swissartresearch.net/aaao/ZP15_ascribes_function">
    <rdfs:range rdf:resource="http://www.cidoc-crm.org/cidoc-crm/E55_Type"/>
    <rdfs:comment xml:lang="en">This property is used to indicate the type of function which is indicated as holding for the subject of the function status.

 
</rdfs:comment>
    <rdfs:label xml:lang="en">ascribes function</rdfs:label>
    <skos:notation rdf:datatype="http://www.w3.org/2001/XMLSchema#string">ZP15</skos:notation>
    <rdfs:domain rdf:resource="https://ontology.swissartresearch.net/aaao/ZE5_Function_Status"/>
    <rdfs:subPropertyOf rdf:resource="https://ontology.swissartresearch.net/aaao/ZP12_ascribes_classification"/>
  </rdf:Property>
  <rdf:Property rdf:about="https://ontology.swissartresearch.net/aaao/ZP16_ascribes_functional_relation">
    <rdfs:range rdf:resource="http://www.cidoc-crm.org/cidoc-crm/E55_Type"/>
    <rdfs:comment xml:lang="en">This property is used to indicate the specific manner in which the function which is indicated as holding for the subject of the function status pertains to this subject.

 
</rdfs:comment>
    <rdfs:label xml:lang="en">ascribes functional relation</rdfs:label>
    <skos:notation rdf:datatype="http://www.w3.org/2001/XMLSchema#string">ZP16</skos:notation>
    <rdfs:domain rdf:resource="https://ontology.swissartresearch.net/aaao/ZE5_Function_Status"/>
    <rdfs:subPropertyOf rdf:resource="https://ontology.swissartresearch.net/aaao/ZP13_ascribes_classification_relation"/>
  </rdf:Property>
  <rdf:Property rdf:about="https://ontology.swissartresearch.net/aaao/ZP17_has_social_status_subject">
    <rdfs:range rdf:resource="http://www.cidoc-crm.org/cidoc-crm/E39_Actor"/>
    <rdfs:comment xml:lang="en">This property is used to indicate the actor for which a certain social status is taken to hold by the instance of social status.

 
</rdfs:comment>
    <rdfs:label xml:lang="en">has social status subject</rdfs:label>
    <skos:notation rdf:datatype="http://www.w3.org/2001/XMLSchema#string">ZP17</skos:notation>
    <rdfs:domain rdf:resource="https://ontology.swissartresearch.net/aaao/ZE6_Social_Status"/>
    <rdfs:subPropertyOf rdf:resource="https://ontology.swissartresearch.net/aaao/ZP11_has_classificatory_subject"/>
  </rdf:Property>
  <rdf:Property rdf:about="https://ontology.swissartresearch.net/aaao/ZP18_ascribes_social_status">
    <rdfs:range rdf:resource="http://www.cidoc-crm.org/cidoc-crm/E55_Type"/>
    <rdfs:comment xml:lang="en">This property is used to indicate the type of social status which is indicated as holding for the subject of the social status ascription.

 
</rdfs:comment>
    <rdfs:label xml:lang="en">ascribes social status</rdfs:label>
    <skos:notation rdf:datatype="http://www.w3.org/2001/XMLSchema#string">ZP18</skos:notation>
    <rdfs:domain rdf:resource="https://ontology.swissartresearch.net/aaao/ZE6_Social_Status"/>
    <rdfs:subPropertyOf rdf:resource="https://ontology.swissartresearch.net/aaao/ZP12_ascribes_classification"/>
  </rdf:Property>
  <rdf:Property rdf:about="https://ontology.swissartresearch.net/aaao/ZP19_ascribes_social_status_relation">
    <rdfs:range rdf:resource="http://www.cidoc-crm.org/cidoc-crm/E55_Type"/>
    <rdfs:comment xml:lang="en">This property is used to indicate the specific manner in which the type of social status which is indicated as holding for the subject pertains to this subject.

 
</rdfs:comment>
    <rdfs:label xml:lang="en">ascribes social status relation</rdfs:label>
    <skos:notation rdf:datatype="http://www.w3.org/2001/XMLSchema#string">ZP19</skos:notation>
    <rdfs:domain rdf:resource="https://ontology.swissartresearch.net/aaao/ZE6_Social_Status"/>
    <rdfs:subPropertyOf rdf:resource="https://ontology.swissartresearch.net/aaao/ZP13_ascribes_classification_relation"/>
  </rdf:Property>
  <rdf:Property rdf:about="https://ontology.swissartresearch.net/aaao/ZP20_has_custodial_subject">
    <rdfs:range rdf:resource="http://www.cidoc-crm.org/cidoc-crm/E18_Physical_Thing"/>
    <rdfs:comment xml:lang="en">This property is used to indicate the physical thing over which a certain custodial status is taken to hold.

 
</rdfs:comment>
    <rdfs:label xml:lang="en">has custodial subject</rdfs:label>
    <skos:notation rdf:datatype="http://www.w3.org/2001/XMLSchema#string">ZP20</skos:notation>
    <rdfs:domain rdf:resource="https://ontology.swissartresearch.net/aaao/ZE7_Custodial_Status"/>
    <rdfs:subPropertyOf rdf:resource="https://ontology.swissartresearch.net/aaao/ZP1_has_intentional_subject"/>
  </rdf:Property>
  <rdf:Property rdf:about="https://ontology.swissartresearch.net/aaao/ZP21_ascribes_custodian">
    <rdfs:range rdf:resource="http://www.cidoc-crm.org/cidoc-crm/E39_Actor"/>
    <rdfs:comment xml:lang="en">This property is used to indicate the custodian to whom the custody of the physical thing which is the subject of the custodial status redounds.

 
</rdfs:comment>
    <rdfs:label xml:lang="en">ascribes custodian</rdfs:label>
    <skos:notation rdf:datatype="http://www.w3.org/2001/XMLSchema#string">ZP21</skos:notation>
    <rdfs:domain rdf:resource="https://ontology.swissartresearch.net/aaao/ZE7_Custodial_Status"/>
    <rdfs:subPropertyOf rdf:resource="https://ontology.swissartresearch.net/aaao/ZP2_ascribes_intentional_target"/>
  </rdf:Property>
  <rdf:Property rdf:about="https://ontology.swissartresearch.net/aaao/ZP22_ascribes_custodial_relation">
    <rdfs:range rdf:resource="http://www.cidoc-crm.org/cidoc-crm/E55_Type"/>
    <rdfs:comment xml:lang="en">This property is used to indicate the specific manner in which the custodial status which is indicated as holding over the legal object by the custodian pertains to this subject.

 
</rdfs:comment>
    <rdfs:label xml:lang="en">ascribes custodial relation</rdfs:label>
    <skos:notation rdf:datatype="http://www.w3.org/2001/XMLSchema#string">ZP22</skos:notation>
    <rdfs:domain rdf:resource="https://ontology.swissartresearch.net/aaao/ZE7_Custodial_Status"/>
    <rdfs:subPropertyOf rdf:resource="https://ontology.swissartresearch.net/aaao/ZP3_ascribes_intentional_relation"/>
  </rdf:Property>
  <rdf:Property rdf:about="https://ontology.swissartresearch.net/aaao/ZP23_has_ownership_subject">
    <rdfs:range rdf:resource="http://www.cidoc-crm.org/cidoc-crm/E18_Physical_Thing"/>
    <rdfs:comment xml:lang="en">This property is used to indicate the legal object over which a certain ownership status is taken to hold.

 
</rdfs:comment>
    <rdfs:label xml:lang="en">has ownership subject</rdfs:label>
    <skos:notation rdf:datatype="http://www.w3.org/2001/XMLSchema#string">ZP23</skos:notation>
    <rdfs:domain rdf:resource="https://ontology.swissartresearch.net/aaao/ZE8_Ownership_Status"/>
    <rdfs:subPropertyOf rdf:resource="https://ontology.swissartresearch.net/aaao/ZP1_has_intentional_subject"/>
  </rdf:Property>
  <rdf:Property rdf:about="https://ontology.swissartresearch.net/aaao/ZP24_ascribes_owner">
    <rdfs:range rdf:resource="http://www.cidoc-crm.org/cidoc-crm/E39_Actor"/>
    <rdfs:comment xml:lang="en">This property is used to indicate the owner to whom the title of the legal object which is the subject of the ownership status redounds.

 
</rdfs:comment>
    <rdfs:label xml:lang="en">ascribes owner</rdfs:label>
    <skos:notation rdf:datatype="http://www.w3.org/2001/XMLSchema#string">ZP24</skos:notation>
    <rdfs:domain rdf:resource="https://ontology.swissartresearch.net/aaao/ZE8_Ownership_Status"/>
    <rdfs:subPropertyOf rdf:resource="https://ontology.swissartresearch.net/aaao/ZP2_ascribes_intentional_target"/>
  </rdf:Property>
  <rdf:Property rdf:about="https://ontology.swissartresearch.net/aaao/ZP25_ascribes_ownership_relation">
    <rdfs:range rdf:resource="http://www.cidoc-crm.org/cidoc-crm/E55_Type"/>
    <rdfs:comment xml:lang="en">This property is used to indicate the specific manner in which the ownership status which is indicated as holding over the legal object by the owner pertains to this subject.

 
</rdfs:comment>
    <rdfs:label xml:lang="en">ascribes ownership relation</rdfs:label>
    <skos:notation rdf:datatype="http://www.w3.org/2001/XMLSchema#string">ZP25</skos:notation>
    <rdfs:domain rdf:resource="https://ontology.swissartresearch.net/aaao/ZE8_Ownership_Status"/>
    <rdfs:subPropertyOf rdf:resource="https://ontology.swissartresearch.net/aaao/ZP3_ascribes_intentional_relation"/>
  </rdf:Property>
  <rdf:Property rdf:about="https://ontology.swissartresearch.net/aaao/ZP26_has_residence_subject">
    <rdfs:range rdf:resource="http://www.cidoc-crm.org/cidoc-crm/E39_Actor"/>
    <rdfs:comment xml:lang="en">This property is used to indicate the actor for whom the residence status is taken to hold.

 
</rdfs:comment>
    <rdfs:label xml:lang="en">has residence subject</rdfs:label>
    <skos:notation rdf:datatype="http://www.w3.org/2001/XMLSchema#string">ZP26</skos:notation>
    <rdfs:domain rdf:resource="https://ontology.swissartresearch.net/aaao/ZE9_Residential_Status"/>
    <rdfs:subPropertyOf rdf:resource="https://ontology.swissartresearch.net/aaao/ZP1_has_intentional_subject"/>
  </rdf:Property>
  <rdf:Property rdf:about="https://ontology.swissartresearch.net/aaao/ZP27_acribes_residence_place">
    <rdfs:range rdf:resource="http://www.cidoc-crm.org/cidoc-crm/E53_Place"/>
    <rdfs:comment xml:lang="en">This property is used to indicate the place at which the subject of the residence status is taken to reside or dwell.

 
</rdfs:comment>
    <rdfs:label xml:lang="en">ascribes residence place</rdfs:label>
    <skos:notation rdf:datatype="http://www.w3.org/2001/XMLSchema#string">ZP27</skos:notation>
    <rdfs:domain rdf:resource="https://ontology.swissartresearch.net/aaao/ZE9_Residential_Status"/>
    <rdfs:subPropertyOf rdf:resource="https://ontology.swissartresearch.net/aaao/ZP77_ascribes_place"/>
  </rdf:Property>
  <rdf:Property rdf:about="https://ontology.swissartresearch.net/aaao/ZP28_ascribes_residence_relation">
    <rdfs:range rdf:resource="http://www.cidoc-crm.org/cidoc-crm/E55_Type"/>
    <rdfs:comment xml:lang="en">This property is used to indicate the specific manner in which the residence status which is indicated as holding over the actor pertains to this subject.

 
</rdfs:comment>
    <rdfs:label xml:lang="en">ascribes residence relation</rdfs:label>
    <skos:notation rdf:datatype="http://www.w3.org/2001/XMLSchema#string">ZP28</skos:notation>
    <rdfs:domain rdf:resource="https://ontology.swissartresearch.net/aaao/ZE9_Residential_Status"/>
    <rdfs:subPropertyOf rdf:resource="https://ontology.swissartresearch.net/aaao/ZP3_ascribes_intentional_relation"/>
  </rdf:Property>
  <rdf:Property rdf:about="https://ontology.swissartresearch.net/aaao/ZP29_has_familial_subject">
    <rdfs:range rdf:resource="http://www.cidoc-crm.org/cidoc-crm/E21_Person"/>
    <rdfs:comment xml:lang="en">This property is used to indicate the person for whom the family status is taken to hold.

 
</rdfs:comment>
    <rdfs:label xml:lang="en">has familial subject</rdfs:label>
    <skos:notation rdf:datatype="http://www.w3.org/2001/XMLSchema#string">ZP29</skos:notation>
    <rdfs:domain rdf:resource="https://ontology.swissartresearch.net/aaao/ZE10_Family_Status"/>
    <rdfs:subPropertyOf rdf:resource="https://ontology.swissartresearch.net/aaao/ZP105_has_social_relation_subject"/>
  </rdf:Property>
  <rdf:Property rdf:about="https://ontology.swissartresearch.net/aaao/ZP30_ascribes_relative">
    <rdfs:range rdf:resource="http://www.cidoc-crm.org/cidoc-crm/E21_Person"/>
    <rdfs:comment xml:lang="en">This property is used to indicate the person with whom the subject of the family relation status has the familial relation which they have. 

 
</rdfs:comment>
    <rdfs:label xml:lang="en">ascribes relative</rdfs:label>
    <skos:notation rdf:datatype="http://www.w3.org/2001/XMLSchema#string">ZP30</skos:notation>
    <rdfs:domain rdf:resource="https://ontology.swissartresearch.net/aaao/ZE10_Family_Status"/>
    <rdfs:subPropertyOf rdf:resource="https://ontology.swissartresearch.net/aaao/ZP103_ascribes_social_relation_target"/>
  </rdf:Property>
  <rdf:Property rdf:about="https://ontology.swissartresearch.net/aaao/ZP31_ascribes_familial_relation">
    <rdfs:range rdf:resource="http://www.cidoc-crm.org/cidoc-crm/E55_Type"/>
    <rdfs:comment xml:lang="en">This property is used to indicate the specific type of family status which is indicated as holding between the subject individual and his/her ascribed relative.

 
</rdfs:comment>
    <rdfs:label xml:lang="en">ascribes familial relation</rdfs:label>
    <skos:notation rdf:datatype="http://www.w3.org/2001/XMLSchema#string">ZP31</skos:notation>
    <rdfs:domain rdf:resource="https://ontology.swissartresearch.net/aaao/ZE10_Family_Status"/>
    <rdfs:subPropertyOf rdf:resource="https://ontology.swissartresearch.net/aaao/ZP104_ascribes_social_relation"/>
  </rdf:Property>
  <rdf:Property rdf:about="https://ontology.swissartresearch.net/aaao/ZP32_has_membership_subject">
    <rdfs:range rdf:resource="http://www.cidoc-crm.org/cidoc-crm/E39_Actor"/>
    <rdfs:comment xml:lang="en">This property is used to indicate the person or group for whom the membership status is taken to hold.

 
</rdfs:comment>
    <rdfs:label xml:lang="en">has membership subject</rdfs:label>
    <skos:notation rdf:datatype="http://www.w3.org/2001/XMLSchema#string">ZP32</skos:notation>
    <rdfs:domain rdf:resource="https://ontology.swissartresearch.net/aaao/ZE11_Membership_Status"/>
    <rdfs:subPropertyOf rdf:resource="https://ontology.swissartresearch.net/aaao/ZP1_has_intentional_subject"/>
  </rdf:Property>
  <rdf:Property rdf:about="https://ontology.swissartresearch.net/aaao/ZP33_ascribes_group">
    <rdfs:range rdf:resource="http://www.cidoc-crm.org/cidoc-crm/E74_Group"/>
    <rdfs:comment xml:lang="en">This property is used to indicate the group ascribed to the subject person of the membership status as having a membership relation thereto. 

 
</rdfs:comment>
    <rdfs:label xml:lang="en">ascribes group</rdfs:label>
    <skos:notation rdf:datatype="http://www.w3.org/2001/XMLSchema#string">ZP33</skos:notation>
    <rdfs:domain rdf:resource="https://ontology.swissartresearch.net/aaao/ZE11_Membership_Status"/>
    <rdfs:subPropertyOf rdf:resource="https://ontology.swissartresearch.net/aaao/ZP2_ascribes_intentional_target"/>
  </rdf:Property>
  <rdf:Property rdf:about="https://ontology.swissartresearch.net/aaao/ZP34_ascribes_membership_relation">
    <rdfs:range rdf:resource="http://www.cidoc-crm.org/cidoc-crm/E55_Type"/>
    <rdfs:comment xml:lang="en">This property is used to indicate the specific type of membership status which is indicated as holding between the subject actor and the group to which it is ascribed as being a member.

 
</rdfs:comment>
    <rdfs:label xml:lang="en">ascribes membership relation</rdfs:label>
    <skos:notation rdf:datatype="http://www.w3.org/2001/XMLSchema#string">ZP34</skos:notation>
    <rdfs:domain rdf:resource="https://ontology.swissartresearch.net/aaao/ZE11_Membership_Status"/>
    <rdfs:subPropertyOf rdf:resource="https://ontology.swissartresearch.net/aaao/ZP3_ascribes_intentional_relation"/>
  </rdf:Property>
  <rdf:Property rdf:about="https://ontology.swissartresearch.net/aaao/ZP35_has_referential_subject">
    <rdfs:range rdf:resource="http://www.cidoc-crm.org/cidoc-crm/E89_Propositional_Object"/>
    <rdfs:comment xml:lang="en">This property is used to indicate the propositional object for which the referential status is taken to hold.</rdfs:comment>
    <rdfs:label xml:lang="en">has referential subject</rdfs:label>
    <skos:notation rdf:datatype="http://www.w3.org/2001/XMLSchema#string">ZP35</skos:notation>
    <rdfs:domain rdf:resource="https://ontology.swissartresearch.net/aaao/ZE12_Referential_Status"/>
    <rdfs:subPropertyOf rdf:resource="https://ontology.swissartresearch.net/aaao/ZP1_has_intentional_subject"/>
  </rdf:Property>
  <rdf:Property rdf:about="https://ontology.swissartresearch.net/aaao/ZP36_ascribes_referent">
    <rdfs:range rdf:resource="http://www.cidoc-crm.org/cidoc-crm/E1_CRM_Entity"/>
    <rdfs:comment xml:lang="en">This property is used to indicate the referent to which the subject propositional object is taken to refer.

 
</rdfs:comment>
    <rdfs:label xml:lang="en">ascribes referent</rdfs:label>
    <skos:notation rdf:datatype="http://www.w3.org/2001/XMLSchema#string">ZP36</skos:notation>
    <rdfs:domain rdf:resource="https://ontology.swissartresearch.net/aaao/ZE12_Referential_Status"/>
    <rdfs:subPropertyOf rdf:resource="https://ontology.swissartresearch.net/aaao/ZP2_ascribes_intentional_target"/>
  </rdf:Property>
  <rdf:Property rdf:about="https://ontology.swissartresearch.net/aaao/ZP37_ascribes_referential_relation">
    <rdfs:range rdf:resource="http://www.cidoc-crm.org/cidoc-crm/E55_Type"/>
    <rdfs:comment xml:lang="en">This property is used to indicate the specific type of referential status which is indicated as holding between the subject propositional object and its indicated intended referent.

 
</rdfs:comment>
    <rdfs:label xml:lang="en">ascribes referential relation</rdfs:label>
    <skos:notation rdf:datatype="http://www.w3.org/2001/XMLSchema#string">ZP37</skos:notation>
    <rdfs:domain rdf:resource="https://ontology.swissartresearch.net/aaao/ZE12_Referential_Status"/>
    <rdfs:subPropertyOf rdf:resource="https://ontology.swissartresearch.net/aaao/ZP3_ascribes_intentional_relation"/>
  </rdf:Property>
  <rdf:Property rdf:about="https://ontology.swissartresearch.net/aaao/ZP38_ascribes_referential_mode">
    <rdfs:range rdf:resource="http://www.cidoc-crm.org/cidoc-crm/E55_Type"/>
    <rdfs:comment xml:lang="en">This property is used to indicate the specific manner in which the referential status which is indicated as holding between the subject propositional object and its indicated intended referent holds.

 
</rdfs:comment>
    <rdfs:label xml:lang="en">ascribes referential mode</rdfs:label>
    <skos:notation rdf:datatype="http://www.w3.org/2001/XMLSchema#string">ZP38</skos:notation>
    <rdfs:domain rdf:resource="https://ontology.swissartresearch.net/aaao/ZE12_Referential_Status"/>
  </rdf:Property>
  <rdf:Property rdf:about="https://ontology.swissartresearch.net/aaao/ZP40_performed">
    <rdfs:range rdf:resource="http://www.cidoc-crm.org/cidoc-crm/E29_Design_or_Procedure"/>
    <rdfs:comment xml:lang="en">This property is used to indicate the performance plan sanctioned by normative rule appealed to by a symbolic act in order to bring out the specific intended communicative effect. At a general level, the performance plan is what is appealed to in order to carry out the symbolic act in the first place. For example, an act of defiance may call on a specific sequence of gestures to be instantiated.
The case of speech act (ZE13) is a special case of symbolic act where the performance plan indicates the series of necessary procedures that must be followed in order for the speech act to have been successfully carried out and to have created a genuine instance of the institutional fact that it was designed to make possible.</rdfs:comment>
    <rdfs:label xml:lang="en">performed</rdfs:label>
    <skos:notation rdf:datatype="http://www.w3.org/2001/XMLSchema#string">ZP40</skos:notation>
    <rdfs:domain rdf:resource="https://ontology.swissartresearch.net/aaao/ZE53_Symbolic_Act"/>
    <rdfs:subPropertyOf rdf:resource="http://www.cidoc-crm.org/cidoc-crm/P33_used_specific_technique"/>
  </rdf:Property>
  <rdf:Property rdf:about="https://ontology.swissartresearch.net/aaao/ZP41_uttered">
    <rdfs:range rdf:resource="http://www.cidoc-crm.org/cidoc-crm/E73_Information_Object"/>
    <rdfs:comment xml:lang="en">It is typical of performance plans for normative procedures to include a necessary invoking clause or set of clauses which must be uttered in the course of the performance of the speech act in order to for it to be successfully carried out. This property enables the documentation of the use of such a linguistic object.</rdfs:comment>
    <rdfs:label xml:lang="en">uttered</rdfs:label>
    <skos:notation rdf:datatype="http://www.w3.org/2001/XMLSchema#string">ZP41</skos:notation>
    <rdfs:domain rdf:resource="https://ontology.swissartresearch.net/aaao/ZE13_Speech_Act"/>
    <rdfs:subPropertyOf rdf:resource="http://www.cidoc-crm.org/cidoc-crm/P16_used_specific_object"/>
  </rdf:Property>
  <rdf:Property rdf:about="https://ontology.swissartresearch.net/aaao/ZP42_intentionally_initiated">
    <rdfs:range rdf:resource="https://ontology.swissartresearch.net/aaao/ZE1_Institutional_Fact"/>
    <rdfs:comment xml:lang="en">This property is used to connect an instance of transformative symbolic act to the instance of institutional fact which it brought into existence through the successful performance of a specified norm type conformant symbolic act.

 
</rdfs:comment>
    <rdfs:label xml:lang="en">intentionally initiated</rdfs:label>
    <skos:notation rdf:datatype="http://www.w3.org/2001/XMLSchema#string">ZP42</skos:notation>
    <rdfs:domain rdf:resource="https://ontology.swissartresearch.net/aaao/ZE52_Transformative_Symbolic_Act"/>
    <rdfs:subPropertyOf rdf:resource="https://ontology.swissartresearch.net/aaao/ZP111_initiated"/>
  </rdf:Property>
  <rdf:Property rdf:about="https://ontology.swissartresearch.net/aaao/ZP43_has_similarity_subject">
    <rdfs:range rdf:resource="http://www.cidoc-crm.org/cidoc-crm/E1_CRM_Entity"/>
    <rdfs:comment xml:lang="en">This property is used to indicate one of two entities for which the similarity status is taken to hold.</rdfs:comment>
    <rdfs:label xml:lang="en">has similarity subject</rdfs:label>
    <skos:notation rdf:datatype="http://www.w3.org/2001/XMLSchema#string">ZP43</skos:notation>
    <rdfs:domain rdf:resource="https://ontology.swissartresearch.net/aaao/ZE14_Similarity_Status"/>
    <rdfs:subPropertyOf rdf:resource="https://ontology.swissartresearch.net/aaao/ZP1_has_intentional_subject"/>
  </rdf:Property>
  <rdf:Property rdf:about="https://ontology.swissartresearch.net/aaao/ZP44_ascribes_similarity_target">
    <rdfs:range rdf:resource="http://www.cidoc-crm.org/cidoc-crm/E1_CRM_Entity"/>
    <rdfs:comment xml:lang="en">This property is used to indicate the other entity for which the similarity status is taken to hold.</rdfs:comment>
    <rdfs:label xml:lang="en">ascribes similarity target</rdfs:label>
    <skos:notation rdf:datatype="http://www.w3.org/2001/XMLSchema#string">ZP44</skos:notation>
    <rdfs:domain rdf:resource="https://ontology.swissartresearch.net/aaao/ZE14_Similarity_Status"/>
    <rdfs:subPropertyOf rdf:resource="https://ontology.swissartresearch.net/aaao/ZP2_ascribes_intentional_target"/>
  </rdf:Property>
  <rdf:Property rdf:about="https://ontology.swissartresearch.net/aaao/ZP45_ascribes_similarity_relation">
    <rdfs:range rdf:resource="http://www.cidoc-crm.org/cidoc-crm/E55_Type"/>
    <rdfs:comment xml:lang="en">This property is used to indicate the specific type of similarity which is indicated as holding between the two entities indicated in the similarity status.</rdfs:comment>
    <rdfs:label xml:lang="en">ascribes similarity relation</rdfs:label>
    <skos:notation rdf:datatype="http://www.w3.org/2001/XMLSchema#string">ZP45</skos:notation>
    <rdfs:domain rdf:resource="https://ontology.swissartresearch.net/aaao/ZE14_Similarity_Status"/>
    <rdfs:subPropertyOf rdf:resource="https://ontology.swissartresearch.net/aaao/ZP3_ascribes_intentional_relation"/>
  </rdf:Property>
  <rdf:Property rdf:about="https://ontology.swissartresearch.net/aaao/ZP46_ascribes_similarity_mode">
    <rdfs:range rdf:resource="http://www.cidoc-crm.org/cidoc-crm/E55_Type"/>
    <rdfs:comment xml:lang="en">This property is used to indicate the specific manner in which the similarity status, which is indicated as holding between the two entities indicated in the similarity status, is the case. It''s function corresponds with the .1 properties in CIDOC-CRM 7.1.1.</rdfs:comment>
    <rdfs:label xml:lang="en">ascribes similarity mode</rdfs:label>
    <skos:notation rdf:datatype="http://www.w3.org/2001/XMLSchema#string">ZP46</skos:notation>
    <rdfs:domain rdf:resource="https://ontology.swissartresearch.net/aaao/ZE14_Similarity_Status"/>
  </rdf:Property>
  <rdf:Property rdf:about="https://ontology.swissartresearch.net/aaao/ZP47_has_set_belonging_subject">
    <rdfs:range rdf:resource="http://www.cidoc-crm.org/cidoc-crm/E1_CRM_Entity"/>
    <rdfs:comment xml:lang="en">This property is used to indicate an entity which is taken as belonging to a particular set by the instance of set status.</rdfs:comment>
    <rdfs:label xml:lang="en">has set belonging subject</rdfs:label>
    <skos:notation rdf:datatype="http://www.w3.org/2001/XMLSchema#string">ZP47</skos:notation>
    <rdfs:domain rdf:resource="https://ontology.swissartresearch.net/aaao/ZE15_Set_Status"/>
    <rdfs:subPropertyOf rdf:resource="https://ontology.swissartresearch.net/aaao/ZP1_has_intentional_subject"/>
  </rdf:Property>
  <rdf:Property rdf:about="https://ontology.swissartresearch.net/aaao/ZP48_ascribes_set">
    <rdfs:range rdf:resource="https://ontology.swissartresearch.net/aaao/ZE24_Notional_Set"/>
    <rdfs:comment xml:lang="en">This property is used to indicate the set to which an entity is indicated as belonging .</rdfs:comment>
    <rdfs:label xml:lang="en">ascribes set</rdfs:label>
    <skos:notation rdf:datatype="http://www.w3.org/2001/XMLSchema#string">ZP48</skos:notation>
    <rdfs:domain rdf:resource="https://ontology.swissartresearch.net/aaao/ZE15_Set_Status"/>
    <rdfs:subPropertyOf rdf:resource="https://ontology.swissartresearch.net/aaao/ZP2_ascribes_intentional_target"/>
  </rdf:Property>
  <rdf:Property rdf:about="https://ontology.swissartresearch.net/aaao/ZP49_ascribes_set_belonging_relation">
    <rdfs:range rdf:resource="http://www.cidoc-crm.org/cidoc-crm/E55_Type"/>
    <rdfs:comment xml:lang="en">This property is used to indicate the specific type of belonging to the set which is indicated as holding between the subject entity and the target set.</rdfs:comment>
    <rdfs:label xml:lang="en">ascribes set belonging relation</rdfs:label>
    <skos:notation rdf:datatype="http://www.w3.org/2001/XMLSchema#string">ZP49</skos:notation>
    <rdfs:domain rdf:resource="https://ontology.swissartresearch.net/aaao/ZE15_Set_Status"/>
    <rdfs:subPropertyOf rdf:resource="https://ontology.swissartresearch.net/aaao/ZP3_ascribes_intentional_relation"/>
  </rdf:Property>
  <rdf:Property rdf:about="https://ontology.swissartresearch.net/aaao/ZP51_has_former_or_current_set_member">
    <rdfs:range rdf:resource="http://www.cidoc-crm.org/cidoc-crm/E1_CRM_Entity"/>
    <rdfs:comment xml:lang="en">This property is used to connect an instance of set to an entity considered to be one of its members.</rdfs:comment>
    <rdfs:label xml:lang="en">has former or current set member</rdfs:label>
    <skos:notation rdf:datatype="http://www.w3.org/2001/XMLSchema#string">ZP51</skos:notation>
    <rdfs:domain rdf:resource="https://ontology.swissartresearch.net/aaao/ZE24_Notional_Set"/>
  </rdf:Property>
  <rdf:Property rdf:about="https://ontology.swissartresearch.net/aaao/ZP52_intentionally_terminated">
    <rdfs:range rdf:resource="https://ontology.swissartresearch.net/aaao/ZE1_Institutional_Fact"/>
    <rdfs:comment xml:lang="en">This property is used to connect an instance of transformative symbolic act to the instance of institutional fact which it cancels through the successful performance of a specified norm type conformant symbolic act.</rdfs:comment>
    <rdfs:label xml:lang="en">intentionally terminated</rdfs:label>
    <skos:notation rdf:datatype="http://www.w3.org/2001/XMLSchema#string">ZP52</skos:notation>
    <rdfs:domain rdf:resource="https://ontology.swissartresearch.net/aaao/ZE52_Transformative_Symbolic_Act"/>
    <rdfs:subPropertyOf rdf:resource="https://ontology.swissartresearch.net/aaao/ZP112_terminated"/>
  </rdf:Property>
  <rdf:Property rdf:about="https://ontology.swissartresearch.net/aaao/ZP54_ascribes_relative_date">
    <rdfs:range rdf:resource="http://www.cidoc-crm.org/cidoc-crm/E4_Period"/>
    <rdfs:comment xml:lang="en">This property is used to connect the instance of dating status to the instance of a period to which another instance of period is related for the purposes of datation.</rdfs:comment>
    <rdfs:label xml:lang="en">ascribes relative date</rdfs:label>
    <skos:notation rdf:datatype="http://www.w3.org/2001/XMLSchema#string">ZP54</skos:notation>
    <rdfs:domain rdf:resource="https://ontology.swissartresearch.net/aaao/ZE25_Dating_Status"/>
    <rdfs:subPropertyOf rdf:resource="https://ontology.swissartresearch.net/aaao/ZP2_ascribes_intentional_target"/>
  </rdf:Property>
  <rdf:Property rdf:about="https://ontology.swissartresearch.net/aaao/ZP55_has_dating_subject">
    <rdfs:range rdf:resource="http://www.cidoc-crm.org/cidoc-crm/E4_Period"/>
    <rdfs:comment xml:lang="en">This property is used to connect the instance of dating status to an instance of a period typically associated with the existence or use of a physical thing or an object which is the ultimate object of inquiry.</rdfs:comment>
    <rdfs:label xml:lang="en">has dating subject</rdfs:label>
    <skos:notation rdf:datatype="http://www.w3.org/2001/XMLSchema#string">ZP55</skos:notation>
    <rdfs:domain rdf:resource="https://ontology.swissartresearch.net/aaao/ZE25_Dating_Status"/>
    <rdfs:subPropertyOf rdf:resource="https://ontology.swissartresearch.net/aaao/ZP1_has_intentional_subject"/>
  </rdf:Property>
  <rdf:Property rdf:about="https://ontology.swissartresearch.net/aaao/ZP56_ascribes_dating_relation">
    <rdfs:range rdf:resource="http://www.cidoc-crm.org/cidoc-crm/E55_Type"/>
    <rdfs:comment xml:lang="en">This property is used to assign the type of relationship the dated period of the object under investigation bears towards the period assigned to it as its datation.</rdfs:comment>
    <rdfs:label xml:lang="en">ascribes dating relation</rdfs:label>
    <skos:notation rdf:datatype="http://www.w3.org/2001/XMLSchema#string">ZP56</skos:notation>
    <rdfs:domain rdf:resource="https://ontology.swissartresearch.net/aaao/ZE25_Dating_Status"/>
    <rdfs:subPropertyOf rdf:resource="https://ontology.swissartresearch.net/aaao/ZP3_ascribes_intentional_relation"/>
  </rdf:Property>
  <rdf:Property rdf:about="https://ontology.swissartresearch.net/aaao/ZP57_has_obligation_subject">
    <rdfs:range rdf:resource="http://www.cidoc-crm.org/cidoc-crm/E54_Dimension"/>
    <rdfs:comment xml:lang="en">This property is used to indicate a dimension which represents an amount of debt owed from one party to another within an instance of formal obligation.</rdfs:comment>
    <rdfs:label xml:lang="en">has obligation subject</rdfs:label>
    <skos:notation rdf:datatype="http://www.w3.org/2001/XMLSchema#string">ZP57</skos:notation>
    <rdfs:domain rdf:resource="https://ontology.swissartresearch.net/aaao/ZE28_Obligation_Status"/>
    <rdfs:subPropertyOf rdf:resource="https://ontology.swissartresearch.net/aaao/ZP89_has_promisory_subject"/>
  </rdf:Property>
  <rdf:Property rdf:about="https://ontology.swissartresearch.net/aaao/ZP58_ascribes_debtor">
    <rdfs:range rdf:resource="http://www.cidoc-crm.org/cidoc-crm/E39_Actor"/>
    <rdfs:comment xml:lang="en">This property is used to indicate an actor whom is bound by an obligation which it is their duty to repay.</rdfs:comment>
    <rdfs:label xml:lang="en">ascribes debtor</rdfs:label>
    <skos:notation rdf:datatype="http://www.w3.org/2001/XMLSchema#string">ZP58</skos:notation>
    <rdfs:domain rdf:resource="https://ontology.swissartresearch.net/aaao/ZE28_Obligation_Status"/>
    <rdfs:subPropertyOf rdf:resource="https://ontology.swissartresearch.net/aaao/ZP87_ascribes_promisor"/>
  </rdf:Property>
  <rdf:Property rdf:about="https://ontology.swissartresearch.net/aaao/ZP59_ascribes_obligation_relation">
    <rdfs:range rdf:resource="http://www.cidoc-crm.org/cidoc-crm/E55_Type"/>
    <rdfs:comment xml:lang="en">This property is used to indicate the specific type of obligation relation that holds between the debtor and the obligation.</rdfs:comment>
    <rdfs:label xml:lang="en">ascribes obligation relation</rdfs:label>
    <skos:notation rdf:datatype="http://www.w3.org/2001/XMLSchema#string">ZP59</skos:notation>
    <rdfs:domain rdf:resource="https://ontology.swissartresearch.net/aaao/ZE28_Obligation_Status"/>
    <rdfs:subPropertyOf rdf:resource="https://ontology.swissartresearch.net/aaao/ZP90_ascribes_promisory_relation"/>
  </rdf:Property>
  <rdf:Property rdf:about="https://ontology.swissartresearch.net/aaao/ZP60_ascribes_debtee">
    <rdfs:range rdf:resource="http://www.cidoc-crm.org/cidoc-crm/E39_Actor"/>
    <rdfs:comment xml:lang="en">This property is used to indicate the actor to whom an obligation is owed in the context of an obligation.</rdfs:comment>
    <rdfs:label xml:lang="en">ascribes debtee</rdfs:label>
    <skos:notation rdf:datatype="http://www.w3.org/2001/XMLSchema#string">ZP60</skos:notation>
    <rdfs:domain rdf:resource="https://ontology.swissartresearch.net/aaao/ZE28_Obligation_Status"/>
    <rdfs:subPropertyOf rdf:resource="https://ontology.swissartresearch.net/aaao/ZP86_ascribes_promissee"/>
  </rdf:Property>
  <rdf:Property rdf:about="https://ontology.swissartresearch.net/aaao/ZP61_transferred_property_right_to">
    <rdfs:range rdf:resource="http://www.cidoc-crm.org/cidoc-crm/E39_Actor"/>
    <rdfs:comment xml:lang="en">This property is used to indicate the receiver of a property right from another party within the context of a transfer of property right.</rdfs:comment>
    <rdfs:label xml:lang="en">transferred property right to</rdfs:label>
    <skos:notation rdf:datatype="http://www.w3.org/2001/XMLSchema#string">ZP61</skos:notation>
    <rdfs:domain rdf:resource="https://ontology.swissartresearch.net/aaao/ZE29_Transfer_of_Property_Right"/>
    <rdfs:subPropertyOf rdf:resource="http://www.cidoc-crm.org/cidoc-crm/P14_carried_out_by"/>
  </rdf:Property>
  <rdf:Property rdf:about="https://ontology.swissartresearch.net/aaao/ZP62_transferred_property_right_from">
    <rdfs:range rdf:resource="http://www.cidoc-crm.org/cidoc-crm/E39_Actor"/>
    <rdfs:comment xml:lang="en">This property is used to indicate the party ceding property right to another party within the context of a transfer of property right.</rdfs:comment>
    <rdfs:label xml:lang="en">transferred property right from</rdfs:label>
    <skos:notation rdf:datatype="http://www.w3.org/2001/XMLSchema#string">ZP62</skos:notation>
    <rdfs:domain rdf:resource="https://ontology.swissartresearch.net/aaao/ZE29_Transfer_of_Property_Right"/>
    <rdfs:subPropertyOf rdf:resource="http://www.cidoc-crm.org/cidoc-crm/P14_carried_out_by"/>
  </rdf:Property>
  <rdf:Property rdf:about="https://ontology.swissartresearch.net/aaao/ZP63_transferred_property_right_over">
    <rdfs:range rdf:resource="http://www.cidoc-crm.org/cidoc-crm/E72_Legal_Object"/>
    <rdfs:comment xml:lang="en">This property is used to indicate the legal object over which property right has been transfered from one party to another.</rdfs:comment>
    <rdfs:label xml:lang="en">transferred property right over</rdfs:label>
    <skos:notation rdf:datatype="http://www.w3.org/2001/XMLSchema#string">ZP63</skos:notation>
    <rdfs:domain rdf:resource="https://ontology.swissartresearch.net/aaao/ZE29_Transfer_of_Property_Right"/>
    <rdfs:subPropertyOf rdf:resource="http://www.cidoc-crm.org/cidoc-crm/P16_used_specific_object"/>
  </rdf:Property>
  <rdf:Property rdf:about="https://ontology.swissartresearch.net/aaao/ZP64_has_property_right_subject">
    <rdfs:range rdf:resource="http://www.cidoc-crm.org/cidoc-crm/E72_Legal_Object"/>
    <rdfs:comment xml:lang="en">This property is used to indicate an object that is subject to a property right of some actor.</rdfs:comment>
    <rdfs:label xml:lang="en">has property right subject</rdfs:label>
    <skos:notation rdf:datatype="http://www.w3.org/2001/XMLSchema#string">ZP64</skos:notation>
    <rdfs:domain rdf:resource="https://ontology.swissartresearch.net/aaao/ZE30_Property_Right_Status"/>
    <rdfs:subPropertyOf rdf:resource="https://ontology.swissartresearch.net/aaao/ZP1_has_intentional_subject"/>
  </rdf:Property>
  <rdf:Property rdf:about="https://ontology.swissartresearch.net/aaao/ZP65_ascribes_property_right_holder">
    <rdfs:range rdf:resource="http://www.cidoc-crm.org/cidoc-crm/E39_Actor"/>
    <rdfs:comment xml:lang="en">This property is used to indicate an actor who holds a right over a legal object within the context of a property right status.</rdfs:comment>
    <rdfs:label xml:lang="en">ascribes property right holder</rdfs:label>
    <skos:notation rdf:datatype="http://www.w3.org/2001/XMLSchema#string">ZP65</skos:notation>
    <rdfs:domain rdf:resource="https://ontology.swissartresearch.net/aaao/ZE30_Property_Right_Status"/>
    <rdfs:subPropertyOf rdf:resource="https://ontology.swissartresearch.net/aaao/ZP2_ascribes_intentional_target"/>
  </rdf:Property>
  <rdf:Property rdf:about="https://ontology.swissartresearch.net/aaao/ZP66_ascribes_property_right_relation">
    <rdfs:range rdf:resource="http://www.cidoc-crm.org/cidoc-crm/E55_Type"/>
    <rdfs:comment xml:lang="en">This property is used to indicate the specific type of property right relation that is held over the legal object by the actor in the context of a property right status.</rdfs:comment>
    <rdfs:label xml:lang="en">ascribes property right relation</rdfs:label>
    <skos:notation rdf:datatype="http://www.w3.org/2001/XMLSchema#string">ZP66</skos:notation>
    <rdfs:domain rdf:resource="https://ontology.swissartresearch.net/aaao/ZE30_Property_Right_Status"/>
    <rdfs:subPropertyOf rdf:resource="https://ontology.swissartresearch.net/aaao/ZP3_ascribes_intentional_relation"/>
  </rdf:Property>
  <rdf:Property rdf:about="https://ontology.swissartresearch.net/aaao/ZP67_generated_obligation_upon">
    <rdfs:range rdf:resource="http://www.cidoc-crm.org/cidoc-crm/E39_Actor"/>
    <rdfs:comment xml:lang="en">This property is used to indicate the party who owes another party within the the context of a declaration of obligation.</rdfs:comment>
    <rdfs:label xml:lang="en">generated obligation upon</rdfs:label>
    <skos:notation rdf:datatype="http://www.w3.org/2001/XMLSchema#string">ZP67</skos:notation>
    <rdfs:domain rdf:resource="https://ontology.swissartresearch.net/aaao/ZE27_Declaration_of_Obligation"/>
    <rdfs:subPropertyOf rdf:resource="http://www.cidoc-crm.org/cidoc-crm/P14_carried_out_by"/>
  </rdf:Property>
  <rdf:Property rdf:about="https://ontology.swissartresearch.net/aaao/ZP68_generated_obligation_to">
    <rdfs:range rdf:resource="http://www.cidoc-crm.org/cidoc-crm/E39_Actor"/>
    <rdfs:comment xml:lang="en">This property is used to indicate the party who is owed by another party within the the context of a declaration of obligation.</rdfs:comment>
    <rdfs:label xml:lang="en">generated obligation to</rdfs:label>
    <skos:notation rdf:datatype="http://www.w3.org/2001/XMLSchema#string">ZP68</skos:notation>
    <rdfs:domain rdf:resource="https://ontology.swissartresearch.net/aaao/ZE27_Declaration_of_Obligation"/>
    <rdfs:subPropertyOf rdf:resource="http://www.cidoc-crm.org/cidoc-crm/P14_carried_out_by"/>
  </rdf:Property>
  <rdf:Property rdf:about="https://ontology.swissartresearch.net/aaao/ZP69_generated_obligation_of">
    <rdfs:range rdf:resource="http://www.cidoc-crm.org/cidoc-crm/E54_Dimension"/>
    <rdfs:comment xml:lang="en">This property is used to indicate the specific amount owed by one party to another within the context of a declaration of obligation.</rdfs:comment>
    <rdfs:label xml:lang="en">generated obligation of</rdfs:label>
    <skos:notation rdf:datatype="http://www.w3.org/2001/XMLSchema#string">ZP69</skos:notation>
    <rdfs:domain rdf:resource="https://ontology.swissartresearch.net/aaao/ZE27_Declaration_of_Obligation"/>
  </rdf:Property>
  <rdf:Property rdf:about="https://ontology.swissartresearch.net/aaao/ZP70_ascribes_social_status_in_relation_to">
    <rdfs:range rdf:resource="http://www.cidoc-crm.org/cidoc-crm/E39_Actor"/>
    <rdfs:comment xml:lang="en">This property is used to indicate a third party actor for whom another''s social status holds relevance (in the form of rights and/or responsibilities that are thus due to them) in the instance of social status.</rdfs:comment>
    <rdfs:label xml:lang="en">ascribes social status in relation to</rdfs:label>
    <skos:notation rdf:datatype="http://www.w3.org/2001/XMLSchema#string">ZP70</skos:notation>
    <rdfs:domain rdf:resource="https://ontology.swissartresearch.net/aaao/ZE6_Social_Status"/>
  </rdf:Property>
  <rdf:Property rdf:about="https://ontology.swissartresearch.net/aaao/ZP75_applies_for_context">
    <rdfs:range rdf:resource="http://www.cidoc-crm.org/cidoc-crm/E5_Event"/>
    <rdfs:comment xml:lang="en">This property is used to indicate an event context which limits the temporal scope within which an instance of institutional fact is meant to hold. When indicated the event context stands as the frame in which the institutional fact is held to be valid by the associated group for whom it has significance.</rdfs:comment>
    <rdfs:label xml:lang="en">applies for context</rdfs:label>
    <skos:notation rdf:datatype="http://www.w3.org/2001/XMLSchema#string">ZP75</skos:notation>
    <rdfs:domain rdf:resource="https://ontology.swissartresearch.net/aaao/ZE1_Institutional_Fact"/>
  </rdf:Property>
  <rdf:Property rdf:about="https://ontology.swissartresearch.net/aaao/ZP76_applies_for_context_type">
    <rdfs:range rdf:resource="http://www.cidoc-crm.org/cidoc-crm/E55_Type"/>
    <rdfs:comment xml:lang="en">This property is used to indicate an event context type which limits the spatio-temporal scope within which an instance of institutional fact is meant to hold to certain kinds of event. When indicated the event context type stands as the frame or frames in which the institutional fact is held to be valid by the associated group for whom it has significance.</rdfs:comment>
    <rdfs:label xml:lang="en">applies for context type</rdfs:label>
    <skos:notation rdf:datatype="http://www.w3.org/2001/XMLSchema#string">ZP76</skos:notation>
    <rdfs:domain rdf:resource="https://ontology.swissartresearch.net/aaao/ZE1_Institutional_Fact"/>
  </rdf:Property>
  <rdf:Property rdf:about="https://ontology.swissartresearch.net/aaao/ZP77_ascribes_place">
    <rdfs:range rdf:resource="http://www.cidoc-crm.org/cidoc-crm/E53_Place"/>
    <rdfs:comment xml:lang="en">This property is used to indicate the place in a locative association that is taken to hold for an entity.</rdfs:comment>
    <rdfs:label xml:lang="en">ascribes place</rdfs:label>
    <skos:notation rdf:datatype="http://www.w3.org/2001/XMLSchema#string">ZP77</skos:notation>
    <rdfs:domain rdf:resource="https://ontology.swissartresearch.net/aaao/ZE35_Locative_Status"/>
    <rdfs:subPropertyOf rdf:resource="https://ontology.swissartresearch.net/aaao/ZP2_ascribes_intentional_target"/>
  </rdf:Property>
  <rdf:Property rdf:about="https://ontology.swissartresearch.net/aaao/ZP78_had_constituent">
    <rdfs:range rdf:resource="https://ontology.swissartresearch.net/aaao/ZE36_Persons"/>
    <rdfs:comment xml:lang="en">This property relates an instance of population to an instance of persons, individual or collective, to which it belongs qua constituent.</rdfs:comment>
    <rdfs:label xml:lang="en">had constituent</rdfs:label>
    <skos:notation rdf:datatype="http://www.w3.org/2001/XMLSchema#string">ZP78</skos:notation>
    <rdfs:domain rdf:resource="https://ontology.swissartresearch.net/aaao/ZE37_Population"/>
  </rdf:Property>
  <rdf:Property rdf:about="https://ontology.swissartresearch.net/aaao/ZP79_had_population">
    <rdfs:range rdf:resource="https://ontology.swissartresearch.net/aaao/ZE37_Population"/>
    <rdfs:comment xml:lang="en">This property relates an instance of population existence to the population whose existence it was.</rdfs:comment>
    <rdfs:label xml:lang="en">had population</rdfs:label>
    <skos:notation rdf:datatype="http://www.w3.org/2001/XMLSchema#string">ZP79</skos:notation>
    <rdfs:domain rdf:resource="https://ontology.swissartresearch.net/aaao/ZE38_Population_Existence"/>
    <rdfs:subPropertyOf rdf:resource="http://www.cidoc-crm.org/cidoc-crm/P11_had_participant"/>
  </rdf:Property>
  <rdf:Property rdf:about="https://ontology.swissartresearch.net/aaao/ZP83_has_physical_locative_subject">
    <rdfs:range rdf:resource="http://www.cidoc-crm.org/cidoc-crm/E18_Physical_Thing"/>
    <rdfs:comment xml:lang="en">This property is used to designate the instance of physical object whose socially defined location the instance of physical locative status delineates.</rdfs:comment>
    <rdfs:label xml:lang="en">has physical locative subject</rdfs:label>
    <skos:notation rdf:datatype="http://www.w3.org/2001/XMLSchema#string">ZP83</skos:notation>
    <rdfs:domain rdf:resource="https://ontology.swissartresearch.net/aaao/ZE43_Physical_Locative_Status"/>
    <rdfs:subPropertyOf rdf:resource="https://ontology.swissartresearch.net/aaao/ZP1_has_intentional_subject"/>
  </rdf:Property>
  <rdf:Property rdf:about="https://ontology.swissartresearch.net/aaao/ZP84_ascribes_location_relation">
    <rdfs:range rdf:resource="http://www.cidoc-crm.org/cidoc-crm/E55_Type"/>
    <rdfs:comment xml:lang="en">This property is used to indicate the specific manner in which the physical locative status which is indicated as holding over the physical object pertains to this subject.</rdfs:comment>
    <rdfs:label xml:lang="en">ascribes location relation</rdfs:label>
    <skos:notation rdf:datatype="http://www.w3.org/2001/XMLSchema#string">ZP84</skos:notation>
    <rdfs:domain rdf:resource="https://ontology.swissartresearch.net/aaao/ZE43_Physical_Locative_Status"/>
    <rdfs:subPropertyOf rdf:resource="https://ontology.swissartresearch.net/aaao/ZP3_ascribes_intentional_relation"/>
  </rdf:Property>
  <rdf:Property rdf:about="https://ontology.swissartresearch.net/aaao/ZP85_has_topographical_subject">
    <rdfs:range rdf:resource="http://www.cidoc-crm.org/cidoc-crm/E53_Place"/>
    <rdfs:comment xml:lang="en">This property is used to designate the instance of place whose socially defined location the instance of topographical status delineates.
 </rdfs:comment>
    <rdfs:label xml:lang="en">has topographical subject</rdfs:label>
    <skos:notation rdf:datatype="http://www.w3.org/2001/XMLSchema#string">ZP85</skos:notation>
    <rdfs:domain rdf:resource="https://ontology.swissartresearch.net/aaao/ZE44_Topographical_Status"/>
    <rdfs:subPropertyOf rdf:resource="https://ontology.swissartresearch.net/aaao/ZP1_has_intentional_subject"/>
  </rdf:Property>
  <rdf:Property rdf:about="https://ontology.swissartresearch.net/aaao/ZP86_ascribes_promissee">
    <rdfs:range rdf:resource="https://ontology.swissartresearch.net/aaao/ZE36_Persons"/>
    <rdfs:comment xml:lang="en">This property is used to indicate the actor to whom a promise has been offered in an intentional promise.</rdfs:comment>
    <rdfs:label xml:lang="en">ascribes promisee</rdfs:label>
    <skos:notation rdf:datatype="http://www.w3.org/2001/XMLSchema#string">ZP86</skos:notation>
    <rdfs:domain rdf:resource="https://ontology.swissartresearch.net/aaao/ZE45_Promisory_Status"/>
    <rdfs:subPropertyOf rdf:resource="https://ontology.swissartresearch.net/aaao/ZP2_ascribes_intentional_target"/>
  </rdf:Property>
  <rdf:Property rdf:about="https://ontology.swissartresearch.net/aaao/ZP87_ascribes_promisor">
    <rdfs:range rdf:resource="http://www.cidoc-crm.org/cidoc-crm/E39_Actor"/>
    <rdfs:comment xml:lang="en">This property is used to indicate an actor who is bound by a promise which it is their duty to fulfil.</rdfs:comment>
    <rdfs:label xml:lang="en">ascribes promisor</rdfs:label>
    <skos:notation rdf:datatype="http://www.w3.org/2001/XMLSchema#string">ZP87</skos:notation>
    <rdfs:domain rdf:resource="https://ontology.swissartresearch.net/aaao/ZE45_Promisory_Status"/>
    <rdfs:subPropertyOf rdf:resource="https://ontology.swissartresearch.net/aaao/ZP2_ascribes_intentional_target"/>
  </rdf:Property>
  <rdf:Property rdf:about="https://ontology.swissartresearch.net/aaao/ZP88_ascribes_topographical_relation">
    <rdfs:range rdf:resource="http://www.cidoc-crm.org/cidoc-crm/E55_Type"/>
    <rdfs:comment xml:lang="en">This property is used to indicate the specific manner in which the topographical status which is indicated as holding between two places.</rdfs:comment>
    <rdfs:label xml:lang="en">ascribes topographical relation</rdfs:label>
    <skos:notation rdf:datatype="http://www.w3.org/2001/XMLSchema#string">ZP88</skos:notation>
    <rdfs:domain rdf:resource="https://ontology.swissartresearch.net/aaao/ZE44_Topographical_Status"/>
    <rdfs:subPropertyOf rdf:resource="https://ontology.swissartresearch.net/aaao/ZP3_ascribes_intentional_relation"/>
  </rdf:Property>
  <rdf:Property rdf:about="https://ontology.swissartresearch.net/aaao/ZP89_has_promisory_subject">
    <rdfs:range rdf:resource="https://ontology.swissartresearch.net/aaao/ZE59_Plan"/>
    <rdfs:comment xml:lang="en">This property is used to indicate an instance of formulation which represents the promise given from one party to another within an instance of an intentional promise.</rdfs:comment>
    <rdfs:label xml:lang="en">has promissory subject</rdfs:label>
    <skos:notation rdf:datatype="http://www.w3.org/2001/XMLSchema#string">ZP89</skos:notation>
    <rdfs:domain rdf:resource="https://ontology.swissartresearch.net/aaao/ZE45_Promisory_Status"/>
    <rdfs:subPropertyOf rdf:resource="https://ontology.swissartresearch.net/aaao/ZP1_has_intentional_subject"/>
  </rdf:Property>
  <rdf:Property rdf:about="https://ontology.swissartresearch.net/aaao/ZP90_ascribes_promisory_relation">
    <rdfs:range rdf:resource="http://www.cidoc-crm.org/cidoc-crm/E55_Type"/>
    <rdfs:comment xml:lang="en">This property is used to indicate the specific type of promise relation that holds between the promisor and the promisee.</rdfs:comment>
    <rdfs:label xml:lang="en">ascribes promissory relation</rdfs:label>
    <skos:notation rdf:datatype="http://www.w3.org/2001/XMLSchema#string">ZP90</skos:notation>
    <rdfs:domain rdf:resource="https://ontology.swissartresearch.net/aaao/ZE45_Promisory_Status"/>
    <rdfs:subPropertyOf rdf:resource="https://ontology.swissartresearch.net/aaao/ZP3_ascribes_intentional_relation"/>
  </rdf:Property>
  <rdf:Property rdf:about="https://ontology.swissartresearch.net/aaao/ZP91_generated_promise_of">
    <rdfs:range rdf:resource="https://ontology.swissartresearch.net/aaao/ZE59_Plan"/>
    <rdfs:comment xml:lang="en">This property associates an instance of promissory agreement to the plan for a futural event (the realized promise) that it generates and which is promised through it.</rdfs:comment>
    <rdfs:label xml:lang="en">generated promise of</rdfs:label>
    <skos:notation rdf:datatype="http://www.w3.org/2001/XMLSchema#string">ZP91</skos:notation>
    <rdfs:domain rdf:resource="https://ontology.swissartresearch.net/aaao/ZE46_Promisory_Agreement"/>
    <rdfs:subPropertyOf rdf:resource="http://iflastandards.info/ns/lrm/lrmoo/R17"/>
  </rdf:Property>
  <rdf:Property rdf:about="https://ontology.swissartresearch.net/aaao/ZP93_has_text_sequence_subject">
    <rdfs:range rdf:resource="http://www.cidoc-crm.org/extensions/crmtex/TX4_Writing_Field"/>
    <rdfs:comment xml:lang="en">This property is used to indicate the text field which has been ascribed a sequential location in relation to another text field.</rdfs:comment>
    <rdfs:label xml:lang="en">has text sequence subject</rdfs:label>
    <skos:notation rdf:datatype="http://www.w3.org/2001/XMLSchema#string">ZP93</skos:notation>
    <rdfs:domain rdf:resource="https://ontology.swissartresearch.net/aaao/ZE49_Text_Sequence_Status"/>
    <rdfs:subPropertyOf rdf:resource="https://ontology.swissartresearch.net/aaao/ZP1_has_intentional_subject"/>
  </rdf:Property>
  <rdf:Property rdf:about="https://ontology.swissartresearch.net/aaao/ZP94_ascribes_text_sequence_correlate">
    <rdfs:range rdf:resource="http://www.cidoc-crm.org/extensions/crmtex/TX4_Writing_Field"/>
    <rdfs:comment xml:lang="en">This property is used to designate a text field to which another text field has been assigned in order to designate its relative place.</rdfs:comment>
    <rdfs:label xml:lang="en">ascribes text sequence correlate</rdfs:label>
    <skos:notation rdf:datatype="http://www.w3.org/2001/XMLSchema#string">ZP94</skos:notation>
    <rdfs:domain rdf:resource="https://ontology.swissartresearch.net/aaao/ZE49_Text_Sequence_Status"/>
    <rdfs:subPropertyOf rdf:resource="https://ontology.swissartresearch.net/aaao/ZP2_ascribes_intentional_target"/>
  </rdf:Property>
  <rdf:Property rdf:about="https://ontology.swissartresearch.net/aaao/ZP95_ascribes_text_sequence_relation">
    <rdfs:range rdf:resource="http://www.cidoc-crm.org/cidoc-crm/E55_Type"/>
    <rdfs:comment xml:lang="en">This property is used to indicate the specific manner in which the text sequence status which is indicated as holding over the textual sequence pertains to this subject.</rdfs:comment>
    <rdfs:label xml:lang="en">ascribes text sequence relation</rdfs:label>
    <skos:notation rdf:datatype="http://www.w3.org/2001/XMLSchema#string">ZP95</skos:notation>
    <rdfs:domain rdf:resource="https://ontology.swissartresearch.net/aaao/ZE49_Text_Sequence_Status"/>
    <rdfs:subPropertyOf rdf:resource="https://ontology.swissartresearch.net/aaao/ZP3_ascribes_intentional_relation"/>
  </rdf:Property>
  <rdf:Property rdf:about="https://ontology.swissartresearch.net/aaao/ZP96_has_authority_status_subject">
    <rdfs:range rdf:resource="http://www.cidoc-crm.org/cidoc-crm/E39_Actor"/>
    <rdfs:comment xml:lang="en">This property is used to indicate the actor which has been ascribed an authority status.</rdfs:comment>
    <rdfs:label xml:lang="en">has authority status subject</rdfs:label>
    <skos:notation rdf:datatype="http://www.w3.org/2001/XMLSchema#string">ZP96</skos:notation>
    <rdfs:domain rdf:resource="https://ontology.swissartresearch.net/aaao/ZE50_Authority_Status"/>
    <rdfs:subPropertyOf rdf:resource="https://ontology.swissartresearch.net/aaao/ZP17_has_social_status_subject"/>
  </rdf:Property>
  <rdf:Property rdf:about="https://ontology.swissartresearch.net/aaao/ZP97_ascribes_authority_status">
    <rdfs:range rdf:resource="http://www.cidoc-crm.org/cidoc-crm/E55_Type"/>
    <rdfs:comment xml:lang="en">This property is used to indicate the type of authority ascribed to the actor by the authority status.</rdfs:comment>
    <rdfs:label xml:lang="en">ascribes authority status</rdfs:label>
    <skos:notation rdf:datatype="http://www.w3.org/2001/XMLSchema#string">ZP97</skos:notation>
    <rdfs:domain rdf:resource="https://ontology.swissartresearch.net/aaao/ZE50_Authority_Status"/>
    <rdfs:subPropertyOf rdf:resource="https://ontology.swissartresearch.net/aaao/ZP18_ascribes_social_status"/>
  </rdf:Property>
  <rdf:Property rdf:about="https://ontology.swissartresearch.net/aaao/ZP100_challenged">
    <rdfs:range rdf:resource="https://ontology.swissartresearch.net/aaao/ZE1_Institutional_Fact"/>
    <rdfs:comment xml:lang="en">This property links an instance of symbolic act with an instance of institutional fact which it challenges through its performance.</rdfs:comment>
    <rdfs:label xml:lang="en">challenged</rdfs:label>
    <skos:notation rdf:datatype="http://www.w3.org/2001/XMLSchema#string">ZP100</skos:notation>
    <rdfs:domain rdf:resource="https://ontology.swissartresearch.net/aaao/ZE53_Symbolic_Act"/>
  </rdf:Property>
  <rdf:Property rdf:about="https://ontology.swissartresearch.net/aaao/ZP101_affirmed">
    <rdfs:range rdf:resource="https://ontology.swissartresearch.net/aaao/ZE1_Institutional_Fact"/>
    <rdfs:comment xml:lang="en">This property links an instance of symbolic act with an instance of institutional fact which it affirms through its performance.</rdfs:comment>
    <rdfs:label xml:lang="en">affirmed</rdfs:label>
    <skos:notation rdf:datatype="http://www.w3.org/2001/XMLSchema#string">ZP101</skos:notation>
    <rdfs:domain rdf:resource="https://ontology.swissartresearch.net/aaao/ZE53_Symbolic_Act"/>
  </rdf:Property>
  <rdf:Property rdf:about="https://ontology.swissartresearch.net/aaao/ZP103_ascribes_social_relation_target">
    <rdfs:range rdf:resource="http://www.cidoc-crm.org/cidoc-crm/E39_Actor"/>
    <rdfs:comment xml:lang="en">This property is used to indicate the person with whom the subject of the social relation status has the social relation which they have.</rdfs:comment>
    <rdfs:label xml:lang="en">ascribes social relation target</rdfs:label>
    <skos:notation rdf:datatype="http://www.w3.org/2001/XMLSchema#string">ZP103</skos:notation>
    <rdfs:domain rdf:resource="https://ontology.swissartresearch.net/aaao/ZE55_Social_Relation_Status"/>
    <rdfs:subPropertyOf rdf:resource="https://ontology.swissartresearch.net/aaao/ZP2_ascribes_intentional_target"/>
  </rdf:Property>
  <rdf:Property rdf:about="https://ontology.swissartresearch.net/aaao/ZP104_ascribes_social_relation">
    <rdfs:range rdf:resource="http://www.cidoc-crm.org/cidoc-crm/E55_Type"/>
    <rdfs:comment xml:lang="en">This property is used to indicate the specific type of social relation status which is indicated as holding between the subject individual and their ascribed social relative.</rdfs:comment>
    <rdfs:label xml:lang="en">ascribes social relation</rdfs:label>
    <skos:notation rdf:datatype="http://www.w3.org/2001/XMLSchema#string">ZP104</skos:notation>
    <rdfs:domain rdf:resource="https://ontology.swissartresearch.net/aaao/ZE55_Social_Relation_Status"/>
    <rdfs:subPropertyOf rdf:resource="https://ontology.swissartresearch.net/aaao/ZP3_ascribes_intentional_relation"/>
  </rdf:Property>
  <rdf:Property rdf:about="https://ontology.swissartresearch.net/aaao/ZP105_has_social_relation_subject">
    <rdfs:range rdf:resource="http://www.cidoc-crm.org/cidoc-crm/E39_Actor"/>
    <rdfs:comment xml:lang="en">This property is used to indicate the person for whom the social relation status is taken to hold.</rdfs:comment>
    <rdfs:label xml:lang="en">has social relation subject</rdfs:label>
    <skos:notation rdf:datatype="http://www.w3.org/2001/XMLSchema#string">ZP105</skos:notation>
    <rdfs:domain rdf:resource="https://ontology.swissartresearch.net/aaao/ZE55_Social_Relation_Status"/>
    <rdfs:subPropertyOf rdf:resource="https://ontology.swissartresearch.net/aaao/ZP1_has_intentional_subject"/>
  </rdf:Property>
  <rdf:Property rdf:about="https://ontology.swissartresearch.net/aaao/ZP111_initiated">
    <rdfs:range rdf:resource="https://ontology.swissartresearch.net/aaao/ZE1_Institutional_Fact"/>
    <rdfs:comment xml:lang="en">This property is used to connect the instance of event to the instance of institutional fact which it brought into existence by fiat thanks to its accordance to a socially defined norm. In this case the bringing about of a new institutional fact need not be intentional or following any particular rule intentionally. Rather, within a social context it is recognized that the very fact of a particular event occurring is causal to the initiation of the related social fact. For example, in certain property right laws, the very fact of writing down an idea (E65 Creation) initiates an instance of property right over the generated information object, regardless of the intention or not of the author to so create such a right.</rdfs:comment>
    <rdfs:label xml:lang="en">initiated</rdfs:label>
    <skos:notation rdf:datatype="http://www.w3.org/2001/XMLSchema#string">ZP111</skos:notation>
    <rdfs:domain rdf:resource="http://www.cidoc-crm.org/cidoc-crm/E5_Event"/>
  </rdf:Property>
  <rdf:Property rdf:about="https://ontology.swissartresearch.net/aaao/ZP112_terminated">
    <rdfs:range rdf:resource="https://ontology.swissartresearch.net/aaao/ZE1_Institutional_Fact"/>
    <rdfs:comment xml:lang="en">This property is used to connect the instance of event to the instance of institutional fact which it terminated the existence of by fiat thanks to its accordance to a socially defined norm. In this case the cancellation of an institutional fact need not be intentional or following any particular rule intentionally. Rather, within a social context it is recognized that the very fact of a particular event occurring is causal to the cancellation of the related social fact. For example, a certain social system may recognize that an ''act of god'' such as an earthquake may terminate the property right of an individual over some object (another social system may not, however).</rdfs:comment>
    <rdfs:label xml:lang="en">terminated</rdfs:label>
    <skos:notation rdf:datatype="http://www.w3.org/2001/XMLSchema#string">ZP112</skos:notation>
    <rdfs:domain rdf:resource="http://www.cidoc-crm.org/cidoc-crm/E5_Event"/>
  </rdf:Property>
  <rdf:Property rdf:about="https://ontology.swissartresearch.net/aaao/ZP113_has_successor_status">
    <rdfs:range rdf:resource="https://ontology.swissartresearch.net/aaao/ZE1_Institutional_Fact"/>
    <rdfs:comment xml:lang="en">This property links one instance of institutional fact with another where the latter succeeds the former as a formal continuation.</rdfs:comment>
    <rdfs:label xml:lang="en">has successor status</rdfs:label>
    <skos:notation rdf:datatype="http://www.w3.org/2001/XMLSchema#string">ZP113</skos:notation>
    <rdfs:domain rdf:resource="https://ontology.swissartresearch.net/aaao/ZE1_Institutional_Fact"/>
  </rdf:Property>
  <rdf:Property rdf:about="https://ontology.swissartresearch.net/aaao/ZP114_has_geographic_scope">
    <rdfs:range rdf:resource="http://www.cidoc-crm.org/cidoc-crm/E53_Place"/>
    <rdfs:comment xml:lang="en">This property is used to connect an institutional fact to a place, which defines the scope of that facts spatial validity.</rdfs:comment>
    <rdfs:label xml:lang="en">has geographic scope</rdfs:label>
    <skos:notation rdf:datatype="http://www.w3.org/2001/XMLSchema#string">ZP114</skos:notation>
    <rdfs:domain rdf:resource="https://ontology.swissartresearch.net/aaao/ZE1_Institutional_Fact"/>
  </rdf:Property>
  <rdf:Property rdf:about="https://ontology.swissartresearch.net/aaao/ZP115_holds_over">
    <rdfs:range rdf:resource="https://ontology.swissartresearch.net/aaao/ZE37_Population"/>
    <rdfs:comment xml:lang="en">This property associates and instance of institutional fact to an instance of population over which this fact holds. As opposed to the property of ZP4 holding for, the effect which this institutional fact holds in relation to the related population is not necessarily one which has been directly intended. The population undergoes the social fact instantiated, rather than causing it to occur directly through agency in a speech act or transformative act. The population is the patient of this operation, not its agent.</rdfs:comment>
    <rdfs:label xml:lang="en">holds over</rdfs:label>
    <skos:notation rdf:datatype="http://www.w3.org/2001/XMLSchema#string">ZP115</skos:notation>
    <rdfs:domain rdf:resource="https://ontology.swissartresearch.net/aaao/ZE1_Institutional_Fact"/>
  </rdf:Property>
  <rdf:Property rdf:about="https://ontology.swissartresearch.net/aaao/ZP116_ascribes_authority_status_relation">
    <rdfs:range rdf:resource="http://www.cidoc-crm.org/cidoc-crm/E55_Type"/>
    <rdfs:comment xml:lang="en">This property is used to indicate the specific manner in which the type of authority status which is indicated as holding for the subject pertains to this subject.</rdfs:comment>
    <rdfs:label xml:lang="en">ascribes authority status relation</rdfs:label>
    <skos:notation rdf:datatype="http://www.w3.org/2001/XMLSchema#string">ZP116</skos:notation>
    <rdfs:domain rdf:resource="https://ontology.swissartresearch.net/aaao/ZE50_Authority_Status"/>
    <rdfs:subPropertyOf rdf:resource="https://ontology.swissartresearch.net/aaao/ZP3_ascribes_intentional_relation"/>
  </rdf:Property>
  <rdf:Property rdf:about="https://ontology.swissartresearch.net/aaao/ZP117_generated_promise_to">
    <rdfs:range rdf:resource="https://ontology.swissartresearch.net/aaao/ZE36_Persons"/>
    <rdfs:comment xml:lang="en">This property is used to indicate the persons to whom a promise is made, when two parties reach a promissory agreement.</rdfs:comment>
    <rdfs:label xml:lang="en">generated promise to</rdfs:label>
    <skos:notation rdf:datatype="http://www.w3.org/2001/XMLSchema#string">ZP117</skos:notation>
    <rdfs:domain rdf:resource="https://ontology.swissartresearch.net/aaao/ZE46_Promisory_Agreement"/>
    <rdfs:subPropertyOf rdf:resource="http://www.cidoc-crm.org/cidoc-crm/P11_had_participant"/>
  </rdf:Property>
  <rdf:Property rdf:about="https://ontology.swissartresearch.net/aaao/ZP118_generated_promise_upon">
    <rdfs:range rdf:resource="http://www.cidoc-crm.org/cidoc-crm/E39_Actor"/>
    <rdfs:comment xml:lang="en">This property is used to indicate the actor upon whom an obligation is generated when two parties reach a promissory agreement.</rdfs:comment>
    <rdfs:label xml:lang="en">generated promise upon</rdfs:label>
    <skos:notation rdf:datatype="http://www.w3.org/2001/XMLSchema#string">ZP118</skos:notation>
    <rdfs:domain rdf:resource="https://ontology.swissartresearch.net/aaao/ZE46_Promisory_Agreement"/>
    <rdfs:subPropertyOf rdf:resource="http://www.cidoc-crm.org/cidoc-crm/P14_carried_out_by"/>
  </rdf:Property>
  <rdf:Property rdf:about="https://ontology.swissartresearch.net/aaao/ZP119_ascribes_event_location_relation">
    <rdfs:range rdf:resource="http://www.cidoc-crm.org/cidoc-crm/E55_Type"/>
    <rdfs:comment xml:lang="en">This property is used to indicate the specific type of event locative status which is indicated as holding between the subject event and its ascribed place.</rdfs:comment>
    <rdfs:label xml:lang="en">ascribes event location relation</rdfs:label>
    <skos:notation rdf:datatype="http://www.w3.org/2001/XMLSchema#string">ZP119</skos:notation>
    <rdfs:domain rdf:resource="https://ontology.swissartresearch.net/aaao/ZE60_Evental_Locative_Status"/>
    <rdfs:subPropertyOf rdf:resource="https://ontology.swissartresearch.net/aaao/ZP3_ascribes_intentional_relation"/>
  </rdf:Property>
  <rdf:Property rdf:about="https://ontology.swissartresearch.net/aaao/ZP120_has_event_location_subject">
    <rdfs:range rdf:resource="http://www.cidoc-crm.org/cidoc-crm/E5_Event"/>
    <rdfs:comment xml:lang="en">This property is used to indicate the event which has been ascribed a place.</rdfs:comment>
    <rdfs:label xml:lang="en">has event location subject</rdfs:label>
    <skos:notation rdf:datatype="http://www.w3.org/2001/XMLSchema#string">ZP120</skos:notation>
    <rdfs:domain rdf:resource="https://ontology.swissartresearch.net/aaao/ZE60_Evental_Locative_Status"/>
    <rdfs:subPropertyOf rdf:resource="https://ontology.swissartresearch.net/aaao/ZP1_has_intentional_subject"/>
  </rdf:Property>
  <rdf:Property rdf:about="https://ontology.swissartresearch.net/aaao/ZP121_involved">
    <rdfs:range rdf:resource="https://ontology.swissartresearch.net/aaao/ZE36_Persons"/>
    <rdfs:comment xml:lang="en">This property describes the passive involvement of instances of ZE39 Persons in an instance of E5 Event.</rdfs:comment>
    <rdfs:label xml:lang="en">involved</rdfs:label>
    <skos:notation rdf:datatype="http://www.w3.org/2001/XMLSchema#string">ZP121</skos:notation>
    <rdfs:domain rdf:resource="http://www.cidoc-crm.org/cidoc-crm/E5_Event"/>
    <rdfs:subPropertyOf rdf:resource="http://www.cidoc-crm.org/cidoc-crm/P12_occurred_in_the_presence_of"/>
  </rdf:Property>
</rdf:RDF>
